Implemented oalists

OAlist/OAlist.thy
@@ -1,167 +1,800 @@
+(* Author: Florian Haftmann, TU Muenchen *)
+(* Author: Andreas Lochbihler, ETH Zurich *)
+(* Author: Alexander Maletzky, RISC Linz *)
+
+section \<open>Associative Lists with Sorted Keys\<close>
+
 theory OAlist
-  imports OAlist_Impl
+  imports Deriving.Comparator
 begin
 
-type_synonym 'a comp_opt = "'a \<Rightarrow> 'a \<Rightarrow> (comparison option)"
+text \<open>We define the type of @{emph \<open>ordered associative lists\<close>} (oalist). An oalist is an associative
+  list (i.\,e. a list of pairs) such that the keys are distinct and sorted wrt. some linear
+  order relation, and no key is mapped to @{term 0}. The latter invariant allows to implement various
+  functions operating on oalists more efficiently.
 
-subsection \<open>A Type Class for @{term compare} that is independent of order relations\<close>
+  The ordering of the keys in an oalist \<open>xs\<close> is encoded as an additional parameter of \<open>xs\<close>.
+  This means that oalists may be ordered wrt. different orderings, even if they are of the same type.
+  Operations operating on more than one oalists, like \<open>map2_val\<close>, typically ensure that the orderings
+  of their arguments are identical by re-ordering one argument wrt. the order relation of the other.
+  This, however, implies that equality of order relations must be effectively decidable if executable
+  code is to be generated.\<close>
 
-class compare =
-  fixes compare :: "'a comparator"
-  assumes compare_greater: "compare x y = GREATER \<longleftrightarrow> compare y x = LESS"
-  assumes compare_equal: "compare x y = EQUAL \<longleftrightarrow> x = y"
-  assumes compare_trans: "compare x y = LESS \<Longrightarrow> compare y z = LESS \<Longrightarrow> compare x z = LESS"
-begin
+subsection \<open>Preliminaries\<close>
 
-lemma compare_same [simp]: "compare x x = EQUAL"
-  by (simp add: compare_equal)
+fun min_list_param :: "('a \<Rightarrow> 'a \<Rightarrow> bool) \<Rightarrow> 'a list \<Rightarrow> 'a" where
+  "min_list_param rel (x # xs) = (case xs of [] \<Rightarrow> x | _ \<Rightarrow> (let m = min_list_param rel xs in if rel x m then x else m))"
 
-lemma uminus_compare [simp]: "- compare x y = compare y x"
-  by (metis comparison.exhaust local.compare_greater uminus_eq_GREATER_iff uminus_eq_LESS_iff)
-
-lemma comparator_eq_on_compare [simp]: "comparator_eq_on compare D"
-  by (unfold_locales, auto simp: compare_equal intro: compare_trans)
-
-abbreviation "less_eq_of_comp \<equiv> c.less_eq_of_comparator compare"
-abbreviation "less_of_comp \<equiv> c.less_of_comparator compare"
-abbreviation "greater_eq_of_comp \<equiv> c.less_eq_of_comparator (- compare)"
-abbreviation "greater_of_comp \<equiv> c.less_of_comparator (- compare)"
-
-lemma less_eq_of_comp_alt: "less_eq_of_comp = (\<lambda>x y. compare x y \<noteq> GREATER)"
-  by (meson c.less_eq_of_comparator_def)
-
-lemma less_of_comp_alt: "less_of_comp = (\<lambda>x y. compare x y = LESS)"
-  by (meson c.less_of_comparator_def)
-
-lemma reflp_less_eq_of_comp: "reflp less_eq_of_comp"
-  by (simp add: c.less_eq_of_comparator_def reflpI)
-
-lemma irreflp_less_of_comp: "irreflp less_of_comp"
-  by (simp add: c.less_of_comparator_def irreflpI)
-
-lemma transp_less_eq_of_comp: "transp less_eq_of_comp"
-  by (smt c.less_eq_of_comparator_def comparison.exhaust compare_equal compare_trans transpI)
-
-lemma transp_less_of_comp: "transp less_of_comp"
-  by (smt c.less_of_comparator_def comparison.exhaust compare_equal compare_trans transpI)
-
-lemma antisymp_less_eq_of_comp: "antisymp less_eq_of_comp"
-  by (metis (no_types, lifting) antisympI c.less_eq_of_comparator_def comparison.exhaust compare_equal compare_greater)
-
-lemma asymp_less_of_comp: "asymp less_of_comp"
-  by (metis asymp.intros irreflp_def irreflp_less_of_comp transpD transp_less_of_comp)
-
-lemma greater_eq_of_comp_alt: "greater_eq_of_comp = (\<lambda>x y. less_eq_of_comp y x)"
-  by (metis c.less_eq_of_comparator_def uminus_compare uminus_apply)
-
-lemma greater_of_comp_alt: "greater_of_comp = (\<lambda>x y. less_of_comp y x)"
-  by (metis c.less_of_comparator_def uminus_compare uminus_apply)
-
-fun update_by' :: "('a \<times> 'b) \<Rightarrow> ('a \<times> 'b) list \<Rightarrow> ('a \<times> 'b::zero) list"
-where
-  "update_by' (k, v) [] = (if v = 0 then [] else [(k, v)])"
-| "update_by' (k, v) ((k', v') # xs) =
-  (case compare k k' of LESS \<Rightarrow> (if v = 0 then (k', v') # xs else (k, v) # (k', v') # xs)
-                     | EQUAL \<Rightarrow> (if v = 0 then xs else (k, v) # xs)
-                   | GREATER \<Rightarrow> (k', v') # update_by' (k, v) xs)"
-
-fun update_by_fun_raw :: "'a \<Rightarrow> ('b \<Rightarrow> 'b) \<Rightarrow> ('a \<times> 'b) list \<Rightarrow> ('a \<times> 'b::zero) list"
-where
-  "update_by_fun_raw k f [] = (let v = f 0 in if v = 0 then [] else [(k, v)])"
-| "update_by_fun_raw k f ((k', v') # xs) =
-  (case compare k k' of LESS \<Rightarrow> (let v = f 0 in if v = 0 then (k', v') # xs else (k, v) # (k', v') # xs)
-                     | EQUAL \<Rightarrow> (let v = f v' in if v = 0 then xs else (k, v) # xs)
-                   | GREATER \<Rightarrow> (k', v') # update_by_fun_raw k f xs)"
-
-fun update_by_fun_gr_raw :: "'a \<Rightarrow> ('b \<Rightarrow> 'b) \<Rightarrow> ('a \<times> 'b) list \<Rightarrow> ('a \<times> 'b::zero) list"
-  where "update_by_fun_gr_raw k f xs =
-          (if xs = [] then
-            (let v = f 0 in if v = 0 then [] else [(k, v)])
-          else if compare k (fst (last xs)) = GREATER then
-            (let v = f 0 in if v = 0 then xs else xs @ [(k, v)])
-          else
-            update_by_fun_raw k f xs
-          )"
-
-fun map_val_raw :: "('a \<Rightarrow> 'b \<Rightarrow> 'c) \<Rightarrow> ('a \<times> 'b::zero) list \<Rightarrow> ('a \<times> 'c::zero) list"
-where
-  "map_val_raw f [] = []"
-| "map_val_raw f ((kx, vx) # xs) =
-    (let v = f kx vx; aux = map_val_raw f xs in if v = 0 then aux else (kx, v) # aux)"
-
-(*
-fun map2_val_raw_tr :: "('a \<Rightarrow> 'b \<Rightarrow> 'c \<Rightarrow> 'd) \<Rightarrow> ('a \<times> 'b::zero) list \<Rightarrow> ('a \<times> 'c::zero) list \<Rightarrow> ('a \<times> 'd::zero) list \<Rightarrow>
-                        ('a \<times> 'd::zero) list"
-where
-  "map2_val_raw_tr f [] [] acc = acc"
-| "map2_val_raw_tr f [] ((ky, vy) # ys) acc =
-    (let v = f ky 0 vy in map2_val_raw_tr f [] ys (if v = 0 then acc else (ky, v) # acc))"
-| "map2_val_raw_tr f ((kx, vx) # xs) [] acc =
-    (let v = f kx vx 0 in map2_val_raw_tr f xs [] (if v = 0 then acc else (kx, v) # acc))"
-| "map2_val_raw_tr f ((kx, vx) # xs) ((ky, vy) # ys) acc =
-    (case compare kx ky of LESS \<Rightarrow> (let v = f kx vx 0 in map2_val_raw_tr f xs ((ky, vy) # ys) (if v = 0 then acc else (kx, v) # acc))
-                        | EQUAL \<Rightarrow> (let v = f kx vx vy in map2_val_raw_tr f xs ys (if v = 0 then acc else (kx, v) # acc))
-                      | GREATER \<Rightarrow> (let v = f ky 0 vy in map2_val_raw_tr f ((kx, vx) # xs) ys (if v = 0 then acc else (ky, v) # acc)))"
-
-definition "map2_val_raw f xs ys = rev (map2_val_raw_tr f xs ys [])"
-*)
-
-fun map2_val_neutr_raw :: "('a \<Rightarrow> 'b \<Rightarrow> 'b \<Rightarrow> 'b) \<Rightarrow> ('a \<times> 'b::zero) list \<Rightarrow> ('a \<times> 'b::zero) list \<Rightarrow> ('a \<times> 'b::zero) list"
-where
-  "map2_val_neutr_raw f xs [] = xs"
-| "map2_val_neutr_raw f [] ys = ys"
-| "map2_val_neutr_raw f ((kx, vx) # xs) ((ky, vy) # ys) =
-    (case compare kx ky of LESS \<Rightarrow> (let v = f kx vx 0; aux = map2_val_neutr_raw f xs ((ky, vy) # ys) in if v = 0 then aux else (kx, v) # aux)
-                        | EQUAL \<Rightarrow> (let v = f kx vx vy; aux = map2_val_neutr_raw f xs ys in if v = 0 then aux else (kx, v) # aux)
-                      | GREATER \<Rightarrow> (let v = f ky 0 vy; aux = map2_val_neutr_raw f ((kx, vx) # xs) ys in if v = 0 then aux else (ky, v) # aux))"
-
-fun map2_val_rneutr_raw :: "('a \<Rightarrow> 'b \<Rightarrow> 'c \<Rightarrow> 'b) \<Rightarrow> ('a \<times> 'b::zero) list \<Rightarrow> ('a \<times> 'c::zero) list \<Rightarrow> ('a \<times> 'b::zero) list"
-where
-  "map2_val_rneutr_raw f xs [] = xs"
-| "map2_val_rneutr_raw f [] ((ky, vy) # ys) =
-    (let v = f ky 0 vy; aux = map2_val_rneutr_raw f [] ys in if v = 0 then aux else (ky, v) # aux)"
-| "map2_val_rneutr_raw f ((kx, vx) # xs) ((ky, vy) # ys) =
-    (case compare kx ky of LESS \<Rightarrow> (let v = f kx vx 0; aux = map2_val_rneutr_raw f xs ((ky, vy) # ys) in if v = 0 then aux else (kx, v) # aux)
-                        | EQUAL \<Rightarrow> (let v = f kx vx vy; aux = map2_val_rneutr_raw f xs ys in if v = 0 then aux else (kx, v) # aux)
-                      | GREATER \<Rightarrow> (let v = f ky 0 vy; aux = map2_val_rneutr_raw f ((kx, vx) # xs) ys in if v = 0 then aux else (ky, v) # aux))"
-
-text \<open>In addition to @{const map2_val_rneutr_raw} one could define \<open>map2_val_lneutr_raw\<close> and \<open>map2_val_raw\<close>,
-  but we do not need them.\<close>
-
-fun lex_ord_raw :: "('a \<Rightarrow> ('b comp_opt)) \<Rightarrow> (('a \<times> 'b::zero) list) comp_opt"
-where
-  "lex_ord_raw f []       []       = Some EQUAL"
-| "lex_ord_raw f []       ((ky, vy) # ys) =
-    (let aux = f ky 0 vy in if aux = Some EQUAL then lex_ord_raw f [] ys else aux)"
-| "lex_ord_raw f ((kx, vx) # xs) []       =
-    (let aux = f kx vx 0 in if aux = Some EQUAL then lex_ord_raw f xs [] else aux)"
-| "lex_ord_raw f ((kx, vx) # xs) ((ky, vy) # ys) =
-  (case compare kx ky of LESS    \<Rightarrow> (let aux = f kx vx 0 in if aux = Some EQUAL then lex_ord_raw f xs ((ky, vy) # ys) else aux)
-                       | EQUAL   \<Rightarrow> (let aux = f kx vx vy in if aux = Some EQUAL then lex_ord_raw f xs ys else aux)
-                       | GREATER \<Rightarrow> (let aux = f ky 0 vy in if aux = Some EQUAL then lex_ord_raw f ((kx, vx) # xs) ys else aux))"
-
-fun prod_ord_raw :: "('a \<Rightarrow> 'b \<Rightarrow> 'c \<Rightarrow> bool) \<Rightarrow> ('a \<times> 'b::zero) list \<Rightarrow> ('a \<times> 'c::zero) list \<Rightarrow> bool"
-where
-  "prod_ord_raw f []       []       = True"
-| "prod_ord_raw f []       ((ky, vy) # ys) = (f ky 0 vy \<and> prod_ord_raw f [] ys)"
-| "prod_ord_raw f ((kx, vx) # xs) []       = (f kx vx 0 \<and> prod_ord_raw f xs [])"
-| "prod_ord_raw f ((kx, vx) # xs) ((ky, vy) # ys) =
-  (case compare kx ky of LESS    \<Rightarrow> (f kx vx 0 \<and> prod_ord_raw f xs ((ky, vy) # ys))
-                     | EQUAL   \<Rightarrow> (f kx vx vy \<and> prod_ord_raw f xs ys)
-                     | GREATER \<Rightarrow> (f ky 0 vy \<and> prod_ord_raw f ((kx, vx) # xs) ys))"
-
-lemma update_by'_eq_update_by:
-  assumes "v \<noteq> 0"
-  shows "update_by' (k, v) xs = c.update_by compare k v xs"
-proof (induct xs, simp add: assms)
-  fix xs and x::"'a \<times> 'b"
-  assume IH: "update_by' (k, v) xs = c.update_by compare_class.compare k v xs"
-  obtain k' v' where x: "x = (k', v')" by fastforce
-  show "update_by' (k, v) (x # xs) = c.update_by compare_class.compare k v (x # xs)"
-    by (simp add: x assms IH cong: comparison.case_cong)
+lemma min_list_param_in:
+  assumes "xs \<noteq> []"
+  shows "min_list_param rel xs \<in> set xs"
+  using assms
+proof (induct xs)
+  case Nil
+  thus ?case by simp
+next
+  case (Cons x xs)
+  show ?case
+  proof (simp add: min_list_param.simps[of rel x xs] Let_def del: min_list_param.simps set_simps(2) split: list.split,
+        intro conjI impI allI, simp, simp)
+    fix y ys
+    assume xs: "xs = y # ys"
+    have "min_list_param rel (y # ys) = min_list_param rel xs" by (simp only: xs)
+    also have "... \<in> set xs" by (rule Cons(1), simp add: xs)
+    also have "... \<subseteq> set (x # y # ys)" by (auto simp: xs)
+    finally show "min_list_param rel (y # ys) \<in> set (x # y # ys)" .
+  qed
 qed
 
-lemma set_update_by'_subset: "set (update_by' kv xs) \<subseteq> insert kv (set xs)"
+lemma min_list_param_minimal:
+  assumes "transp rel" and "\<And>x y. x \<in> set xs \<Longrightarrow> y \<in> set xs \<Longrightarrow> rel x y \<or> rel y x"
+    and "z \<in> set xs"
+  shows "rel (min_list_param rel xs) z"
+  using assms(2, 3)
+proof (induct xs)
+  case Nil
+  from Nil(2) show ?case by simp
+next
+  case (Cons x xs)
+  from Cons(3) have disj1: "z = x \<or> z \<in> set xs" by simp
+  have "x \<in> set (x # xs)" by simp
+  hence disj2: "rel x z \<or> rel z x" using Cons(3) by (rule Cons(2))
+  have *: "rel (min_list_param rel xs) z" if "z \<in> set xs" using _ that
+  proof (rule Cons(1))
+    fix a b
+    assume "a \<in> set xs" and "b \<in> set xs"
+    hence "a \<in> set (x # xs)" and "b \<in> set (x # xs)" by simp_all
+    thus "rel a b \<or> rel b a" by (rule Cons(2))
+  qed
+  show ?case
+  proof (simp add: min_list_param.simps[of rel x xs] Let_def del: min_list_param.simps set_simps(2) split: list.split,
+        intro conjI impI allI)
+    assume "xs = []"
+    with disj1 disj2 show "rel x z" by simp
+  next
+    fix y ys
+    assume "xs = y # ys" and "rel x (min_list_param rel (y # ys))"
+    hence "rel x (min_list_param rel xs)" by simp
+    from disj1 show "rel x z"
+    proof
+      assume "z = x"
+      thus ?thesis using disj2 by simp
+    next
+      assume "z \<in> set xs"
+      hence "rel (min_list_param rel xs) z" by (rule *)
+      with assms(1) \<open>rel x (min_list_param rel xs)\<close> show ?thesis by (rule transpD)
+    qed
+  next
+    fix y ys
+    assume xs: "xs = y # ys" and "\<not> rel x (min_list_param rel (y # ys))"
+    from disj1 show "rel (min_list_param rel (y # ys)) z"
+    proof
+      assume "z = x"
+      have "min_list_param rel (y # ys) \<in> set (y # ys)" by (rule min_list_param_in, simp)
+      hence "min_list_param rel (y # ys) \<in> set (x # xs)" by (simp add: xs)
+      with \<open>x \<in> set (x # xs)\<close> have "rel x (min_list_param rel (y # ys)) \<or> rel (min_list_param rel (y # ys)) x"
+        by (rule Cons(2))
+      with \<open>\<not> rel x (min_list_param rel (y # ys))\<close> have "rel (min_list_param rel (y # ys)) x" by simp
+      thus ?thesis by (simp only: \<open>z = x\<close>)
+    next
+      assume "z \<in> set xs"
+      hence "rel (min_list_param rel xs) z" by (rule *)
+      thus ?thesis by (simp only: xs)
+    qed
+  qed
+qed
+
+(*
+subsection \<open>Syntactic Type Class for Default Elements\<close>
+
+text \<open>We do not want to use the existing type-class @{class default}, but instead introduce a new one:\<close>
+
+class oalist_dflt = fixes dflt::'a
+
+simproc_setup reorient_dflt ("dflt = x") = Reorient_Proc.proc
+*)
+
+subsection \<open>Type \<open>key_order\<close>\<close>
+
+typedef 'a key_order = "{compare :: 'a comparator. comparator compare}"
+  morphisms key_compare Abs_key_order
+proof -
+  from well_order_on obtain r where "well_order_on (UNIV::'a set) r" ..
+  hence "linear_order r" by (simp only: well_order_on_def)
+  hence lin: "(x, y) \<in> r \<or> (y, x) \<in> r" for x y
+    by (metis Diff_iff Linear_order_in_diff_Id UNIV_I \<open>well_order r\<close> well_order_on_Field)
+  have antisym: "(x, y) \<in> r \<Longrightarrow> (y, x) \<in> r \<Longrightarrow> x = y" for x y
+    by (meson \<open>linear_order r\<close> antisymD linear_order_on_def partial_order_on_def)
+  have trans: "(x, y) \<in> r \<Longrightarrow> (y, z) \<in> r \<Longrightarrow> (x, z) \<in> r" for x y z
+    by (meson \<open>linear_order r\<close> linear_order_on_def order_on_defs(1) partial_order_on_def trans_def)
+  define comp where "comp = (\<lambda>x y. if (x, y) \<in> r then if (y, x) \<in> r then Eq else Lt else Gt)"
+  show ?thesis
+  proof (rule, simp)
+    show "comparator comp"
+    proof (standard, simp_all add: comp_def split: if_splits, intro impI)
+      fix x y
+      assume "(x, y) \<in> r" and "(y, x) \<in> r"
+      thus "x = y" by (rule antisym)
+    next
+      fix x y
+      assume "(x, y) \<notin> r"
+      with lin show "(y, x) \<in> r" by blast
+    next
+      fix x y z
+      assume "(y, x) \<notin> r" and "(z, y) \<notin> r"
+      assume "(x, y) \<in> r" and "(y, z) \<in> r"
+      hence "(x, z) \<in> r" by (rule trans)
+      moreover have "(z, x) \<notin> r"
+      proof
+        assume "(z, x) \<in> r"
+        with \<open>(x, z) \<in> r\<close> have "x = z" by (rule antisym)
+        from \<open>(z, y) \<notin> r\<close> \<open>(x, y) \<in> r\<close> show False unfolding \<open>x = z\<close> ..
+      qed
+      ultimately show "(z, x) \<notin> r \<and> ((z, x) \<notin> r \<longrightarrow> (x, z) \<in> r)" by simp
+    qed
+  qed
+qed
+
+lemma comparator_key_compare [simp, intro!]: "comparator (key_compare ko)"
+  using key_compare[of ko] by simp
+
+instantiation key_order :: (type) equal
+begin
+  definition equal_key_order :: "'a key_order \<Rightarrow> 'a key_order \<Rightarrow> bool" where "equal_key_order = (=)"
+  instance by (standard, simp add: equal_key_order_def)
+end
+
+setup_lifting type_definition_key_order
+
+instantiation key_order :: (type) uminus
+begin
+
+lift_definition uminus_key_order :: "'a key_order \<Rightarrow> 'a key_order" is "\<lambda>c x y. invert_order (c x y)"
+proof -
+  fix comp::"'a comparator"
+  assume "comparator comp"
+  then interpret comp: comparator comp .
+  show "comparator (\<lambda>x y. invert_order (comp x y))"
+  proof
+    fix x y
+    assume "invert_order (comp x y) = Eq"
+    thus "x = y" using comp.sym comp.weak_eq by auto
+  next
+    fix x y
+    show "invert_order (invert_order (comp x y)) = invert_order (comp y x)" by (simp add: comp.sym)
+  next
+    fix x y z
+    assume "invert_order (comp x y) = Lt" and "invert_order (comp y z) = Lt"
+    hence "comp z y = Lt" and "comp y x = Lt" by (simp_all add: comp.sym)
+    hence "comp z x = Lt" by (rule comp.trans)
+    thus "invert_order (comp x z) = Lt" by (simp only: comp.sym)
+  qed
+qed
+
+instance ..
+
+end
+
+lift_definition le_of_key_order :: "'a key_order \<Rightarrow> 'a \<Rightarrow> 'a \<Rightarrow> bool" is "\<lambda>cmp. le_of_comp cmp" .
+
+lift_definition lt_of_key_order :: "'a key_order \<Rightarrow> 'a \<Rightarrow> 'a \<Rightarrow> bool" is "\<lambda>cmp. lt_of_comp cmp" .
+
+definition key_order_of_ord :: "('a \<Rightarrow> 'a \<Rightarrow> bool) \<Rightarrow> 'a key_order"
+  where "key_order_of_ord ord = Abs_key_order (comp_of_ords ord (\<lambda>x y. ord x y \<and> \<not> ord y x))"
+
+lift_definition key_order_of_le :: "'a::linorder key_order" is comparator_of
+  by (fact comparator_of)
+
+interpretation key_order_lin: linorder "le_of_key_order ko" "lt_of_key_order ko"
+proof transfer
+  fix comp::"'a comparator"
+  assume "comparator comp"
+  then interpret comp: comparator comp .
+  show "class.linorder comp.le comp.lt" by (fact comp.linorder)
+qed
+
+lemma le_of_key_order_alt: "le_of_key_order ko x y = (key_compare ko x y \<noteq> Gt)"
+  by (transfer, simp add: comparator.nGt_le_conv)
+
+lemma lt_of_key_order_alt: "lt_of_key_order ko x y = (key_compare ko x y = Lt)"
+  by (transfer, meson comparator.Lt_lt_conv)
+
+lemma key_compare_Gt: "key_compare ko x y = Gt \<longleftrightarrow> key_compare ko y x = Lt"
+  by (transfer, meson comparator.nGt_le_conv comparator.nLt_le_conv)
+
+lemma key_compare_Eq: "key_compare ko x y = Eq \<longleftrightarrow> x = y"
+  by (transfer, simp add: comparator.eq)
+
+lemma key_compare_same [simp]: "key_compare ko x x = Eq"
+  by (simp add: key_compare_Eq)
+
+lemma uminus_key_compare [simp]: "invert_order (key_compare ko x y) = key_compare ko y x"
+  by (transfer, simp add: comparator.sym)
+
+lemma key_compare_uminus [simp]: "key_compare (- ko) x y = key_compare ko y x"
+proof -
+  have "key_compare (- ko) x y = invert_order (key_compare ko x y)" by (transfer, rule refl)
+  also have "... = key_compare ko y x" by simp
+  finally show ?thesis .
+qed
+
+lemma uminus_key_order_sameD:
+  assumes "- ko = (ko::'a key_order)"
+  shows "x = (y::'a)"
+proof (rule ccontr)
+  assume "x \<noteq> y"
+  hence "key_compare ko x y \<noteq> Eq" by (simp add: key_compare_Eq)
+  hence "key_compare ko x y \<noteq> invert_order (key_compare ko x y)"
+    by (metis invert_order.elims order.distinct(5))
+  also have "invert_order (key_compare ko x y) = key_compare (- ko) x y" by simp
+  finally have "- ko \<noteq> ko" by (auto simp del: key_compare_uminus)
+  thus False using assms ..
+qed
+
+lemma key_compare_key_order_of_ord:
+  assumes "antisymp ord" and "transp ord" and "\<And>x y. ord x y \<or> ord y x"
+  shows "key_compare (key_order_of_ord ord) = (\<lambda>x y. if ord x y then if x = y then Eq else Lt else Gt)"
+proof -
+  have eq: "key_compare (key_order_of_ord ord) = comp_of_ords ord (\<lambda>x y. ord x y \<and> \<not> ord y x)"
+    unfolding key_order_of_ord_def
+  proof (rule Abs_key_order_inverse, simp, rule comp_of_ords, unfold_locales)
+    fix x
+    from assms(3) show "ord x x" by blast
+  next
+    fix x y z
+    assume "ord x y" and "ord y z"
+    with assms(2) show "ord x z" by (rule transpD)
+  next
+    fix x y
+    assume "ord x y" and "ord y x"
+    with assms(1) show "x = y" by (rule antisympD)
+  qed (rule refl, rule assms(3))
+  have *: "x = y" if "ord x y" and "ord y x" for x y using assms(1) that by (rule antisympD)
+  show ?thesis by (rule, rule, auto simp: eq comp_of_ords_def intro: *)
+qed
+
+lemma key_compare_key_order_of_le:
+  "key_compare key_order_of_le = (\<lambda>x y. if x < y then Lt else if x = y then Eq else Gt)"
+  by (transfer, intro ext, fact comparator_of_def)
+
+subsection \<open>Invariant\<close>
+
+definition oalist_inv :: "(('a \<times> 'b::zero) list \<times> ('a key_order)) \<Rightarrow> bool"
+  where "oalist_inv xs \<longleftrightarrow> (0 \<notin> snd ` set (fst xs) \<and> sorted_wrt (lt_of_key_order (snd xs)) (map fst (fst xs)))"
+
+lemma oalist_invI:
+  assumes "0 \<notin> snd ` set xs" and "sorted_wrt (lt_of_key_order ko) (map fst xs)"
+  shows "oalist_inv (xs, ko)"
+  unfolding oalist_inv_def using assms unfolding fst_conv snd_conv by blast
+
+lemma oalist_invD1:
+  assumes "oalist_inv (xs, ko)"
+  shows "0 \<notin> snd ` set xs"
+  using assms unfolding oalist_inv_def fst_conv by blast
+
+lemma oalist_invD2:
+  assumes "oalist_inv (xs, ko)"
+  shows "sorted_wrt (lt_of_key_order ko) (map fst xs)"
+  using assms unfolding oalist_inv_def fst_conv snd_conv by blast
+
+lemma oalist_inv_Nil: "oalist_inv ([], ko)"
+  by (simp add: oalist_inv_def)
+
+lemma oalist_inv_singleton: "oalist_inv ([(k, v)], ko) \<longleftrightarrow> (v \<noteq> 0)"
+  by (auto simp: oalist_inv_def)
+
+lemma oalist_inv_ConsI:
+  assumes "oalist_inv (xs, ko)" and "v \<noteq> 0" and "xs \<noteq> [] \<Longrightarrow> lt_of_key_order ko k (fst (hd xs))"
+  shows "oalist_inv ((k, v) # xs, ko)"
+proof (rule oalist_invI)
+  from assms(1) have "0 \<notin> snd ` set xs" by (rule oalist_invD1)
+  with assms(2) show "0 \<notin> snd ` set ((k, v) # xs)" by simp
+next
+  show "sorted_wrt (lt_of_key_order ko) (map fst ((k, v) # xs))"
+  proof (cases "xs = []")
+    case True
+    thus ?thesis by simp
+  next
+    case False
+    then obtain k' v' xs' where xs: "xs = (k', v') # xs'" by (metis list.exhaust prod.exhaust)
+    from assms(3)[OF False] have "lt_of_key_order ko k k'" by (simp add: xs)
+    moreover from assms(1) have "sorted_wrt (lt_of_key_order ko) (map fst xs)" by (rule oalist_invD2)
+    ultimately show "sorted_wrt (lt_of_key_order ko) (map fst ((k, v) # xs))"
+      by (simp add: xs sorted_wrt2[OF key_order_lin.transp_less] del: sorted_wrt.simps)
+  qed
+qed
+
+lemma oalist_inv_ConsD1:
+  assumes "oalist_inv (x # xs, ko)"
+  shows "oalist_inv (xs, ko)"
+proof (rule oalist_invI)
+  from assms have "0 \<notin> snd ` set (x # xs)" by (rule oalist_invD1)
+  thus "0 \<notin> snd ` set xs" by simp
+next
+  from assms have "sorted_wrt (lt_of_key_order ko) (map fst (x # xs))" by (rule oalist_invD2)
+  thus "sorted_wrt (lt_of_key_order ko) (map fst xs)" by simp
+qed
+
+lemma oalist_inv_ConsD2:
+  assumes "oalist_inv ((k, v) # xs, ko)"
+  shows "v \<noteq> 0"
+proof -
+  from assms have "0 \<notin> snd ` set ((k, v) # xs)" by (rule oalist_invD1)
+  thus ?thesis by auto
+qed
+
+lemma oalist_inv_ConsD3:
+  assumes "oalist_inv ((k, v) # xs, ko)" and "k' \<in> fst ` set xs"
+  shows "lt_of_key_order ko k k'"
+proof -
+  from assms(2) obtain x where "x \<in> set xs" and "k' = fst x" by fastforce
+  from assms(1) have "sorted_wrt (lt_of_key_order ko) (map fst ((k, v) # xs))" by (rule oalist_invD2)
+  hence "\<forall>x\<in>set xs. lt_of_key_order ko k (fst x)" by simp
+  hence "lt_of_key_order ko k (fst x)" using \<open>x \<in> set xs\<close> ..
+  thus ?thesis by (simp only: \<open>k' = fst x\<close>)
+qed
+
+lemma oalist_inv_tl:
+  assumes "oalist_inv (xs, ko)"
+  shows "oalist_inv (tl xs, ko)"
+proof (rule oalist_invI)
+  from assms have "0 \<notin> snd ` set xs" by (rule oalist_invD1)
+  thus "0 \<notin> snd ` set (tl xs)" by (metis (no_types, lifting) image_iff list.set_sel(2) tl_Nil)
+next
+  show "sorted_wrt (lt_of_key_order ko) (map fst (tl xs))"
+    by (metis hd_Cons_tl oalist_invD2 oalist_inv_ConsD1 assms tl_Nil)
+qed
+
+lemma oalist_inv_filter:
+  assumes "oalist_inv (xs, ko)"
+  shows "oalist_inv (filter P xs, ko)"
+proof (rule oalist_invI)
+  from assms have "0 \<notin> snd ` set xs" by (rule oalist_invD1)
+  thus "0 \<notin> snd ` set (filter P xs)" by auto
+next
+  from assms have "sorted_wrt (lt_of_key_order ko) (map fst xs)" by (rule oalist_invD2)
+  thus "sorted_wrt (lt_of_key_order ko) (map fst (filter P xs))" by (induct xs, simp, simp)
+qed
+
+lemma oalist_inv_map:
+  assumes "oalist_inv (xs, ko)"
+    and "\<And>a. snd (f a) = 0 \<Longrightarrow> snd a = 0"
+    and "\<And>a b. key_compare ko (fst (f a)) (fst (f b)) = key_compare ko (fst a) (fst b)"
+  shows "oalist_inv (map f xs, ko)"
+proof (rule oalist_invI)
+  show "0 \<notin> snd ` set (map f xs)"
+  proof (simp, rule)
+    assume "0 \<in> snd ` f ` set xs"
+    then obtain a where "a \<in> set xs" and "snd (f a) = 0" by fastforce
+    from this(2) have "snd a = 0" by (rule assms(2))
+    from assms(1) have "0 \<notin> snd ` set xs" by (rule oalist_invD1)
+    moreover from \<open>a \<in> set xs\<close> have "0 \<in> snd ` set xs" by (simp add: \<open>snd a = 0\<close>[symmetric])
+    ultimately show False ..
+  qed
+next
+  from assms(1) have "sorted_wrt (lt_of_key_order ko) (map fst xs)" by (rule oalist_invD2)
+  hence "sorted_wrt (\<lambda>x y. key_compare ko (fst x) (fst y) = Lt) xs"
+    by (simp only: sorted_wrt_map lt_of_key_order_alt)
+  thus "sorted_wrt (lt_of_key_order ko) (map fst (map f xs))"
+    by (simp add: sorted_wrt_map lt_of_key_order_alt assms(3))
+qed
+
+lemma oalist_inv_induct [consumes 1, case_names Nil Cons]:
+  assumes "oalist_inv (xs, ko)"
+  assumes "P []"
+  assumes "\<And>k v xs. oalist_inv ((k, v) # xs, ko) \<Longrightarrow> oalist_inv (xs, ko) \<Longrightarrow> v \<noteq> 0 \<Longrightarrow>
+              (\<And>k'. k' \<in> fst ` set xs \<Longrightarrow> lt_of_key_order ko k k') \<Longrightarrow> P xs \<Longrightarrow> P ((k, v) # xs)"
+  shows "P xs"
+  using assms(1)
+proof (induct xs)
+  case Nil
+  from assms(2) show ?case .
+next
+  case (Cons x xs)
+  obtain k v where x: "x = (k, v)" by fastforce
+  from Cons(2) have "oalist_inv ((k, v) # xs, ko)" and "oalist_inv (xs, ko)" and "v \<noteq> 0" unfolding x
+    by (this, rule oalist_inv_ConsD1, rule oalist_inv_ConsD2)
+  moreover from Cons(2) have "lt_of_key_order ko k k'" if "k' \<in> fst ` set xs" for k' using that
+    unfolding x by (rule oalist_inv_ConsD3)
+  moreover from \<open>oalist_inv (xs, ko)\<close> have "P xs" by (rule Cons(1))
+  ultimately show ?case unfolding x by (rule assms(3))
+qed
+
+subsection \<open>Operations on Lists of Pairs\<close>
+
+type_synonym ('a, 'b) comp_opt = "'a \<Rightarrow> 'b \<Rightarrow> (order option)"
+
+context fixes ko :: "'a key_order"
+begin
+
+fun lookup_pair :: "('a \<times> 'b) list \<Rightarrow> 'a \<Rightarrow> 'b::zero"
+where
+  "lookup_pair [] x = 0"|
+  "lookup_pair ((k, v) # xs) x =
+    (case key_compare ko x k of
+       Lt \<Rightarrow> 0
+     | Eq \<Rightarrow> v
+     | Gt \<Rightarrow> lookup_pair xs x)"
+
+fun update_by_pair :: "('a \<times> 'b) \<Rightarrow> ('a \<times> 'b) list \<Rightarrow> ('a \<times> 'b::zero) list"
+where
+  "update_by_pair (k, v) [] = (if v = 0 then [] else [(k, v)])"
+| "update_by_pair (k, v) ((k', v') # xs) =
+  (case key_compare ko k k' of Lt \<Rightarrow> (if v = 0 then (k', v') # xs else (k, v) # (k', v') # xs)
+                     | Eq \<Rightarrow> (if v = 0 then xs else (k, v) # xs)
+                   | Gt \<Rightarrow> (k', v') # update_by_pair (k, v) xs)"
+
+(* TODO: Add update_by_gr_pair. *)
+
+definition sort_oalist :: "('a \<times> 'b) list \<Rightarrow> ('a \<times> 'b::zero) list"
+  where "sort_oalist xs = foldr update_by_pair xs []"
+
+fun update_by_fun_pair :: "'a \<Rightarrow> ('b \<Rightarrow> 'b) \<Rightarrow> ('a \<times> 'b) list \<Rightarrow> ('a \<times> 'b::zero) list"
+where
+  "update_by_fun_pair k f [] = (let v = f 0 in if v = 0 then [] else [(k, v)])"
+| "update_by_fun_pair k f ((k', v') # xs) =
+  (case key_compare ko k k' of Lt \<Rightarrow> (let v = f 0 in if v = 0 then (k', v') # xs else (k, v) # (k', v') # xs)
+                     | Eq \<Rightarrow> (let v = f v' in if v = 0 then xs else (k, v) # xs)
+                   | Gt \<Rightarrow> (k', v') # update_by_fun_pair k f xs)"
+
+definition update_by_fun_gr_pair :: "'a \<Rightarrow> ('b \<Rightarrow> 'b) \<Rightarrow> ('a \<times> 'b) list \<Rightarrow> ('a \<times> 'b::zero) list"
+  where "update_by_fun_gr_pair k f xs =
+          (if xs = [] then
+            (let v = f 0 in if v = 0 then [] else [(k, v)])
+          else if key_compare ko k (fst (last xs)) = Gt then
+            (let v = f 0 in if v = 0 then xs else xs @ [(k, v)])
+          else
+            update_by_fun_pair k f xs
+          )"
+
+fun map_pair :: "(('a \<times> 'b) \<Rightarrow> ('a \<times> 'c)) \<Rightarrow> ('a \<times> 'b::zero) list \<Rightarrow> ('a \<times> 'c::zero) list"
+where
+  "map_pair f [] = []"
+| "map_pair f (kv # xs) =
+    (let (k, v) = f kv; aux = map_pair f xs in if v = 0 then aux else (k, v) # aux)"
+
+text \<open>The difference between @{const List.map} and @{const map_pair} is that the latter removes
+  @{term 0} values, whereas the former does not.\<close>
+
+abbreviation map_val_pair :: "('a \<Rightarrow> 'b \<Rightarrow> 'c) \<Rightarrow> ('a \<times> 'b::zero) list \<Rightarrow> ('a \<times> 'c::zero) list"
+  where "map_val_pair f \<equiv> map_pair (\<lambda>(k, v). (k, f k v))"
+
+fun map2_val_pair :: "('a \<Rightarrow> 'b \<Rightarrow> 'c \<Rightarrow> 'd) \<Rightarrow> ('a key_order \<Rightarrow> ('a \<times> 'b) list \<Rightarrow> ('a \<times> 'd) list) \<Rightarrow> ('a key_order \<Rightarrow> ('a \<times> 'c) list \<Rightarrow> ('a \<times> 'd) list) \<Rightarrow>
+                     ('a \<times> 'b::zero) list \<Rightarrow> ('a \<times> 'c::zero) list \<Rightarrow> ('a \<times> 'd::zero) list"
+where
+  "map2_val_pair f g h xs [] = g ko xs"
+| "map2_val_pair f g h [] ys = h ko ys"
+| "map2_val_pair f g h ((kx, vx) # xs) ((ky, vy) # ys) =
+    (case key_compare ko kx ky of
+             Lt    \<Rightarrow> (let v = f kx vx 0; aux = map2_val_pair f g h xs ((ky, vy) # ys) in if v = 0 then aux else (kx, v) # aux)
+           | Eq   \<Rightarrow> (let v = f kx vx vy; aux = map2_val_pair f g h xs ys in if v = 0 then aux else (kx, v) # aux)
+           | Gt \<Rightarrow> (let v = f ky 0 vy; aux = map2_val_pair f g h ((kx, vx) # xs) ys in if v = 0 then aux else (ky, v) # aux))"
+
+fun lex_ord_pair :: "('a \<Rightarrow> (('b, 'c) comp_opt)) \<Rightarrow> (('a \<times> 'b::zero) list, ('a \<times> 'c::zero) list) comp_opt"
+where
+  "lex_ord_pair f []       []       = Some Eq"|
+  "lex_ord_pair f []       ((ky, vy) # ys) =
+    (let aux = f ky 0 vy in if aux = Some Eq then lex_ord_pair f [] ys else aux)"|
+  "lex_ord_pair f ((kx, vx) # xs) []       =
+    (let aux = f kx vx 0 in if aux = Some Eq then lex_ord_pair f xs [] else aux)"|
+  "lex_ord_pair f ((kx, vx) # xs) ((ky, vy) # ys) =
+    (case key_compare ko kx ky of
+             Lt    \<Rightarrow> (let aux = f kx vx 0 in if aux = Some Eq then lex_ord_pair f xs ((ky, vy) # ys) else aux)
+           | Eq   \<Rightarrow> (let aux = f kx vx vy in if aux = Some Eq then lex_ord_pair f xs ys else aux)
+           | Gt \<Rightarrow> (let aux = f ky 0 vy in if aux = Some Eq then lex_ord_pair f ((kx, vx) # xs) ys else aux))"
+
+fun prod_ord_pair :: "('a \<Rightarrow> 'b \<Rightarrow> 'c \<Rightarrow> bool) \<Rightarrow> ('a \<times> 'b::zero) list \<Rightarrow> ('a \<times> 'c::zero) list \<Rightarrow> bool"
+where
+  "prod_ord_pair f []       []       = True"|
+  "prod_ord_pair f []       ((ky, vy) # ys) = (f ky 0 vy \<and> prod_ord_pair f [] ys)"|
+  "prod_ord_pair f ((kx, vx) # xs) []       = (f kx vx 0 \<and> prod_ord_pair f xs [])"|
+  "prod_ord_pair f ((kx, vx) # xs) ((ky, vy) # ys) =
+    (case key_compare ko kx ky of
+             Lt    \<Rightarrow> (f kx vx 0 \<and> prod_ord_pair f xs ((ky, vy) # ys))
+           | Eq   \<Rightarrow> (f kx vx vy \<and> prod_ord_pair f xs ys)
+           | Gt \<Rightarrow> (f ky 0 vy \<and> prod_ord_pair f ((kx, vx) # xs) ys))"
+
+text \<open>@{const prod_ord_pair} is actually just a special case of @{const lex_ord_pair}, as proved below
+  in lemma ``prod_ord_pair_eq_lex_ord_pair''.\<close>
+
+subsubsection \<open>@{const lookup_pair}\<close>
+
+lemma lookup_pair_eq_0:
+  assumes "oalist_inv (xs, ko)"
+  shows "lookup_pair xs k = 0 \<longleftrightarrow> (k \<notin> fst ` set xs)"
+  using assms
+proof (induct xs rule: oalist_inv_induct)
+  case Nil
+  show ?case by simp
+next
+  case (Cons k' v' xs)
+  show ?case
+  proof (simp add: Cons(3) key_compare_Eq split: order.splits, rule, simp_all only: atomize_imp[symmetric])
+    assume "key_compare ko k k' = Lt"
+    hence "k \<noteq> k'" by auto
+    moreover have "k \<notin> fst ` set xs"
+    proof
+      assume "k \<in> fst ` set xs"
+      hence "lt_of_key_order ko k' k" by (rule Cons(4))
+      with \<open>key_compare ko k k' = Lt\<close> show False by (simp add: lt_of_key_order_alt[symmetric])
+    qed
+    ultimately show "k \<noteq> k' \<and> k \<notin> fst ` set xs" ..
+  next
+    assume "key_compare ko k k' = Gt"
+    hence "k \<noteq> k'" by auto
+    thus "(local.lookup_pair xs k = 0) = (k \<noteq> k' \<and> k \<notin> fst ` set xs)" by (simp add: Cons(5))
+  qed
+qed
+
+lemma lookup_pair_eq_value:
+  assumes "oalist_inv (xs, ko)" and "v \<noteq> 0"
+  shows "lookup_pair xs k = v \<longleftrightarrow> ((k, v) \<in> set xs)"
+  using assms(1)
+proof (induct xs rule: oalist_inv_induct)
+  case Nil
+  from assms(2) show ?case by simp
+next
+  case (Cons k' v' xs)
+  have *: "(k', u) \<notin> set xs" for u
+  proof
+    assume "(k', u) \<in> set xs"
+    hence "fst (k', u) \<in> fst ` set xs" by fastforce
+    hence "k' \<in> fst ` set xs" by simp
+    hence "lt_of_key_order ko k' k'" by (rule Cons(4))
+    thus False by (simp add: lt_of_key_order_alt[symmetric])
+  qed
+  show ?case
+  proof (simp add: assms(2) Cons(5) key_compare_Eq split: order.split, intro conjI impI)
+    assume "key_compare ko k k' = Lt"
+    show "(k, v) \<notin> set xs"
+    proof
+      assume "(k, v) \<in> set xs"
+      hence "fst (k, v) \<in> fst ` set xs" by fastforce
+      hence "k \<in> fst ` set xs" by simp
+      hence "lt_of_key_order ko k' k" by (rule Cons(4))
+      with \<open>key_compare ko k k' = Lt\<close> show False by (simp add: lt_of_key_order_alt[symmetric])
+    qed
+  qed (auto simp: *)
+qed
+
+lemma lookup_pair_eq_valueI:
+  assumes "oalist_inv (xs, ko)" and "(k, v) \<in> set xs"
+  shows "lookup_pair xs k = v"
+proof -
+  from assms(2) have "v \<in> snd ` set xs" by force
+  moreover from assms(1) have "0 \<notin> snd ` set xs" by (rule oalist_invD1)
+  ultimately have "v \<noteq> 0" by blast
+  with assms show ?thesis by (simp add: lookup_pair_eq_value)
+qed
+
+lemma lookup_pair_inj:
+  assumes "oalist_inv (xs, ko)" and "oalist_inv (ys, ko)" and "lookup_pair xs = lookup_pair ys"
+  shows "xs = ys"
+  using assms
+proof (induct xs arbitrary: ys rule: oalist_inv_induct)
+  case Nil
+  thus ?case
+  proof (induct ys rule: oalist_inv_induct)
+    case Nil
+    show ?case by simp
+  next
+    case (Cons k' v' ys)
+    have "v' = lookup_pair ((k', v') # ys) k'" by simp
+    also have "... = lookup_pair [] k'" by (simp only: Cons(6))
+    also have "... = 0" by simp
+    finally have "v' = 0" .
+    with Cons(3) show ?case ..
+  qed
+next
+  case *: (Cons k v xs)
+  from *(6, 7) show ?case
+  proof (induct ys rule: oalist_inv_induct)
+    case Nil
+    have "v = lookup_pair ((k, v) # xs) k" by simp
+    also have "... = lookup_pair [] k" by (simp only: Nil)
+    also have "... = 0" by simp
+    finally have "v = 0" .
+    with *(3) show ?case ..
+  next
+    case (Cons k' v' ys)
+    show ?case
+    proof (cases "key_compare ko k k'")
+      case Lt
+      hence "\<not> lt_of_key_order ko k' k" by (simp add: lt_of_key_order_alt[symmetric])
+      with Cons(4) have "k \<notin> fst ` set ys" by blast
+      moreover from Lt have "k \<noteq> k'" by auto
+      ultimately have "k \<notin> fst ` set ((k', v') # ys)" by simp
+      hence "0 = lookup_pair ((k', v') # ys) k"
+        by (simp add: lookup_pair_eq_0[OF Cons(1)] del: lookup_pair.simps)
+      also have "... = lookup_pair ((k, v) # xs) k" by (simp only: Cons(6))
+      also have "... = v" by simp
+      finally have "v = 0" by simp
+      with *(3) show ?thesis ..
+    next
+      case Eq
+      hence "k' = k" by (simp only: key_compare_Eq)
+      have "v' = lookup_pair ((k', v') # ys) k'" by simp
+      also have "... = lookup_pair ((k, v) # xs) k" by (simp only: Cons(6) \<open>k' = k\<close>)
+      also have "... = v" by simp
+      finally have "v' = v" .
+      moreover note \<open>k' = k\<close>
+      moreover from Cons(2) have "xs = ys"
+      proof (rule *(5))
+        show "lookup_pair xs = lookup_pair ys"
+        proof
+          fix k0
+          show "lookup_pair xs k0 = lookup_pair ys k0"
+          proof (cases "lt_of_key_order ko k k0")
+            case True
+            hence eq: "key_compare ko k0 k = Gt"
+              by (simp add: key_compare_Gt lt_of_key_order_alt)
+            have "lookup_pair xs k0 = lookup_pair ((k, v) # xs) k0" by (simp add: eq)
+            also have "... = lookup_pair ((k, v') # ys) k0" by (simp only: Cons(6) \<open>k' = k\<close>)
+            also have "... = lookup_pair ys k0" by (simp add: eq)
+            finally show ?thesis .
+          next
+            case False
+            with *(4) have "k0 \<notin> fst ` set xs" by blast
+            with *(2) have eq: "lookup_pair xs k0 = 0" by (simp add: lookup_pair_eq_0)
+            from False Cons(4) have "k0 \<notin> fst ` set ys" unfolding \<open>k' = k\<close> by blast
+            with Cons(2) have "lookup_pair ys k0 = 0" by (simp add: lookup_pair_eq_0)
+            with eq show ?thesis by simp
+          qed
+        qed
+      qed
+      ultimately show ?thesis by simp
+    next
+      case Gt
+      hence "\<not> lt_of_key_order ko k k'" by (simp add: key_compare_Gt lt_of_key_order_alt[symmetric])
+      with *(4) have "k' \<notin> fst ` set xs" by blast
+      moreover from Gt have "k' \<noteq> k" by auto
+      ultimately have "k' \<notin> fst ` set ((k, v) # xs)" by simp
+      hence "0 = lookup_pair ((k, v) # xs) k'"
+        by (simp add: lookup_pair_eq_0[OF *(1)] del: lookup_pair.simps)
+      also have "... = lookup_pair ((k', v') # ys) k'" by (simp only: Cons(6))
+      also have "... = v'" by simp
+      finally have "v' = 0" by simp
+      with Cons(3) show ?thesis ..
+    qed
+  qed
+qed
+
+lemma lookup_pair_tl:
+  assumes "oalist_inv (xs, ko)"
+  shows "lookup_pair (tl xs) k =
+          (if (\<forall>k'\<in>fst ` set xs. le_of_key_order ko k k') then 0 else lookup_pair xs k)"
+proof -
+  from assms have 1: "oalist_inv (tl xs, ko)" by (rule oalist_inv_tl)
+  show ?thesis
+  proof (split if_split, intro conjI impI)
+    assume *: "\<forall>x\<in>fst ` set xs. le_of_key_order ko k x"
+    show "lookup_pair (tl xs) k = 0"
+    proof (simp add: lookup_pair_eq_0[OF 1], rule)
+      assume k_in: "k \<in> fst ` set (tl xs)"
+      hence "xs \<noteq> []" by auto
+      then obtain k' v' ys where xs: "xs = (k', v') # ys" using prod.exhaust list.exhaust by metis
+      have "k' \<in> fst ` set xs" unfolding xs by fastforce
+      with * have "le_of_key_order ko k k'" ..
+      from assms have "oalist_inv ((k', v') # ys, ko)" by (simp only: xs)
+      moreover from k_in have "k \<in> fst ` set ys" by (simp add: xs)
+      ultimately have "lt_of_key_order ko k' k" by (rule oalist_inv_ConsD3)
+      with \<open>le_of_key_order ko k k'\<close> show False by simp
+    qed
+  next
+    assume "\<not> (\<forall>k'\<in>fst ` set xs. le_of_key_order ko k k')"
+    hence "\<exists>x\<in>fst ` set xs. \<not> le_of_key_order ko k x" by simp
+    then obtain k'' where k''_in: "k'' \<in> fst ` set xs" and "\<not> le_of_key_order ko k k''" ..
+    from this(2) have "lt_of_key_order ko k'' k" by simp
+    from k''_in have "xs \<noteq> []" by auto
+    then obtain k' v' ys where xs: "xs = (k', v') # ys" using prod.exhaust list.exhaust by metis
+    from k''_in have "k'' = k' \<or> k'' \<in> fst ` set ys" by (simp add: xs)
+    hence "lt_of_key_order ko k' k"
+    proof
+      assume "k'' = k'"
+      with \<open>lt_of_key_order ko k'' k\<close> show ?thesis by simp
+    next
+      from assms have "oalist_inv ((k', v') # ys, ko)" by (simp only: xs)
+      moreover assume "k'' \<in> fst ` set ys"
+      ultimately have "lt_of_key_order ko k' k''" by (rule oalist_inv_ConsD3)
+      thus ?thesis using \<open>lt_of_key_order ko k'' k\<close> by (rule key_order_lin.less_trans)
+    qed
+    hence "key_compare ko k k' = Gt" by (simp add: key_compare_Gt lt_of_key_order_alt)
+    thus "lookup_pair (tl xs) k = lookup_pair xs k" by (simp add: xs lt_of_key_order_alt)
+  qed
+qed
+
+lemma lookup_pair_filter:
+  assumes "oalist_inv (xs, ko)"
+  shows "lookup_pair (filter P xs) k = (let v = lookup_pair xs k in if P (k, v) then v else 0)"
+  using assms
+proof (induct xs rule: oalist_inv_induct)
+  case Nil
+  show ?case by simp
+next
+  case (Cons k' v' xs)
+  show ?case
+  proof (simp add: Cons(5) Let_def key_compare_Eq split: order.split, intro conjI impI)
+    show "lookup_pair xs k' = 0"
+    proof (simp add: lookup_pair_eq_0 Cons(2), rule)
+      assume "k' \<in> fst ` set xs"
+      hence "lt_of_key_order ko k' k'" by (rule Cons(4))
+      thus False by simp
+    qed
+  next
+    assume "key_compare ko k k' = Lt"
+    hence "lt_of_key_order ko k k'" by (simp only: lt_of_key_order_alt)
+    show "lookup_pair xs k = 0"
+    proof (simp add: lookup_pair_eq_0 Cons(2), rule)
+      assume "k \<in> fst ` set xs"
+      hence "lt_of_key_order ko k' k" by (rule Cons(4))
+      with \<open>lt_of_key_order ko k k'\<close> show False by simp
+    qed
+  qed
+qed
+
+lemma lookup_pair_map:
+  assumes "oalist_inv (xs, ko)"
+    and "\<And>k'. snd (f (k', 0)) = 0"
+    and "\<And>a b. key_compare ko (fst (f a)) (fst (f b)) = key_compare ko (fst a) (fst b)"
+  shows "lookup_pair (map f xs) (fst (f (k, v))) = snd (f (k, lookup_pair xs k))"
+  using assms(1)
+proof (induct xs rule: oalist_inv_induct)
+  case Nil
+  show ?case by (simp add: assms(2))
+next
+  case (Cons k' v' xs)
+  obtain k'' v'' where f: "f (k', v') = (k'', v'')" by fastforce
+  have "key_compare ko k k' = key_compare ko (fst (f (k, v))) (fst (f (k', v')))"
+    by (simp add: assms(3))
+  also have "... = key_compare ko (fst (f (k, v))) k''" by (simp add: f)
+  finally have eq: "key_compare ko k k' = key_compare ko (fst (f (k, v))) k''" .
+  show ?case
+  proof (simp add: assms(2) split: order.split, intro conjI impI, simp add: key_compare_Eq)
+    assume "k = k'"
+    hence "lookup_pair (f (k', v') # map f xs) (fst (f (k', v))) =
+            lookup_pair (f (k', v') # map f xs) (fst (f (k, v)))" by simp
+    also have "... = snd (f (k', v'))" by (simp add: f eq[symmetric], simp add: \<open>k = k'\<close>)
+    finally show "lookup_pair (f (k', v') # map f xs) (fst (f (k', v))) = snd (f (k', v'))" .
+  qed (simp_all add: f eq Cons(5))
+qed
+
+lemma lookup_pair_Cons:
+  assumes "oalist_inv ((k, v) # xs, ko)"
+  shows "lookup_pair ((k, v) # xs) k0 = (if k = k0 then v else lookup_pair xs k0)"
+proof (simp add: key_compare_Eq split: order.split, intro impI)
+  assume "key_compare ko k0 k = Lt"
+  from assms have inv: "oalist_inv (xs, ko)" by (rule oalist_inv_ConsD1)
+  show "lookup_pair xs k0 = 0"
+  proof (simp only: lookup_pair_eq_0[OF inv], rule)
+    assume "k0 \<in> fst ` set xs"
+    with assms have "lt_of_key_order ko k k0" by (rule oalist_inv_ConsD3)
+    with \<open>key_compare ko k0 k = Lt\<close> show False by (simp add: lt_of_key_order_alt[symmetric])
+  qed
+qed
+
+subsubsection \<open>@{const update_by_pair}\<close>
+
+lemma set_update_by_pair_subset: "set (update_by_pair kv xs) \<subseteq> insert kv (set xs)"
 proof (induct xs arbitrary: kv)
   case Nil
   obtain k v where kv: "kv = (k, v)" by fastforce
@@ -171,14 +804,14 @@ next
   obtain k' v' where x: "x = (k', v')" by fastforce
   obtain k v where kv: "kv = (k, v)" by fastforce
   have 1: "set xs \<subseteq> insert a (insert b (set xs))" for a b by auto
-  have 2: "set (update_by' kv xs) \<subseteq> insert kv (insert (k', v') (set xs))" for kv
+  have 2: "set (update_by_pair kv xs) \<subseteq> insert kv (insert (k', v') (set xs))" for kv
     using Cons by blast
-  show ?case by (simp add: x kv 1 2 split: comparison.split)
+  show ?case by (simp add: x kv 1 2 split: order.split)
 qed
 
-lemma update_by'_sorted:
-  assumes "sorted_wrt less_of_comp (map fst xs)"
-  shows "sorted_wrt less_of_comp (map fst (update_by' kv xs))"
+lemma update_by_pair_sorted:
+  assumes "sorted_wrt (lt_of_key_order ko) (map fst xs)"
+  shows "sorted_wrt (lt_of_key_order ko) (map fst (update_by_pair kv xs))"
   using assms
 proof (induct xs arbitrary: kv)
   case Nil
@@ -188,37 +821,36 @@ next
   case (Cons x xs)
   obtain k' v' where x: "x = (k', v')" by fastforce
   obtain k v where kv: "kv = (k, v)" by fastforce
-  from Cons(2) have 1: "sorted_wrt less_of_comp (k' # (map fst xs))" by (simp add: x)
-  hence 2: "sorted_wrt less_of_comp (map fst xs)" using sorted_wrt.elims(3) by fastforce
-  hence 3: "sorted_wrt less_of_comp (map fst (update_by' (k, u) xs))" for u by (rule Cons(1))
-  have 4: "sorted_wrt less_of_comp (k' # map fst (update_by' (k, u) xs))"
-    if *: "compare_class.compare k k' = GREATER" for u
+  from Cons(2) have 1: "sorted_wrt (lt_of_key_order ko) (k' # (map fst xs))" by (simp add: x)
+  hence 2: "sorted_wrt (lt_of_key_order ko) (map fst xs)" using sorted_wrt.elims(3) by fastforce
+  hence 3: "sorted_wrt (lt_of_key_order ko) (map fst (update_by_pair (k, u) xs))" for u by (rule Cons(1))
+  have 4: "sorted_wrt (lt_of_key_order ko) (k' # map fst (update_by_pair (k, u) xs))"
+    if *: "key_compare ko k k' = Gt" for u
   proof (simp, intro conjI ballI)
     fix y
-    assume "y \<in> set (update_by' (k, u) xs)"
-    also from set_update_by'_subset have "... \<subseteq> insert (k, u) (set xs)" .
+    assume "y \<in> set (update_by_pair (k, u) xs)"
+    also from set_update_by_pair_subset have "... \<subseteq> insert (k, u) (set xs)" .
     finally have "y = (k, u) \<or> y \<in> set xs" by simp
-    thus "less_of_comp k' (fst y)"
+    thus "lt_of_key_order ko k' (fst y)"
     proof
       assume "y = (k, u)"
       hence "fst y = k" by simp
-      from * show ?thesis unfolding \<open>fst y = k\<close>
-        by (meson c.less_of_comparator_def compare_greater)
+      with * show ?thesis by (simp only: lt_of_key_order_alt key_compare_Gt)
     next
-      from 1 have 5: "\<forall>y \<in> fst ` set xs. less_of_comp k' y" by simp
+      from 1 have 5: "\<forall>y \<in> fst ` set xs. lt_of_key_order ko k' y" by simp
       assume "y \<in> set xs"
       hence "fst y \<in> fst ` set xs" by simp
       with 5 show ?thesis ..
     qed
   qed (fact 3)
   show ?case
-    by (simp add: kv x 1 2 4 sorted_wrt2[OF transp_less_of_comp] split: comparison.split del: sorted_wrt.simps, intro conjI impI,
-        simp add: less_of_comp_alt, simp add: 1 compare_equal del: sorted_wrt.simps)
+    by (simp add: kv x 1 2 4 sorted_wrt2[OF key_order_lin.transp_less] split: order.split del: sorted_wrt.simps,
+        intro conjI impI, simp add: 1 key_compare_Eq del: sorted_wrt.simps, simp add: lt_of_key_order_alt)
 qed
 
-lemma update_by'_not_zero:
+lemma update_by_pair_not_0:
   assumes "0 \<notin> snd ` set xs"
-  shows "0 \<notin> snd ` set (update_by' kv xs)"
+  shows "0 \<notin> snd ` set (update_by_pair kv xs)"
   using assms
 proof (induct xs arbitrary: kv)
   case Nil
@@ -228,14 +860,25 @@ next
   case (Cons x xs)
   obtain k' v' where x: "x = (k', v')" by fastforce
   obtain k v where kv: "kv = (k, v)" by fastforce
-  from Cons(2) have 1: "v' \<noteq> 0" and 2: "0 \<notin> snd ` set xs" by (simp add: x, simp)
-  from 2 have 3: "0 \<notin> snd ` set (update_by' (k, u) xs)" for u by (rule Cons(1))
-  show ?case by (simp add: kv x 1 2 3 split: comparison.split)
+  from Cons(2) have 1: "v' \<noteq> 0" and 2: "0 \<notin> snd ` set xs" by (auto simp: x)
+  from 2 have 3: "0 \<notin> snd ` set (update_by_pair (k, u) xs)" for u by (rule Cons(1))
+  show ?case by (auto simp: kv x 1 2 3 split: order.split)
 qed
 
-lemma update_by'_eq_Cons:
-  assumes "v \<noteq> 0" and "xs = [] \<or> compare k (fst (hd xs)) = LESS"
-  shows "update_by' (k, v) xs = (k, v) # xs"
+corollary oalist_inv_update_by_pair:
+  assumes "oalist_inv (xs, ko)"
+  shows "oalist_inv (update_by_pair kv xs, ko)"
+proof (rule oalist_invI)
+  from assms have "0 \<notin> snd ` set xs" by (rule oalist_invD1)
+  thus "0 \<notin> snd ` set (update_by_pair kv xs)" by (rule update_by_pair_not_0)
+next
+  from assms have "sorted_wrt (lt_of_key_order ko) (map fst xs)" by (rule oalist_invD2)
+  thus "sorted_wrt (lt_of_key_order ko) (map fst (update_by_pair kv xs))" by (rule update_by_pair_sorted)
+qed
+
+lemma update_by_pair_less:
+  assumes "v \<noteq> 0" and "xs = [] \<or> key_compare ko k (fst (hd xs)) = Lt"
+  shows "update_by_pair (k, v) xs = (k, v) # xs"
   using assms(2)
 proof (induct xs)
 case Nil
@@ -243,168 +886,2019 @@ case Nil
 next
   case (Cons x xs)
   obtain k' v' where x: "x = (k', v')" by fastforce
-  from Cons(2) have "compare_class.compare k k' = LESS" by (simp add: x)
+  from Cons(2) have "key_compare ko k k' = Lt" by (simp add: x)
   with assms(1) show ?case by (simp add: x)
 qed
 
-lemma update_by_fun_gr_raw_eq_update_by_fun_raw:
-  assumes "sorted_wrt less_of_comp (map fst xs)"
-  shows "update_by_fun_gr_raw k f xs = update_by_fun_raw k f xs"
-  sorry
+lemma lookup_pair_update_by_pair:
+  assumes "oalist_inv (xs, ko)"
+  shows "lookup_pair (update_by_pair (k1, v) xs) k2 = (if k1 = k2 then v else lookup_pair xs k2)"
+  using assms
+proof (induct xs arbitrary: v rule: oalist_inv_induct)
+  case Nil
+  show ?case by (simp split: order.split, simp add: key_compare_Eq)
+next
+  case (Cons k' v' xs)
+  show ?case
+  proof (split if_split, intro conjI impI)
+    assume "k1 = k2"
+    with Cons(5) have eq: "lookup_pair (update_by_pair (k2, u) xs) k2 = u" for u
+      by (simp del: update_by_pair.simps)
+    show "lookup_pair (update_by_pair (k1, v) ((k', v') # xs)) k2 = v"
+    proof (simp add: \<open>k1 = k2\<close> eq split: order.split, intro conjI impI)
+      assume "key_compare ko k2 k' = Eq"
+      hence "\<not> lt_of_key_order ko k' k2" by (simp add: lt_of_key_order_alt key_compare_Eq)
+      with Cons(4) have "k2 \<notin> fst ` set xs" by auto
+      thus "lookup_pair xs k2 = 0" using Cons(2) by (simp add: lookup_pair_eq_0)
+    qed
+  next
+    assume "k1 \<noteq> k2"
+    with Cons(5) have eq: "lookup_pair (update_by_pair (k1, u) xs) k2 = lookup_pair xs k2" for u
+      by (simp del: update_by_pair.simps)
+    have *: "lookup_pair xs k2 = 0" if "lt_of_key_order ko k2 k'"
+    proof -
+      from \<open>lt_of_key_order ko k2 k'\<close> have "\<not> lt_of_key_order ko k' k2" by auto
+      with Cons(4) have "k2 \<notin> fst ` set xs" by auto
+      thus "lookup_pair xs k2 = 0" using Cons(2) by (simp add: lookup_pair_eq_0)
+    qed
+    show "lookup_pair (update_by_pair (k1, v) ((k', v') # xs)) k2 = lookup_pair ((k', v') # xs) k2"
+      by (simp add: \<open>k1 \<noteq> k2\<close> eq split: order.split,
+          auto intro: * simp: \<open>k1 \<noteq> k2\<close>[symmetric] key_compare_Eq key_compare_Gt lt_of_key_order_alt[symmetric])
+  qed
+qed
 
-lemma map2_val_rneutr_raw_singleton_eq_update_by_fun_raw:
-  assumes "\<And>a x. f a x 0 = x"
-  shows "map2_val_rneutr_raw f xs [(k, v)] = update_by_fun_raw k (\<lambda>x. f k x v) xs"
-  sorry
+corollary update_by_pair_id:
+  assumes "oalist_inv (xs, ko)" and "lookup_pair xs k = v"
+  shows "update_by_pair (k, v) xs = xs"
+proof (rule lookup_pair_inj, rule oalist_inv_update_by_pair)
+  show "lookup_pair (update_by_pair (k, v) xs) = lookup_pair xs"
+  proof
+    fix k0
+    from assms(2) show "lookup_pair (update_by_pair (k, v) xs) k0 = lookup_pair xs k0"
+      by (auto simp: lookup_pair_update_by_pair[OF assms(1)])
+  qed
+qed fact+
 
-lemma map2_val_rneutr_raw_eq_map2_val_neutr_raw:
-  assumes "\<And>a x. f a x 0 = x" and "\<And>a. f a 0 = id"
-  shows "map2_val_rneutr_raw f = map2_val_neutr_raw f"
-  sorry
+lemma set_update_by_pair:
+  assumes "oalist_inv (xs, ko)" and "v \<noteq> 0"
+  shows "set (update_by_pair (k, v) xs) = insert (k, v) (set xs - range (Pair k))" (is "?A = ?B")
+proof (rule set_eqI)
+  fix x::"'a \<times> 'b"
+  obtain k' v' where x: "x = (k', v')" by fastforce
+  from assms(1) have inv: "oalist_inv (update_by_pair (k, v) xs, ko)" by (rule oalist_inv_update_by_pair)
+  show "(x \<in> ?A) \<longleftrightarrow> (x \<in> ?B)"
+  proof (cases "v' = 0")
+    case True
+    have "0 \<notin> snd ` set (update_by_pair (k, v) xs)" and "0 \<notin> snd ` set xs"
+      by (rule oalist_invD1, fact)+
+    hence "(k', 0) \<notin> set (update_by_pair (k, v) xs)" and "(k', 0) \<notin> set xs"
+      using image_iff by fastforce+
+    thus ?thesis by (simp add: x True assms(2))
+  next
+    case False
+    show ?thesis
+      by (auto simp: x lookup_pair_eq_value[OF inv False, symmetric] lookup_pair_eq_value[OF assms(1) False]
+          lookup_pair_update_by_pair[OF assms(1)])
+  qed
+qed
+
+subsubsection \<open>@{const update_by_fun_pair} and @{const update_by_fun_gr_pair}\<close>
+
+lemma update_by_fun_pair_eq_update_by_pair:
+  assumes "oalist_inv (xs, ko)"
+  shows "update_by_fun_pair k f xs = update_by_pair (k, f (lookup_pair xs k)) xs"
+  using assms by (induct xs rule: oalist_inv_induct, simp, simp split: order.split)
+
+corollary oalist_inv_update_by_fun_pair:
+  assumes "oalist_inv (xs, ko)"
+  shows "oalist_inv (update_by_fun_pair k f xs, ko)"
+  unfolding update_by_fun_pair_eq_update_by_pair[OF assms] using assms by (rule oalist_inv_update_by_pair)
+
+corollary lookup_pair_update_by_fun_pair:
+  assumes "oalist_inv (xs, ko)"
+  shows "lookup_pair (update_by_fun_pair k1 f xs) k2 = (if k1 = k2 then f else id) (lookup_pair xs k2)"
+  by (simp add: update_by_fun_pair_eq_update_by_pair[OF assms] lookup_pair_update_by_pair[OF assms])
+
+lemma update_by_fun_pair_gr:
+  assumes "oalist_inv (xs, ko)" and "xs = [] \<or> key_compare ko k (fst (last xs)) = Gt"
+  shows "update_by_fun_pair k f xs = xs @ (if f 0 = 0 then [] else [(k, f 0)])"
+  using assms
+proof (induct xs rule: oalist_inv_induct)
+  case Nil
+  show ?case by simp
+next
+  case (Cons k' v' xs)
+  from Cons(6) have 1: "key_compare ko k (fst (last ((k', v') # xs))) = Gt" by simp
+  have eq1: "key_compare ko k k' = Gt"
+  proof (cases "xs = []")
+    case True
+    with 1 show ?thesis by simp
+  next
+    case False
+    have "lt_of_key_order ko k' (fst (last xs))" by (rule Cons(4), simp add: False)
+    from False 1 have "key_compare ko k (fst (last xs)) = Gt" by simp
+    moreover from \<open>lt_of_key_order ko k' (fst (last xs))\<close> have "key_compare ko (fst (last xs)) k' = Gt"
+      by (simp add: key_compare_Gt lt_of_key_order_alt)
+    ultimately show ?thesis
+      by (meson key_compare_Gt key_order_lin.less_trans lt_of_key_order_alt)
+  qed
+  have eq2: "update_by_fun_pair k f xs = xs @ (if f 0 = 0 then [] else [(k, f 0)])"
+  proof (rule Cons(5), simp only: disj_commute[of "xs = []"], rule disjCI)
+    assume "xs \<noteq> []"
+    with 1 show "key_compare ko k (fst (last xs)) = Gt" by simp
+  qed
+  show ?case by (simp split: order.split add: Let_def eq1 eq2)
+qed
+
+corollary update_by_fun_gr_pair_eq_update_by_fun_pair:
+  assumes "oalist_inv (xs, ko)"
+  shows "update_by_fun_gr_pair k f xs = update_by_fun_pair k f xs"
+  by (simp add: update_by_fun_gr_pair_def Let_def update_by_fun_pair_gr[OF assms] split: order.split)
+
+corollary oalist_inv_update_by_fun_gr_pair:
+  assumes "oalist_inv (xs, ko)"
+  shows "oalist_inv (update_by_fun_gr_pair k f xs, ko)"
+  unfolding update_by_fun_pair_eq_update_by_pair[OF assms] update_by_fun_gr_pair_eq_update_by_fun_pair[OF assms]
+  using assms by (rule oalist_inv_update_by_pair)
+
+corollary lookup_pair_update_by_fun_gr_pair:
+  assumes "oalist_inv (xs, ko)"
+  shows "lookup_pair (update_by_fun_gr_pair k1 f xs) k2 = (if k1 = k2 then f else id) (lookup_pair xs k2)"
+  by (simp add: update_by_fun_pair_eq_update_by_pair[OF assms]
+      update_by_fun_gr_pair_eq_update_by_fun_pair[OF assms] lookup_pair_update_by_pair[OF assms])
+
+subsubsection \<open>@{const map_pair}\<close>
+
+lemma map_pair_subset: "set (map_pair f xs) \<subseteq> f ` set xs"
+proof (induct xs rule: map_pair.induct)
+  case (1 f)
+  show ?case by simp
+next
+  case (2 f kv xs)
+  obtain k v where f: "f kv = (k, v)" by fastforce
+  from f[symmetric] refl have *: "set (map_pair f xs) \<subseteq> f ` set xs" by (rule 2)
+  show ?case by (simp add: f Let_def, intro conjI impI subset_insertI2 *)
+qed
+
+lemma oalist_inv_map_pair:
+  assumes "oalist_inv (xs, ko)"
+    and "\<And>a b. key_compare ko (fst (f a)) (fst (f b)) = key_compare ko (fst a) (fst b)"
+  shows "oalist_inv (map_pair f xs, ko)"
+  using assms(1)
+proof (induct xs rule: oalist_inv_induct)
+  case Nil
+  from oalist_inv_Nil show ?case by simp
+next
+  case (Cons k v xs)
+  obtain k' v' where f: "f (k, v) = (k', v')" by fastforce
+  show ?case
+  proof (simp add: f Let_def Cons(5), rule)
+    assume "v' \<noteq> 0"
+    with Cons(5) show "oalist_inv ((k', v') # map_pair f xs, ko)"
+    proof (rule oalist_inv_ConsI)
+      assume "map_pair f xs \<noteq> []"
+      hence "hd (map_pair f xs) \<in> set (map_pair f xs)" by simp
+      also have "... \<subseteq> f ` set xs" by (fact map_pair_subset)
+      finally obtain x where "x \<in> set xs" and eq: "hd (map_pair f xs) = f x" ..
+      from this(1) have "fst x \<in> fst ` set xs" by fastforce
+      hence "lt_of_key_order ko k (fst x)" by (rule Cons(4))
+      hence "lt_of_key_order ko (fst (f (k, v))) (fst (f x))"
+        by (simp add: lt_of_key_order_alt assms(2))
+      thus "lt_of_key_order ko k' (fst (hd (map_pair f xs)))" by (simp add: f eq)
+    qed
+  qed
+qed
+
+lemma lookup_pair_map_pair:
+  assumes "oalist_inv (xs, ko)"
+    and "\<And>k'. snd (f (k', 0)) = 0"
+    and "\<And>a b. key_compare ko (fst (f a)) (fst (f b)) = key_compare ko (fst a) (fst b)"
+  shows "lookup_pair (map_pair f xs) (fst (f (k, v))) = snd (f (k, lookup_pair xs k))"
+  using assms(1)
+proof (induct xs rule: oalist_inv_induct)
+  case Nil
+  show ?case by (simp add: assms(2))
+next
+  case (Cons k' v' xs)
+  obtain k'' v'' where f: "f (k', v') = (k'', v'')" by fastforce
+  have "key_compare ko (fst (f (k, v))) k'' = key_compare ko (fst (f (k, v))) (fst (f (k', v')))"
+    by (simp add: f)
+  also have "... = key_compare ko k k'"
+    by (simp add: assms(3))
+  finally have eq: "key_compare ko (fst (f (k, v))) k'' = key_compare ko k k'" .
+  have *: "lookup_pair xs k = 0" if "key_compare ko k k' \<noteq> Gt"
+  proof (simp add: lookup_pair_eq_0[OF Cons(2)], rule)
+    assume "k \<in> fst ` set xs"
+    hence "lt_of_key_order ko k' k" by (rule Cons(4))
+    hence "key_compare ko k k' = Gt" by (simp add: key_compare_Gt lt_of_key_order_alt)
+    with \<open>key_compare ko k k' \<noteq> Gt\<close> show False ..
+  qed
+  show ?case
+  proof (simp add: assms(2) f Let_def eq Cons(5) split: order.split, intro conjI impI)
+    assume "key_compare ko k k' = Lt"
+    hence "key_compare ko k k' \<noteq> Gt" by simp
+    hence "lookup_pair xs k = 0" by (rule *)
+    thus "snd (f (k, lookup_pair xs k)) = 0" by (simp add: assms(2))
+  next
+    assume "v'' = 0"
+    assume "key_compare ko k k' = Eq"
+    hence "k = k'" and "key_compare ko k k' \<noteq> Gt" by (simp only: key_compare_Eq, simp)
+    from this(2) have "lookup_pair xs k = 0" by (rule *)
+    hence "snd (f (k, lookup_pair xs k)) = 0" by (simp add: assms(2))
+    also have "... = snd (f (k, v'))" by (simp add: \<open>k = k'\<close> f \<open>v'' = 0\<close>)
+    finally show "snd (f (k, lookup_pair xs k)) = snd (f (k, v'))" .
+  qed (simp add: f key_compare_Eq)
+qed
+
+lemma oalist_inv_map_val_pair:
+  assumes "oalist_inv (xs, ko)"
+  shows "oalist_inv (map_val_pair f xs, ko)"
+  by (rule oalist_inv_map_pair, fact assms, auto)
+
+lemma lookup_pair_map_val_pair:
+  assumes "oalist_inv (xs, ko)" and "\<And>k'. f k' 0 = 0"
+  shows "lookup_pair (map_val_pair f xs) k = f k (lookup_pair xs k)"
+proof -
+  let ?f = "\<lambda>(k', v'). (k', f k' v')"
+  have "lookup_pair (map_val_pair f xs) k = lookup_pair (map_val_pair f xs) (fst (?f (k, 0)))"
+    by simp
+  also have "... = snd (?f (k, local.lookup_pair xs k))"
+    by (rule lookup_pair_map_pair, fact assms(1), auto simp: assms(2))
+  also have "... = f k (lookup_pair xs k)" by simp
+  finally show ?thesis .
+qed
+
+subsubsection \<open>@{const map2_val_pair}\<close>
+
+definition map2_val_compat :: "('a key_order \<Rightarrow> ('a \<times> 'b::zero) list \<Rightarrow> ('a \<times> 'c::zero) list) \<Rightarrow> bool"
+  where "map2_val_compat f \<longleftrightarrow> (\<forall>zs. (oalist_inv (zs, ko) \<longrightarrow> (oalist_inv (f ko zs, ko) \<and> fst ` set (f ko zs) \<subseteq> fst ` set zs)))"
+
+lemma map2_val_compatI:
+  assumes "\<And>zs. oalist_inv (zs, ko) \<Longrightarrow> oalist_inv (f ko zs, ko)"
+    and "\<And>zs. oalist_inv (zs, ko) \<Longrightarrow> fst ` set (f ko zs) \<subseteq> fst ` set zs"
+  shows "map2_val_compat f"
+  unfolding map2_val_compat_def using assms by blast
+
+lemma map2_val_compatD1:
+  assumes "map2_val_compat f" and "oalist_inv (zs, ko)"
+  shows "oalist_inv (f ko zs, ko)"
+  using assms unfolding map2_val_compat_def by blast
+
+lemma map2_val_compatD2:
+  assumes "map2_val_compat f" and "oalist_inv (zs, ko)"
+  shows "fst ` set (f ko zs) \<subseteq> fst ` set zs"
+  using assms unfolding map2_val_compat_def by blast
+
+lemma map2_val_compat_Nil:
+  assumes "map2_val_compat (f::'a key_order \<Rightarrow> ('a \<times> 'b::zero) list \<Rightarrow> ('a \<times> 'c::zero) list)"
+  shows "f ko [] = []"
+proof -
+  from assms oalist_inv_Nil have "fst ` set (f ko []) \<subseteq> fst ` set ([]::('a \<times> 'b) list)"
+    by (rule map2_val_compatD2)
+  thus ?thesis by simp
+qed
+
+lemma fst_map2_val_pair_subset:
+  assumes "oalist_inv (xs, ko)" and "oalist_inv (ys, ko)"
+  assumes "map2_val_compat g" and "map2_val_compat h"
+  shows "fst ` set (map2_val_pair f g h xs ys) \<subseteq> fst ` set xs \<union> fst ` set ys"
+  using assms
+proof (induct f g h xs ys rule: map2_val_pair.induct)
+  case (1 f g h xs)
+  show ?case by (simp, rule map2_val_compatD2, fact+)
+next
+  case (2 f g h v va)
+  show ?case by (simp del: set_simps(2), rule map2_val_compatD2, fact+)
+next
+  case (3 f g h kx vx xs ky vy ys)
+  from 3(4) have "oalist_inv (xs, ko)" by (rule oalist_inv_ConsD1)
+  from 3(5) have "oalist_inv (ys, ko)" by (rule oalist_inv_ConsD1)
+  show ?case
+  proof (simp split: order.split, intro conjI impI)
+    assume "key_compare ko kx ky = Lt"
+    hence "fst ` set (map2_val_pair f g h xs ((ky, vy) # ys)) \<subseteq> fst ` set xs \<union> fst ` set ((ky, vy) # ys)"
+      using refl \<open>oalist_inv (xs, ko)\<close> 3(5, 6, 7) by (rule 3(2))
+    thus "fst ` set (let v = f kx vx 0; aux = map2_val_pair f g h xs ((ky, vy) # ys)
+                       in if v = 0 then aux else (kx, v) # aux)
+          \<subseteq> insert ky (insert kx (fst ` set xs \<union> fst ` set ys))" by (auto simp: Let_def)
+  next
+    assume "key_compare ko kx ky = Eq"
+    hence "fst ` set (map2_val_pair f g h xs ys) \<subseteq> fst ` set xs \<union> fst ` set ys"
+      using refl \<open>oalist_inv (xs, ko)\<close> \<open>oalist_inv (ys, ko)\<close> 3(6, 7) by (rule 3(1))
+    thus "fst ` set (let v = f kx vx vy; aux = map2_val_pair f g h xs ys in if v = 0 then aux else (kx, v) # aux)
+          \<subseteq> insert ky (insert kx (fst ` set xs \<union> fst ` set ys))" by (auto simp: Let_def)
+  next
+    assume "key_compare ko kx ky = Gt"
+    hence "fst ` set (map2_val_pair f g h ((kx, vx) # xs) ys) \<subseteq> fst ` set ((kx, vx) # xs) \<union> fst ` set ys"
+      using refl 3(4) \<open>oalist_inv (ys, ko)\<close> 3(6, 7) by (rule 3(3))
+    thus "fst ` set (let v = f ky 0 vy; aux = map2_val_pair f g h ((kx, vx) # xs) ys
+                        in if v = 0 then aux else (ky, v) # aux)
+          \<subseteq> insert ky (insert kx (fst ` set xs \<union> fst ` set ys))" by (auto simp: Let_def)
+  qed
+qed
+
+lemma oalist_inv_map2_val_pair:
+  assumes "oalist_inv (xs, ko)" and "oalist_inv (ys, ko)"
+  assumes "map2_val_compat g" and "map2_val_compat h"
+  shows "oalist_inv (map2_val_pair f g h xs ys, ko)"
+  using assms(1, 2)
+proof (induct xs arbitrary: ys rule: oalist_inv_induct)
+  case Nil
+  show ?case
+  proof (cases ys)
+    case Nil
+    show ?thesis by (simp add: Nil, rule map2_val_compatD1, fact assms(3), fact oalist_inv_Nil)
+  next
+    case (Cons y ys')
+    show ?thesis by (simp add: Cons, rule map2_val_compatD1, fact assms(4), simp only: Cons[symmetric], fact Nil)
+  qed
+next
+  case *: (Cons k v xs)
+  from *(6) show ?case
+  proof (induct ys rule: oalist_inv_induct)
+    case Nil
+    show ?case by (simp, rule map2_val_compatD1, fact assms(3), fact *(1))
+  next
+    case (Cons k' v' ys)
+    show ?case
+    proof (simp split: order.split, intro conjI impI)
+      assume "key_compare ko k k' = Lt"
+      hence 0: "lt_of_key_order ko k k'" by (simp only: lt_of_key_order_alt)
+      from Cons(1) have 1: "oalist_inv (map2_val_pair f g h xs ((k', v') # ys), ko)" by (rule *(5))
+      show "oalist_inv (let v = f k v 0; aux = map2_val_pair f g h xs ((k', v') # ys)
+              in if v = 0 then aux else (k, v) # aux, ko)"
+      proof (simp add: Let_def, intro conjI impI)
+        assume "f k v 0 \<noteq> 0"
+        with 1 show "oalist_inv ((k, f k v 0) # map2_val_pair f g h xs ((k', v') # ys), ko)"
+        proof (rule oalist_inv_ConsI)
+          define k0 where "k0 = fst (hd (local.map2_val_pair f g h xs ((k', v') # ys)))"
+          assume "map2_val_pair f g h xs ((k', v') # ys) \<noteq> []"
+          hence "k0 \<in> fst ` set (map2_val_pair f g h xs ((k', v') # ys))" by (simp add: k0_def)
+          also from *(2) Cons(1) assms(3, 4) have "... \<subseteq> fst ` set xs \<union> fst ` set ((k', v') # ys)"
+            by (rule fst_map2_val_pair_subset)
+          finally have "k0 \<in> fst ` set xs \<or> k0 = k' \<or> k0 \<in> fst ` set ys" by auto
+          thus "lt_of_key_order ko k k0"
+          proof (elim disjE)
+            assume "k0 = k'"
+            with 0 show ?thesis by simp
+          next
+            assume "k0 \<in> fst ` set ys"
+            hence "lt_of_key_order ko k' k0" by (rule Cons(4))
+            with 0 show ?thesis by (rule key_order_lin.less_trans)
+          qed (rule *(4))
+        qed
+      qed (rule 1)
+    next
+      assume "key_compare ko k k' = Eq"
+      hence "k = k'" by (simp only: key_compare_Eq)
+      from Cons(2) have 1: "oalist_inv (map2_val_pair f g h xs ys, ko)" by (rule *(5))
+      show "oalist_inv (let v = f k v v'; aux = map2_val_pair f g h xs ys in if v = 0 then aux else (k, v) # aux, ko)"
+      proof (simp add: Let_def, intro conjI impI)
+        assume "f k v v' \<noteq> 0"
+        with 1 show "oalist_inv ((k, f k v v') # map2_val_pair f g h xs ys, ko)"
+        proof (rule oalist_inv_ConsI)
+          define k0 where "k0 = fst (hd (map2_val_pair f g h xs ys))"
+          assume "map2_val_pair f g h xs ys \<noteq> []"
+          hence "k0 \<in> fst ` set (map2_val_pair f g h xs ys)" by (simp add: k0_def)
+          also from *(2) Cons(2) assms(3, 4) have "... \<subseteq> fst ` set xs \<union> fst ` set ys"
+            by (rule fst_map2_val_pair_subset)
+          finally show "lt_of_key_order ko k k0"
+          proof
+            assume "k0 \<in> fst ` set ys"
+            hence "lt_of_key_order ko k' k0" by (rule Cons(4))
+            thus ?thesis by (simp only: \<open>k = k'\<close>)
+          qed (rule *(4))
+        qed
+      qed (rule 1)
+    next
+      assume "key_compare ko k k' = Gt"
+      hence 0: "lt_of_key_order ko k' k" by (simp only: lt_of_key_order_alt key_compare_Gt)
+      show "oalist_inv (let va = f k' 0 v'; aux = map2_val_pair f g h ((k, v) # xs) ys
+              in if va = 0 then aux else (k', va) # aux, ko)"
+      proof (simp add: Let_def, intro conjI impI)
+        assume "f k' 0 v' \<noteq> 0"
+        with Cons(5) show "oalist_inv ((k', f k' 0 v') # map2_val_pair f g h ((k, v) # xs) ys, ko)"
+        proof (rule oalist_inv_ConsI)
+          define k0 where "k0 = fst (hd (map2_val_pair f g h ((k, v) # xs) ys))"
+          assume "map2_val_pair f g h ((k, v) # xs) ys \<noteq> []"
+          hence "k0 \<in> fst ` set (map2_val_pair f g h ((k, v) # xs) ys)" by (simp add: k0_def)
+          also from *(1) Cons(2) assms(3, 4) have "... \<subseteq> fst ` set ((k, v) # xs) \<union> fst ` set ys"
+            by (rule fst_map2_val_pair_subset)
+          finally have "k0 = k \<or> k0 \<in> fst ` set xs \<or> k0 \<in> fst ` set ys" by auto
+          thus "lt_of_key_order ko k' k0"
+          proof (elim disjE)
+            assume "k0 = k"
+            with 0 show ?thesis by simp
+          next
+            assume "k0 \<in> fst ` set xs"
+            hence "lt_of_key_order ko k k0" by (rule *(4))
+            with 0 show ?thesis by (rule key_order_lin.less_trans)
+          qed (rule Cons(4))
+        qed
+      qed (rule Cons(5))
+    qed
+  qed
+qed
+
+lemma lookup_pair_map2_val_pair:
+  assumes "oalist_inv (xs, ko)" and "oalist_inv (ys, ko)"
+  assumes "map2_val_compat g" and "map2_val_compat h"
+  assumes "\<And>zs. oalist_inv (zs, ko) \<Longrightarrow> g ko zs = map_val_pair (\<lambda>k v. f k v 0) zs"
+    and "\<And>zs. oalist_inv (zs, ko) \<Longrightarrow> h ko zs = map_val_pair (\<lambda>k. f k 0) zs"
+    and "\<And>k. f k 0 0 = 0"
+  shows "lookup_pair (map2_val_pair f g h xs ys) k0 = f k0 (lookup_pair xs k0) (lookup_pair ys k0)"
+  using assms(1, 2)
+proof (induct xs arbitrary: ys rule: oalist_inv_induct)
+  case Nil
+  show ?case
+  proof (cases ys)
+    case Nil
+    show ?thesis by (simp add: Nil map2_val_compat_Nil[OF assms(3)] assms(7))
+  next
+    case (Cons y ys')
+    then obtain k v ys' where ys: "ys = (k, v) # ys'" by fastforce
+    from Nil have "lookup_pair (h ko ys) k0 = lookup_pair (map_val_pair (\<lambda>k. f k 0) ys) k0"
+      by (simp only: assms(6))
+    also have "... = f k0 0 (lookup_pair ys k0)" by (rule lookup_pair_map_val_pair, fact Nil, fact assms(7))
+    finally have "lookup_pair (h ko ((k, v) # ys')) k0 = f k0 0 (lookup_pair ((k, v) # ys') k0)"
+      by (simp only: ys)
+    thus ?thesis by (simp add: ys)
+  qed
+next
+  case *: (Cons k v xs)
+  from *(6) show ?case
+  proof (induct ys rule: oalist_inv_induct)
+    case Nil
+    from *(1) have "lookup_pair (g ko ((k, v) # xs)) k0 = lookup_pair (map_val_pair (\<lambda>k v. f k v 0) ((k, v) # xs)) k0"
+      by (simp only: assms(5))
+    also have "... = f k0 (lookup_pair ((k, v) # xs) k0) 0"
+      by (rule lookup_pair_map_val_pair, fact *(1), fact assms(7))
+    finally show ?case by simp
+  next
+    case (Cons k' v' ys)
+    show ?case
+    proof (cases "key_compare ko k0 k = Lt \<and> key_compare ko k0 k' = Lt")
+      case True
+      hence 1: "key_compare ko k0 k = Lt" and 2: "key_compare ko k0 k' = Lt" by simp_all
+      hence eq: "f k0 (lookup_pair ((k, v) # xs) k0) (lookup_pair ((k', v') # ys) k0) = 0"
+        by (simp add: assms(7))
+      from *(1) Cons(1) assms(3, 4) have inv: "oalist_inv (map2_val_pair f g h ((k, v) # xs) ((k', v') # ys), ko)"
+        by (rule oalist_inv_map2_val_pair)
+      show ?thesis
+      proof (simp only: eq lookup_pair_eq_0[OF inv], rule)
+        assume "k0 \<in> fst ` set (local.map2_val_pair f g h ((k, v) # xs) ((k', v') # ys))"
+        also from *(1) Cons(1) assms(3, 4) have "... \<subseteq> fst ` set ((k, v) # xs) \<union> fst ` set ((k', v') # ys)"
+          by (rule fst_map2_val_pair_subset)
+        finally have "k0 \<in> fst ` set xs \<or> k0 \<in> fst ` set ys" using 1 2 by auto
+        thus False
+        proof
+          assume "k0 \<in> fst ` set xs"
+          hence "lt_of_key_order ko k k0" by (rule *(4))
+          with 1 show ?thesis by (simp add: lt_of_key_order_alt[symmetric])
+        next
+          assume "k0 \<in> fst ` set ys"
+          hence "lt_of_key_order ko k' k0" by (rule Cons(4))
+          with 2 show ?thesis by (simp add: lt_of_key_order_alt[symmetric])
+        qed
+      qed
+    next
+      case False
+      show ?thesis
+      proof (simp split: order.split del: lookup_pair.simps, intro conjI impI)
+        assume "key_compare ko k k' = Lt"
+        with False have "key_compare ko k0 k \<noteq> Lt" by (auto simp: lt_of_key_order_alt[symmetric])
+        show "lookup_pair (let v = f k v 0; aux = map2_val_pair f g h xs ((k', v') # ys)
+                            in if v = 0 then aux else (k, v) # aux) k0 =
+              f k0 (lookup_pair ((k, v) # xs) k0) (lookup_pair ((k', v') # ys) k0)"
+        proof (cases "key_compare ko k0 k")
+          case Lt
+          with \<open>key_compare ko k0 k \<noteq> Lt\<close> show ?thesis ..
+        next
+          case Eq
+          hence "k0 = k" by (simp only: key_compare_Eq)
+          with \<open>key_compare ko k k' = Lt\<close> have "key_compare ko k0 k' = Lt" by simp
+          hence eq1: "lookup_pair ((k', v') # ys) k = 0" by (simp add: \<open>k0 = k\<close>)
+          have eq2: "lookup_pair ((k, v) # xs) k = v" by simp
+          show ?thesis
+          proof (simp add: Let_def eq1 eq2 \<open>k0 = k\<close> del: lookup_pair.simps, intro conjI impI)
+            from *(2) Cons(1) assms(3, 4) have inv: "oalist_inv (map2_val_pair f g h xs ((k', v') # ys), ko)"
+              by (rule oalist_inv_map2_val_pair)
+            show "lookup_pair (map2_val_pair f g h xs ((k', v') # ys)) k = 0"
+            proof (simp only: lookup_pair_eq_0[OF inv], rule)
+              assume "k \<in> fst ` set (local.map2_val_pair f g h xs ((k', v') # ys))"
+              also from *(2) Cons(1) assms(3, 4) have "... \<subseteq> fst ` set xs \<union> fst ` set ((k', v') # ys)"
+                by (rule fst_map2_val_pair_subset)
+              finally have "k \<in> fst ` set xs \<or> k \<in> fst ` set ys" using \<open>key_compare ko k k' = Lt\<close>
+                by auto
+              thus False
+              proof
+                assume "k \<in> fst ` set xs"
+                hence "lt_of_key_order ko k k" by (rule *(4))
+                thus ?thesis by simp
+              next
+                assume "k \<in> fst ` set ys"
+                hence "lt_of_key_order ko k' k" by (rule Cons(4))
+                with \<open>key_compare ko k k' = Lt\<close> show ?thesis by (simp add: lt_of_key_order_alt[symmetric])
+              qed
+            qed
+          qed simp
+        next
+          case Gt
+          hence eq1: "lookup_pair ((k, v) # xs) k0 = lookup_pair xs k0"
+            and eq2: "lookup_pair ((k, f k v 0) # map2_val_pair f g h xs ((k', v') # ys)) k0 =
+                  lookup_pair (map2_val_pair f g h xs ((k', v') # ys)) k0" by simp_all
+          show ?thesis
+            by (simp add: Let_def eq1 eq2 del: lookup_pair.simps, rule *(5), fact Cons(1))
+        qed
+      next
+        assume "key_compare ko k k' = Eq"
+        hence "k = k'" by (simp only: key_compare_Eq)
+        with False have "key_compare ko k0 k' \<noteq> Lt" by (auto simp: lt_of_key_order_alt[symmetric])
+        show "lookup_pair (let v = f k v v'; aux = map2_val_pair f g h xs ys in
+                            if v = 0 then aux else (k, v) # aux) k0 =
+              f k0 (lookup_pair ((k, v) # xs) k0) (lookup_pair ((k', v') # ys) k0)"
+        proof (cases "key_compare ko k0 k'")
+          case Lt
+          with \<open>key_compare ko k0 k' \<noteq> Lt\<close> show ?thesis ..
+        next
+          case Eq
+          hence "k0 = k'" by (simp only: key_compare_Eq)
+          show ?thesis
+          proof (simp add: Let_def \<open>k = k'\<close> \<open>k0 = k'\<close>, intro impI)
+            from *(2) Cons(2) assms(3, 4) have inv: "oalist_inv (map2_val_pair f g h xs ys, ko)"
+              by (rule oalist_inv_map2_val_pair)
+            show "lookup_pair (map2_val_pair f g h xs ys) k' = 0"
+            proof (simp only: lookup_pair_eq_0[OF inv], rule)
+              assume "k' \<in> fst ` set (map2_val_pair f g h xs ys)"
+              also from *(2) Cons(2) assms(3, 4) have "... \<subseteq> fst ` set xs \<union> fst ` set ys"
+                by (rule fst_map2_val_pair_subset)
+              finally show False
+              proof
+                assume "k' \<in> fst ` set ys"
+                hence "lt_of_key_order ko k' k'" by (rule Cons(4))
+                thus ?thesis by simp
+              next
+                assume "k' \<in> fst ` set xs"
+                hence "lt_of_key_order ko k k'" by (rule *(4))
+                thus ?thesis by (simp add: \<open>k = k'\<close>)
+              qed
+            qed
+          qed
+        next
+          case Gt
+          hence eq1: "lookup_pair ((k, v) # xs) k0 = lookup_pair xs k0"
+            and eq2: "lookup_pair ((k', v') # ys) k0 = lookup_pair ys k0"
+            and eq3: "lookup_pair ((k, f k v v') # map2_val_pair f g h xs ys) k0 =
+                  lookup_pair (map2_val_pair f g h xs ys) k0" by (simp_all add: \<open>k = k'\<close>)
+          show ?thesis by (simp add: Let_def eq1 eq2 eq3 del: lookup_pair.simps, rule *(5), fact Cons(2))
+        qed
+      next
+        assume "key_compare ko k k' = Gt"
+        hence "key_compare ko k' k = Lt" by (simp only: key_compare_Gt)
+        with False have "key_compare ko k0 k' \<noteq> Lt" by (auto simp: lt_of_key_order_alt[symmetric])
+        show "lookup_pair (let va = f k' 0 v'; aux = map2_val_pair f g h ((k, v) # xs) ys
+                            in if va = 0 then aux else (k', va) # aux) k0 =
+              f k0 (lookup_pair ((k, v) # xs) k0) (lookup_pair ((k', v') # ys) k0)"
+        proof (cases "key_compare ko k0 k'")
+          case Lt
+          with \<open>key_compare ko k0 k' \<noteq> Lt\<close> show ?thesis ..
+        next
+          case Eq
+          hence "k0 = k'" by (simp only: key_compare_Eq)
+          with \<open>key_compare ko k' k = Lt\<close> have "key_compare ko k0 k = Lt" by simp
+          hence eq1: "lookup_pair ((k, v) # xs) k' = 0" by (simp add: \<open>k0 = k'\<close>)
+          have eq2: "lookup_pair ((k', v') # ys) k' = v'" by simp
+          show ?thesis
+          proof (simp add: Let_def eq1 eq2 \<open>k0 = k'\<close> del: lookup_pair.simps, intro conjI impI)
+            from *(1) Cons(2) assms(3, 4) have inv: "oalist_inv (map2_val_pair f g h ((k, v) # xs) ys, ko)"
+              by (rule oalist_inv_map2_val_pair)
+            show "lookup_pair (map2_val_pair f g h ((k, v) # xs) ys) k' = 0"
+            proof (simp only: lookup_pair_eq_0[OF inv], rule)
+              assume "k' \<in> fst ` set (map2_val_pair f g h ((k, v) # xs) ys)"
+              also from *(1) Cons(2) assms(3, 4) have "... \<subseteq> fst ` set ((k, v) # xs) \<union> fst ` set ys"
+                by (rule fst_map2_val_pair_subset)
+              finally have "k' \<in> fst ` set xs \<or> k' \<in> fst ` set ys" using \<open>key_compare ko k' k = Lt\<close>
+                by auto
+              thus False
+              proof
+                assume "k' \<in> fst ` set ys"
+                hence "lt_of_key_order ko k' k'" by (rule Cons(4))
+                thus ?thesis by simp
+              next
+                assume "k' \<in> fst ` set xs"
+                hence "lt_of_key_order ko k k'" by (rule *(4))
+                with \<open>key_compare ko k' k = Lt\<close> show ?thesis by (simp add: lt_of_key_order_alt[symmetric])
+              qed
+            qed
+          qed simp
+        next
+          case Gt
+          hence eq1: "lookup_pair ((k', v') # ys) k0 = lookup_pair ys k0"
+            and eq2: "lookup_pair ((k', f k' 0 v') # map2_val_pair f g h ((k, v) # xs) ys) k0 =
+                  lookup_pair (map2_val_pair f g h ((k, v) # xs) ys) k0" by simp_all
+          show ?thesis by (simp add: Let_def eq1 eq2 del: lookup_pair.simps, rule Cons(5))
+        qed
+      qed
+    qed
+  qed
+qed
+
+lemma map2_val_pair_singleton_eq_update_by_fun_pair:
+  assumes "oalist_inv (xs, ko)"
+  assumes "\<And>k x. f k x 0 = x" and "\<And>zs. oalist_inv (zs, ko) \<Longrightarrow> g ko zs = zs"
+    and "h ko [(k, v)] = map_val_pair (\<lambda>k. f k 0) [(k, v)]"
+  shows "map2_val_pair f g h xs [(k, v)] = update_by_fun_pair k (\<lambda>x. f k x v) xs"
+  using assms(1)
+proof (induct xs rule: oalist_inv_induct)
+  case Nil
+  show ?case by (simp add: Let_def assms(4))
+next
+  case (Cons k' v' xs)
+  show ?case
+  proof (cases "key_compare ko k' k")
+    case Lt
+    hence gr: "key_compare ko k k' = Gt" by (simp only: key_compare_Gt)
+    show ?thesis by (simp add: Lt gr Let_def assms(2) Cons(3, 5))
+  next
+    case Eq
+    hence eq1: "key_compare ko k k' = Eq" and eq2: "k = k'" by (simp_all only: key_compare_Eq)
+    show ?thesis by (simp add: Eq eq1 eq2 Let_def assms(3)[OF Cons(2)])
+  next
+    case Gt
+    hence less: "key_compare ko k k' = Lt" by (simp only: key_compare_Gt)
+    show ?thesis by (simp add: Gt less Let_def assms(3)[OF Cons(1)])
+  qed
+qed
+
+subsubsection \<open>@{const lex_ord_pair}\<close>
+
+lemma lex_ord_pair_EqI:
+  assumes "oalist_inv (xs, ko)" and "oalist_inv (ys, ko)"
+    and "\<And>k. k \<in> fst ` set xs \<union> fst ` set ys \<Longrightarrow> f k (lookup_pair xs k) (lookup_pair ys k) = Some Eq"
+  shows "lex_ord_pair f xs ys = Some Eq"
+  using assms
+proof (induct xs arbitrary: ys rule: oalist_inv_induct)
+  case Nil
+  thus ?case
+  proof (induct ys rule: oalist_inv_induct)
+    case Nil
+    show ?case by simp
+  next
+    case (Cons k v ys)
+    show ?case
+    proof (simp add: Let_def, intro conjI impI, rule Cons(5))
+      fix k0
+      assume "k0 \<in> fst ` set [] \<union> fst ` set ys"
+      hence "k0 \<in> fst ` set ys" by simp
+      hence "lt_of_key_order ko k k0" by (rule Cons(4))
+      hence "f k0 (lookup_pair [] k0) (lookup_pair ys k0) = f k0 (lookup_pair [] k0) (lookup_pair ((k, v) # ys) k0)"
+        by (auto simp add: lookup_pair_Cons[OF Cons(1)] simp del: lookup_pair.simps)
+      also have "... = Some Eq" by (rule Cons(6), simp add: \<open>k0 \<in> fst ` set ys\<close>)
+      finally show "f k0 (lookup_pair [] k0) (lookup_pair ys k0) = Some Eq" .
+    next
+      have "f k 0 v = f k (lookup_pair [] k) (lookup_pair ((k, v) # ys) k)" by simp
+      also have "... = Some Eq" by (rule Cons(6), simp)
+      finally show "f k 0 v = Some Eq" .
+    qed
+  qed
+next
+  case *: (Cons k v xs)
+  from *(6, 7) show ?case
+  proof (induct ys rule: oalist_inv_induct)
+    case Nil
+    show ?case
+    proof (simp add: Let_def, intro conjI impI, rule *(5), rule oalist_inv_Nil)
+      fix k0
+      assume "k0 \<in> fst ` set xs \<union> fst ` set []"
+      hence "k0 \<in> fst ` set xs" by simp
+      hence "lt_of_key_order ko k k0" by (rule *(4))
+      hence "f k0 (lookup_pair xs k0) (lookup_pair [] k0) = f k0 (lookup_pair ((k, v) # xs) k0) (lookup_pair [] k0)"
+        by (auto simp add: lookup_pair_Cons[OF *(1)] simp del: lookup_pair.simps)
+      also have "... = Some Eq" by (rule Nil, simp add: \<open>k0 \<in> fst ` set xs\<close>)
+      finally show "f k0 (lookup_pair xs k0) (lookup_pair [] k0) = Some Eq" .
+    next
+      have "f k v 0 = f k (lookup_pair ((k, v) # xs) k) (lookup_pair [] k)" by simp
+      also have "... = Some Eq" by (rule Nil, simp)
+      finally show "f k v 0 = Some Eq" .
+    qed
+  next
+    case (Cons k' v' ys)
+    show ?case
+    proof (simp split: order.split, intro conjI impI)
+      assume "key_compare ko k k' = Lt"
+      show "(let aux = f k v 0 in if aux = Some Eq then lex_ord_pair f xs ((k', v') # ys) else aux) = Some Eq"
+      proof (simp add: Let_def, intro conjI impI, rule *(5), rule Cons(1))
+        fix k0
+        assume k0_in: "k0 \<in> fst ` set xs \<union> fst ` set ((k', v') # ys)"
+        hence "k0 \<in> fst ` set xs \<or> k0 = k' \<or> k0 \<in> fst ` set ys" by auto
+        hence "k0 \<noteq> k"
+        proof (elim disjE)
+          assume "k0 \<in> fst ` set xs"
+          hence "lt_of_key_order ko k k0" by (rule *(4))
+          thus ?thesis by simp
+        next
+          assume "k0 = k'"
+          with \<open>key_compare ko k k' = Lt\<close> show ?thesis by auto
+        next
+          assume "k0 \<in> fst ` set ys"
+          hence "lt_of_key_order ko k' k0" by (rule Cons(4))
+          with \<open>key_compare ko k k' = Lt\<close> show ?thesis by (simp add: lt_of_key_order_alt[symmetric])
+        qed
+        hence "f k0 (lookup_pair xs k0) (lookup_pair ((k', v') # ys) k0) =
+                f k0 (lookup_pair ((k, v) # xs) k0) (lookup_pair ((k', v') # ys) k0)"
+          by (auto simp add: lookup_pair_Cons[OF *(1)] simp del: lookup_pair.simps)
+        also have "... = Some Eq" by (rule Cons(6), rule set_rev_mp, fact k0_in, auto)
+        finally show "f k0 (lookup_pair xs k0) (lookup_pair ((k', v') # ys) k0) = Some Eq" .
+      next
+        have "f k v 0 = f k (lookup_pair ((k, v) # xs) k) (lookup_pair ((k', v') # ys) k)"
+          by (simp add: \<open>key_compare ko k k' = Lt\<close>)
+        also have "... = Some Eq" by (rule Cons(6), simp)
+        finally show "f k v 0 = Some Eq" .
+      qed
+    next
+      assume "key_compare ko k k' = Eq"
+      hence "k = k'" by (simp only: key_compare_Eq)
+      show "(let aux = f k v v' in if aux = Some Eq then lex_ord_pair f xs ys else aux) = Some Eq"
+      proof (simp add: Let_def, intro conjI impI, rule *(5), rule Cons(2))
+        fix k0
+        assume k0_in: "k0 \<in> fst ` set xs \<union> fst ` set ys"
+        hence "k0 \<noteq> k'"
+        proof
+          assume "k0 \<in> fst ` set xs"
+          hence "lt_of_key_order ko k k0" by (rule *(4))
+          thus ?thesis by (simp add: \<open>k = k'\<close>)
+        next
+          assume "k0 \<in> fst ` set ys"
+          hence "lt_of_key_order ko k' k0" by (rule Cons(4))
+          thus ?thesis by simp
+        qed
+        hence "f k0 (lookup_pair xs k0) (lookup_pair ys k0) =
+                f k0 (lookup_pair ((k, v) # xs) k0) (lookup_pair ((k', v') # ys) k0)"
+          by (simp add: lookup_pair_Cons[OF *(1)] lookup_pair_Cons[OF Cons(1)] del: lookup_pair.simps,
+              auto simp: \<open>k = k'\<close>)
+        also have "... = Some Eq" by (rule Cons(6), rule set_rev_mp, fact k0_in, auto)
+        finally show "f k0 (lookup_pair xs k0) (lookup_pair ys k0) = Some Eq" .
+      next
+        have "f k v v' = f k (lookup_pair ((k, v) # xs) k) (lookup_pair ((k', v') # ys) k)"
+          by (simp add: \<open>k = k'\<close>)
+        also have "... = Some Eq" by (rule Cons(6), simp)
+        finally show "f k v v' = Some Eq" .
+      qed
+    next
+      assume "key_compare ko k k' = Gt"
+      hence "key_compare ko k' k = Lt" by (simp only: key_compare_Gt)
+      show "(let aux = f k' 0 v' in if aux = Some Eq then lex_ord_pair f ((k, v) # xs) ys else aux) = Some Eq"
+      proof (simp add: Let_def, intro conjI impI, rule Cons(5))
+        fix k0
+        assume k0_in: "k0 \<in> fst ` set ((k, v) # xs) \<union> fst ` set ys"
+        hence "k0 \<in> fst ` set xs \<or> k0 = k \<or> k0 \<in> fst ` set ys" by auto
+        hence "k0 \<noteq> k'"
+        proof (elim disjE)
+          assume "k0 \<in> fst ` set xs"
+          hence "lt_of_key_order ko k k0" by (rule *(4))
+          with \<open>key_compare ko k' k = Lt\<close> show ?thesis by (simp add: lt_of_key_order_alt[symmetric])
+        next
+          assume "k0 = k"
+          with \<open>key_compare ko k' k = Lt\<close> show ?thesis by auto
+        next
+          assume "k0 \<in> fst ` set ys"
+          hence "lt_of_key_order ko k' k0" by (rule Cons(4))
+          thus ?thesis by simp
+        qed
+        hence "f k0 (lookup_pair ((k, v) # xs) k0) (lookup_pair ys k0) =
+                f k0 (lookup_pair ((k, v) # xs) k0) (lookup_pair ((k', v') # ys) k0)"
+          by (auto simp add: lookup_pair_Cons[OF Cons(1)] simp del: lookup_pair.simps)
+        also have "... = Some Eq" by (rule Cons(6), rule set_rev_mp, fact k0_in, auto)
+        finally show "f k0 (lookup_pair ((k, v) # xs) k0) (lookup_pair ys k0) = Some Eq" .
+      next
+        have "f k' 0 v' = f k' (lookup_pair ((k, v) # xs) k') (lookup_pair ((k', v') # ys) k')"
+          by (simp add: \<open>key_compare ko k' k = Lt\<close>)
+        also have "... = Some Eq" by (rule Cons(6), simp)
+        finally show "f k' 0 v' = Some Eq" .
+      qed
+    qed
+  qed
+qed
+
+lemma lex_ord_pair_valI:
+  assumes "oalist_inv (xs, ko)" and "oalist_inv (ys, ko)" and "aux \<noteq> Some Eq"
+  assumes "k \<in> fst ` set xs \<union> fst ` set ys" and "aux = f k (lookup_pair xs k) (lookup_pair ys k)"
+    and "\<And>k'. k' \<in> fst ` set xs \<union> fst ` set ys \<Longrightarrow> lt_of_key_order ko k' k \<Longrightarrow>
+              f k' (lookup_pair xs k') (lookup_pair ys k') = Some Eq"
+  shows "lex_ord_pair f xs ys = aux"
+  using assms(1, 2, 4, 5, 6)
+proof (induct xs arbitrary: ys rule: oalist_inv_induct)
+  case Nil
+  thus ?case
+  proof (induct ys rule: oalist_inv_induct)
+    case Nil
+    from Nil(1) show ?case by simp
+  next
+    case (Cons k' v' ys)
+    from Cons(6) have "k = k' \<or> k \<in> fst ` set ys" by simp
+    thus ?case
+    proof
+      assume "k = k'"
+      with Cons(7) have "f k' 0 v' = aux" by simp
+      thus ?thesis by (simp add: Let_def \<open>k = k'\<close> assms(3))
+    next
+      assume "k \<in> fst `set ys"
+      hence "lt_of_key_order ko k' k" by (rule Cons(4))
+      hence "key_compare ko k k' = Gt" by (simp add: lt_of_key_order_alt key_compare_Gt)
+      hence eq1: "lookup_pair ((k', v') # ys) k = lookup_pair ys k" by simp
+      have "f k' (lookup_pair [] k') (lookup_pair ((k', v') # ys) k') = Some Eq"
+        by (rule Cons(8), simp, fact)
+      hence eq2: "f k' 0 v' = Some Eq" by simp
+      show ?thesis
+      proof (simp add: Let_def eq2, rule Cons(5))
+        from \<open>k \<in> fst `set ys\<close> show "k \<in> fst ` set [] \<union> fst ` set ys" by simp
+      next
+        show "aux = f k (lookup_pair [] k) (lookup_pair ys k)" by (simp only: Cons(7) eq1)
+      next
+        fix k0
+        assume "lt_of_key_order ko k0 k"
+        assume "k0 \<in> fst ` set [] \<union> fst ` set ys"
+        hence k0_in: "k0 \<in> fst ` set ys" by simp
+        hence "lt_of_key_order ko k' k0" by (rule Cons(4))
+        hence "key_compare ko k0 k' = Gt" by (simp add: lt_of_key_order_alt key_compare_Gt)
+        hence "f k0 (lookup_pair [] k0) (lookup_pair ys k0) =
+                f k0 (lookup_pair [] k0) (lookup_pair ((k', v') # ys) k0)" by simp
+        also have "... = Some Eq" by (rule Cons(8), simp add: k0_in, fact)
+        finally show "f k0 (lookup_pair [] k0) (lookup_pair ys k0) = Some Eq" .
+      qed
+    qed
+  qed
+next
+  case *: (Cons k' v' xs)
+  from *(6, 7, 8, 9) show ?case
+  proof (induct ys rule: oalist_inv_induct)
+    case Nil
+    from Nil(1) have "k = k' \<or> k \<in> fst ` set xs" by simp
+    thus ?case
+    proof
+      assume "k = k'"
+      with Nil(2) have "f k' v' 0 = aux" by simp
+      thus ?thesis by (simp add: Let_def \<open>k = k'\<close> assms(3))
+    next
+      assume "k \<in> fst ` set xs"
+      hence "lt_of_key_order ko k' k" by (rule *(4))
+      hence "key_compare ko k k' = Gt" by (simp add: lt_of_key_order_alt key_compare_Gt)
+      hence eq1: "lookup_pair ((k', v') # xs) k = lookup_pair xs k" by simp
+      have "f k' (lookup_pair ((k', v') # xs) k') (lookup_pair [] k') = Some Eq"
+        by (rule Nil(3), simp, fact)
+      hence eq2: "f k' v' 0 = Some Eq" by simp
+      show ?thesis
+      proof (simp add: Let_def eq2, rule *(5), fact oalist_inv_Nil)
+        from \<open>k \<in> fst `set xs\<close> show "k \<in> fst ` set xs \<union> fst ` set []" by simp
+      next
+        show "aux = f k (lookup_pair xs k) (lookup_pair [] k)" by (simp only: Nil(2) eq1)
+      next
+        fix k0
+        assume "lt_of_key_order ko k0 k"
+        assume "k0 \<in> fst ` set xs \<union> fst ` set []"
+        hence k0_in: "k0 \<in> fst ` set xs" by simp
+        hence "lt_of_key_order ko k' k0" by (rule *(4))
+        hence "key_compare ko k0 k' = Gt" by (simp add: lt_of_key_order_alt key_compare_Gt)
+        hence "f k0 (lookup_pair xs k0) (lookup_pair [] k0) =
+                f k0 (lookup_pair ((k', v') # xs) k0) (lookup_pair [] k0)" by simp
+        also have "... = Some Eq" by (rule Nil(3), simp add: k0_in, fact)
+        finally show "f k0 (lookup_pair xs k0) (lookup_pair [] k0) = Some Eq" .
+      qed
+    qed
+  next
+    case (Cons k'' v'' ys)
+
+    have 0: thesis if 1: "lt_of_key_order ko k k'" and 2: "lt_of_key_order ko k k''" for thesis
+    proof -
+      from 1 have "k \<noteq> k'" by simp
+      moreover from 2 have "k \<noteq> k''" by simp
+      ultimately have "k \<in> fst ` set xs \<or> k \<in> fst ` set ys" using Cons(6) by simp
+      thus ?thesis
+      proof
+        assume "k \<in> fst ` set xs"
+        hence "lt_of_key_order ko k' k" by (rule *(4))
+        with 1 show ?thesis by simp
+      next
+        assume "k \<in> fst ` set ys"
+        hence "lt_of_key_order ko k'' k" by (rule Cons(4))
+        with 2 show ?thesis by simp
+      qed
+    qed
+
+    show ?case
+    proof (simp split: order.split, intro conjI impI)
+      assume Lt: "key_compare ko k' k'' = Lt"
+      show "(let aux = f k' v' 0 in if aux = Some Eq then lex_ord_pair f xs ((k'', v'') # ys) else aux) = aux"
+      proof (simp add: Let_def split: order.split, intro conjI impI)
+        assume "f k' v' 0 = Some Eq"
+        have "k \<noteq> k'"
+        proof
+          assume "k = k'"
+          have "aux = f k v' 0" by (simp add: Cons(7) \<open>k = k'\<close> Lt)
+          with \<open>f k' v' 0 = Some Eq\<close> assms(3) show False by (simp add: \<open>k = k'\<close>)
+        qed
+        from Cons(1) show "lex_ord_pair f xs ((k'', v'') # ys) = aux"
+        proof (rule *(5))
+          from Cons(6) \<open>k \<noteq> k'\<close> show "k \<in> fst ` set xs \<union> fst ` set ((k'', v'') # ys)" by simp
+        next
+          show "aux = f k (lookup_pair xs k) (lookup_pair ((k'', v'') # ys) k)"
+            by (simp add: Cons(7) lookup_pair_Cons[OF *(1)] \<open>k \<noteq> k'\<close>[symmetric] del: lookup_pair.simps)
+        next
+          fix k0
+          assume "lt_of_key_order ko k0 k"
+          assume k0_in: "k0 \<in> fst ` set xs \<union> fst ` set ((k'', v'') # ys)"
+          also have "... \<subseteq> fst ` set ((k', v') # xs) \<union> fst ` set ((k'', v'') # ys)" by fastforce
+          finally have k0_in': "k0 \<in> fst ` set ((k', v') # xs) \<union> fst ` set ((k'', v'') # ys)" .
+          have "k' \<noteq> k0"
+          proof
+            assume "k' = k0"
+            with k0_in have "k' \<in> fst ` set xs \<union> fst ` set ((k'', v'') # ys)" by simp
+            with Lt have "k' \<in> fst ` set xs \<or> k' \<in> fst ` set ys" by auto
+            thus False
+            proof
+              assume "k' \<in> fst ` set xs"
+              hence "lt_of_key_order ko k' k'" by (rule *(4))
+              thus ?thesis by simp
+            next
+              assume "k' \<in> fst ` set ys"
+              hence "lt_of_key_order ko k'' k'" by (rule Cons(4))
+              with Lt show ?thesis by (simp add: lt_of_key_order_alt[symmetric])
+            qed
+          qed
+          hence "f k0 (lookup_pair xs k0) (lookup_pair ((k'', v'') # ys) k0) =
+                  f k0 (lookup_pair ((k', v') # xs) k0) (lookup_pair ((k'', v'') # ys) k0)"
+            by (simp add: lookup_pair_Cons[OF *(1)] del: lookup_pair.simps)
+          also from k0_in' \<open>lt_of_key_order ko k0 k\<close> have "... = Some Eq" by (rule Cons(8))
+          finally show "f k0 (lookup_pair xs k0) (lookup_pair ((k'', v'') # ys) k0) = Some Eq" .
+        qed
+      next
+        assume "f k' v' 0 \<noteq> Some Eq"
+        have "\<not> lt_of_key_order ko k' k"
+        proof
+          have "k' \<in> fst ` set ((k', v') # xs) \<union> fst ` set ((k'', v'') # ys)" by simp
+          moreover assume "lt_of_key_order ko k' k"
+          ultimately have "f k' (lookup_pair ((k', v') # xs) k') (lookup_pair ((k'', v'') # ys) k') = Some Eq"
+            by (rule Cons(8))
+          hence "f k' v' 0 = Some Eq" by (simp add: Lt)
+          with \<open>f k' v' 0 \<noteq> Some Eq\<close> show False ..
+        qed
+        moreover have "\<not> lt_of_key_order ko k k'"
+        proof
+          assume "lt_of_key_order ko k k'"
+          moreover from this Lt have "lt_of_key_order ko k k''"
+            by (simp add: lt_of_key_order_alt[symmetric])
+          ultimately show False by (rule 0)
+        qed
+        ultimately have "k = k'" by simp
+        show "f k' v' 0 = aux" by (simp add: Cons(7) \<open>k = k'\<close> Lt)
+      qed
+    next
+      assume "key_compare ko k' k'' = Eq"
+      hence "k' = k''" by (simp only: key_compare_Eq)
+      show "(let aux = f k' v' v'' in if aux = Some Eq then lex_ord_pair f xs ys else aux) = aux"
+      proof (simp add: Let_def \<open>k' = k''\<close> split: order.split, intro conjI impI)
+        assume "f k'' v' v'' = Some Eq"
+        have "k \<noteq> k''"
+        proof
+          assume "k = k''"
+          have "aux = f k v' v''" by (simp add: Cons(7) \<open>k = k''\<close> \<open>k' = k''\<close>)
+          with \<open>f k'' v' v'' = Some Eq\<close> assms(3) show False by (simp add: \<open>k = k''\<close>)
+        qed
+        from Cons(2) show "lex_ord_pair f xs ys = aux"
+        proof (rule *(5))
+          from Cons(6) \<open>k \<noteq> k''\<close> show "k \<in> fst ` set xs \<union> fst ` set ys" by (simp add: \<open>k' = k''\<close>)
+        next
+          show "aux = f k (lookup_pair xs k) (lookup_pair ys k)"
+            by (simp add: Cons(7) lookup_pair_Cons[OF *(1)] lookup_pair_Cons[OF Cons(1)] del: lookup_pair.simps,
+                simp add: \<open>k' = k''\<close> \<open>k \<noteq> k''\<close>[symmetric])
+        next
+          fix k0
+          assume "lt_of_key_order ko k0 k"
+          assume k0_in: "k0 \<in> fst ` set xs \<union> fst ` set ys"
+          also have "... \<subseteq> fst ` set ((k', v') # xs) \<union> fst ` set ((k'', v'') # ys)" by fastforce
+          finally have k0_in': "k0 \<in> fst ` set ((k', v') # xs) \<union> fst ` set ((k'', v'') # ys)" .
+          have "k'' \<noteq> k0"
+          proof
+            assume "k'' = k0"
+            with k0_in have "k'' \<in> fst ` set xs \<union> fst ` set ys" by simp
+            thus False
+            proof
+              assume "k'' \<in> fst ` set xs"
+              hence "lt_of_key_order ko k' k''" by (rule *(4))
+              thus ?thesis by (simp add: \<open>k' = k''\<close>)
+            next
+              assume "k'' \<in> fst ` set ys"
+              hence "lt_of_key_order ko k'' k''" by (rule Cons(4))
+              thus ?thesis by simp
+            qed
+          qed
+          hence "f k0 (lookup_pair xs k0) (lookup_pair ys k0) =
+                  f k0 (lookup_pair ((k', v') # xs) k0) (lookup_pair ((k'', v'') # ys) k0)"
+            by (simp add: lookup_pair_Cons[OF *(1)] lookup_pair_Cons[OF Cons(1)] del: lookup_pair.simps,
+                simp add: \<open>k' = k''\<close>)
+          also from k0_in' \<open>lt_of_key_order ko k0 k\<close> have "... = Some Eq" by (rule Cons(8))
+          finally show "f k0 (lookup_pair xs k0) (lookup_pair ys k0) = Some Eq" .
+        qed
+      next
+        assume "f k'' v' v'' \<noteq> Some Eq"
+        have "\<not> lt_of_key_order ko k'' k"
+        proof
+          have "k'' \<in> fst ` set ((k', v') # xs) \<union> fst ` set ((k'', v'') # ys)" by simp
+          moreover assume "lt_of_key_order ko k'' k"
+          ultimately have "f k'' (lookup_pair ((k', v') # xs) k'') (lookup_pair ((k'', v'') # ys) k'') = Some Eq"
+            by (rule Cons(8))
+          hence "f k'' v' v'' = Some Eq" by (simp add: \<open>k' = k''\<close>)
+          with \<open>f k'' v' v'' \<noteq> Some Eq\<close> show False ..
+        qed
+        moreover have "\<not> lt_of_key_order ko k k''"
+        proof
+          assume "lt_of_key_order ko k k''"
+          hence "lt_of_key_order ko k k'" by (simp only: \<open>k' = k''\<close>)
+          thus False using \<open>lt_of_key_order ko k k''\<close> by (rule 0)
+        qed
+        ultimately have "k = k''" by simp
+        show "f k'' v' v'' = aux" by (simp add: Cons(7) \<open>k = k''\<close> \<open>k' = k''\<close>)
+      qed
+    next
+      assume Gt: "key_compare ko k' k'' = Gt"
+      hence Lt: "key_compare ko k'' k' = Lt" by (simp only: key_compare_Gt)
+      show "(let aux = f k'' 0 v'' in if aux = Some Eq then lex_ord_pair f ((k', v') # xs) ys else aux) = aux"
+      proof (simp add: Let_def split: order.split, intro conjI impI)
+        assume "f k'' 0 v'' = Some Eq"
+        have "k \<noteq> k''"
+        proof
+          assume "k = k''"
+          have "aux = f k 0 v''" by (simp add: Cons(7) \<open>k = k''\<close> Lt)
+          with \<open>f k'' 0 v'' = Some Eq\<close> assms(3) show False by (simp add: \<open>k = k''\<close>)
+        qed
+        show "lex_ord_pair f ((k', v') # xs) ys = aux"
+        proof (rule Cons(5))
+          from Cons(6) \<open>k \<noteq> k''\<close> show "k \<in> fst ` set ((k', v') # xs) \<union> fst ` set ys" by simp
+        next
+          show "aux = f k (lookup_pair ((k', v') # xs) k) (lookup_pair ys k)"
+            by (simp add: Cons(7) lookup_pair_Cons[OF Cons(1)] \<open>k \<noteq> k''\<close>[symmetric] del: lookup_pair.simps)
+        next
+          fix k0
+          assume "lt_of_key_order ko k0 k"
+          assume k0_in: "k0 \<in> fst ` set ((k', v') # xs) \<union> fst ` set ys"
+          also have "... \<subseteq> fst ` set ((k', v') # xs) \<union> fst ` set ((k'', v'') # ys)" by fastforce
+          finally have k0_in': "k0 \<in> fst ` set ((k', v') # xs) \<union> fst ` set ((k'', v'') # ys)" .
+          have "k'' \<noteq> k0"
+          proof
+            assume "k'' = k0"
+            with k0_in have "k'' \<in> fst ` set ((k', v') # xs) \<union> fst ` set ys" by simp
+            with Lt have "k'' \<in> fst ` set xs \<or> k'' \<in> fst ` set ys" by auto
+            thus False
+            proof
+              assume "k'' \<in> fst ` set xs"
+              hence "lt_of_key_order ko k' k''" by (rule *(4))
+              with Lt show ?thesis by (simp add: lt_of_key_order_alt[symmetric])
+            next
+              assume "k'' \<in> fst ` set ys"
+              hence "lt_of_key_order ko k'' k''" by (rule Cons(4))
+              thus ?thesis by simp
+            qed
+          qed
+          hence "f k0 (lookup_pair ((k', v') # xs) k0) (lookup_pair ys k0) =
+                  f k0 (lookup_pair ((k', v') # xs) k0) (lookup_pair ((k'', v'') # ys) k0)"
+            by (simp add: lookup_pair_Cons[OF Cons(1)] del: lookup_pair.simps)
+          also from k0_in' \<open>lt_of_key_order ko k0 k\<close> have "... = Some Eq" by (rule Cons(8))
+          finally show "f k0 (lookup_pair ((k', v') # xs) k0) (lookup_pair ys k0) = Some Eq" .
+        qed
+      next
+        assume "f k'' 0 v'' \<noteq> Some Eq"
+        have "\<not> lt_of_key_order ko k'' k"
+        proof
+          have "k'' \<in> fst ` set ((k', v') # xs) \<union> fst ` set ((k'', v'') # ys)" by simp
+          moreover assume "lt_of_key_order ko k'' k"
+          ultimately have "f k'' (lookup_pair ((k', v') # xs) k'') (lookup_pair ((k'', v'') # ys) k'') = Some Eq"
+            by (rule Cons(8))
+          hence "f k'' 0 v'' = Some Eq" by (simp add: Lt)
+          with \<open>f k'' 0 v'' \<noteq> Some Eq\<close> show False ..
+        qed
+        moreover have "\<not> lt_of_key_order ko k k''"
+        proof
+          assume "lt_of_key_order ko k k''"
+          with Lt have "lt_of_key_order ko k k'" by (simp add: lt_of_key_order_alt[symmetric])
+          thus False using \<open>lt_of_key_order ko k k''\<close> by (rule 0)
+        qed
+        ultimately have "k = k''" by simp
+        show "f k'' 0 v'' = aux" by (simp add: Cons(7) \<open>k = k''\<close> Lt)
+      qed
+    qed
+  qed
+qed
+
+lemma lex_ord_pair_EqD:
+  assumes "oalist_inv (xs, ko)" and "oalist_inv (ys, ko)" and "lex_ord_pair f xs ys = Some Eq"
+    and "k \<in> fst ` set xs \<union> fst ` set ys"
+  shows "f k (lookup_pair xs k) (lookup_pair ys k) = Some Eq"
+proof (rule ccontr)
+  let ?A = "(fst ` set xs \<union> fst ` set ys) \<inter> {k. f k (lookup_pair xs k) (lookup_pair ys k) \<noteq> Some Eq}"
+  define k0 where "k0 = key_order_lin.Min ko ?A"
+  have "finite ?A" by auto
+  assume "f k (lookup_pair xs k) (lookup_pair ys k) \<noteq> Some Eq"
+  with assms(4) have "k \<in> ?A" by simp
+  hence "?A \<noteq> {}" by blast
+  with \<open>finite ?A\<close> have "k0 \<in> ?A" unfolding k0_def by (rule key_order_lin.Min_in)
+  hence k0_in: "k0 \<in> fst ` set xs \<union> fst ` set ys"
+    and neq: "f k0 (lookup_pair xs k0) (lookup_pair ys k0) \<noteq> Some Eq" by simp_all
+  have "le_of_key_order ko k0 k'" if "k' \<in> ?A" for k' unfolding k0_def using \<open>finite ?A\<close> that
+    by (rule key_order_lin.Min_le)
+  hence "f k' (lookup_pair xs k') (lookup_pair ys k') = Some Eq"
+    if "k' \<in> fst ` set xs \<union> fst ` set ys" and "lt_of_key_order ko k' k0" for k' using that by fastforce
+  with assms(1, 2) neq k0_in refl have "lex_ord_pair f xs ys = f k0 (lookup_pair xs k0) (lookup_pair ys k0)"
+    by (rule lex_ord_pair_valI)
+  with assms(3) neq show False by simp
+qed
+
+lemma lex_ord_pair_valE:
+  assumes "oalist_inv (xs, ko)" and "oalist_inv (ys, ko)" and "lex_ord_pair f xs ys = aux"
+    and "aux \<noteq> Some Eq"
+  obtains k where "k \<in> fst ` set xs \<union> fst ` set ys" and "aux = f k (lookup_pair xs k) (lookup_pair ys k)"
+    and "\<And>k'. k' \<in> fst ` set xs \<union> fst ` set ys \<Longrightarrow> lt_of_key_order ko k' k \<Longrightarrow>
+            f k' (lookup_pair xs k') (lookup_pair ys k') = Some Eq"
+proof -
+  let ?A = "(fst ` set xs \<union> fst ` set ys) \<inter> {k. f k (lookup_pair xs k) (lookup_pair ys k) \<noteq> Some Eq}"
+  define k where "k = key_order_lin.Min ko ?A"
+  have "finite ?A" by auto
+  have "\<exists>k \<in> fst ` set xs \<union> fst ` set ys. f k (lookup_pair xs k) (lookup_pair ys k) \<noteq> Some Eq" (is ?prop)
+  proof (rule ccontr)
+    assume "\<not> ?prop"
+    hence "f k (lookup_pair xs k) (lookup_pair ys k) = Some Eq"
+      if "k \<in> fst ` set xs \<union> fst ` set ys" for k using that by auto
+    with assms(1, 2) have "lex_ord_pair f xs ys = Some Eq" by (rule lex_ord_pair_EqI)
+    with assms(3, 4) show False by simp
+  qed
+  then obtain k0 where "k0 \<in> fst ` set xs \<union> fst ` set ys"
+    and "f k0 (lookup_pair xs k0) (lookup_pair ys k0) \<noteq> Some Eq" ..
+  hence "k0 \<in> ?A" by simp
+  hence "?A \<noteq> {}" by blast
+  with \<open>finite ?A\<close> have "k \<in> ?A" unfolding k_def by (rule key_order_lin.Min_in)
+  hence k_in: "k \<in> fst ` set xs \<union> fst ` set ys"
+    and neq: "f k (lookup_pair xs k) (lookup_pair ys k) \<noteq> Some Eq" by simp_all
+  have "le_of_key_order ko k k'" if "k' \<in> ?A" for k' unfolding k_def using \<open>finite ?A\<close> that
+    by (rule key_order_lin.Min_le)
+  hence *: "\<And>k'. k' \<in> fst ` set xs \<union> fst ` set ys \<Longrightarrow> lt_of_key_order ko k' k \<Longrightarrow>
+            f k' (lookup_pair xs k') (lookup_pair ys k') = Some Eq" by fastforce
+  with assms(1, 2) neq k_in refl have "lex_ord_pair f xs ys = f k (lookup_pair xs k) (lookup_pair ys k)"
+    by (rule lex_ord_pair_valI)
+  hence "aux = f k (lookup_pair xs k) (lookup_pair ys k)" by (simp only: assms(3))
+  with k_in show ?thesis using * ..
+qed
+
+subsubsection \<open>@{const prod_ord_pair}\<close>
+
+lemma prod_ord_pair_eq_lex_ord_pair:
+  "prod_ord_pair P xs ys = (lex_ord_pair (\<lambda>k x y. if P k x y then Some Eq else None) xs ys = Some Eq)"
+proof (induct P xs ys rule: prod_ord_pair.induct)
+  case (1 P)
+  show ?case by simp
+next
+  case (2 P ky vy ys)
+  thus ?case by simp
+next
+  case (3 P kx vx xs)
+  thus ?case by simp
+next
+  case (4 P kx vx xs ky vy ys)
+  show ?case
+  proof (cases "key_compare ko kx ky")
+    case Lt
+    thus ?thesis by (simp add: 4(2)[OF Lt])
+  next
+    case Eq
+    thus ?thesis by (simp add: 4(1)[OF Eq])
+  next
+    case Gt
+    thus ?thesis by (simp add: 4(3)[OF Gt])
+  qed
+qed
+
+lemma prod_ord_pairI:
+  assumes "oalist_inv (xs, ko)" and "oalist_inv (ys, ko)"
+    and "\<And>k. k \<in> fst ` set xs \<union> fst ` set ys \<Longrightarrow> P k (lookup_pair xs k) (lookup_pair ys k)"
+  shows "prod_ord_pair P xs ys"
+  unfolding prod_ord_pair_eq_lex_ord_pair by (rule lex_ord_pair_EqI, fact, fact, simp add: assms(3))
+
+lemma prod_ord_pairD:
+  assumes "oalist_inv (xs, ko)" and "oalist_inv (ys, ko)" and "prod_ord_pair P xs ys"
+    and "k \<in> fst ` set xs \<union> fst ` set ys"
+  shows "P k (lookup_pair xs k) (lookup_pair ys k)"
+proof -
+  from assms have "(if P k (lookup_pair xs k) (lookup_pair ys k) then Some Eq else None) = Some Eq"
+    unfolding prod_ord_pair_eq_lex_ord_pair by (rule lex_ord_pair_EqD)
+  thus ?thesis by (simp split: if_splits)
+qed
+
+corollary prod_ord_pair_alt:
+  assumes "oalist_inv (xs, ko)" and "oalist_inv (ys, ko)"
+  shows "(prod_ord_pair P xs ys) \<longleftrightarrow> (\<forall>k\<in>fst ` set xs \<union> fst ` set ys. P k (lookup_pair xs k) (lookup_pair ys k))"
+  using prod_ord_pairI[OF assms] prod_ord_pairD[OF assms] by meson
+
+subsubsection \<open>@{const sort_oalist}\<close>
+
+lemma oalist_inv_foldr_update_by_pair:
+  assumes "oalist_inv (ys, ko)"
+  shows "oalist_inv (foldr update_by_pair xs ys, ko)"
+proof (induct xs)
+  case Nil
+  from assms show ?case by simp
+next
+  case (Cons x xs)
+  hence "oalist_inv (update_by_pair x (foldr update_by_pair xs ys), ko)"
+    by (rule oalist_inv_update_by_pair)
+  thus ?case by simp
+qed
+
+corollary oalist_inv_sort_oalist: "oalist_inv (sort_oalist xs, ko)"
+proof -
+  from oalist_inv_Nil have "oalist_inv (foldr local.update_by_pair xs [], ko)"
+    by (rule oalist_inv_foldr_update_by_pair)
+  thus "oalist_inv (sort_oalist xs, ko)" by (simp only: sort_oalist_def)
+qed
+
+lemma sort_oalist_id:
+  assumes "oalist_inv (xs, ko)"
+  shows "sort_oalist xs = xs"
+proof -
+  have "foldr update_by_pair xs ys = xs @ ys" if "oalist_inv (xs @ ys, ko)" for ys using assms that
+  proof (induct xs rule: oalist_inv_induct)
+    case Nil
+    show ?case by simp
+  next
+    case (Cons k v xs)
+    from Cons(6) have *: "oalist_inv ((k, v) # (xs @ ys), ko)" by simp
+    hence 1: "oalist_inv (xs @ ys, ko)" by (rule oalist_inv_ConsD1)
+    hence 2: "foldr update_by_pair xs ys = xs @ ys" by (rule Cons(5))
+    show ?case
+    proof (simp add: 2, rule update_by_pair_less)
+      from * show "v \<noteq> 0" by (auto simp: oalist_inv_def)
+    next
+      have "key_compare ko k (fst (hd (xs @ ys))) = Lt \<or> xs @ ys = []"
+      proof (rule disjCI)
+        assume "xs @ ys \<noteq> []"
+        then obtain k'' v'' zs where eq: "xs @ ys = (k'', v'') # zs"
+          using list.exhaust prod.exhaust by metis
+        from * have "lt_of_key_order ko k k''" by (simp add: eq oalist_inv_def)
+        thus "key_compare ko k (fst (hd (xs @ ys))) = Lt" by (simp add: eq lt_of_key_order_alt)
+      qed
+      thus "xs @ ys = [] \<or> key_compare ko k (fst (hd (xs @ ys))) = Lt" by auto
+    qed
+  qed
+  with assms show ?thesis by (simp add: sort_oalist_def)
+qed
 
 end
 
-subsection \<open>Invariant\<close>
-
-definition oalist_inv :: "('a::compare \<times> 'b::zero) list \<Rightarrow> bool"
-  where "oalist_inv xs \<longleftrightarrow> (0 \<notin> snd ` set xs \<and> sorted_wrt less_of_comp (map fst xs))"
-
-lemma oalist_invI:
-  assumes "0 \<notin> snd ` set xs" and "sorted_wrt less_of_comp (map fst xs)"
-  shows "oalist_inv xs"
-  unfolding oalist_inv_def using assms by blast
-
-lemma oalist_invD1:
-  assumes "oalist_inv xs"
-  shows "0 \<notin> snd ` set xs"
-  using assms unfolding oalist_inv_def by blast
-
-lemma oalist_invD2:
-  assumes "oalist_inv xs"
-  shows "sorted_wrt less_of_comp (map fst xs)"
-  using assms unfolding oalist_inv_def by blast
-
-lemma oalist_inv_Nil: "oalist_inv []"
-  by (simp add: oalist_inv_def)
-
-lemma oalist_inv_filter:
-  assumes "oalist_inv xs"
-  shows "oalist_inv (filter P xs)"
-proof (rule oalist_invI)
-  from assms have "0 \<notin> snd ` set xs" by (rule oalist_invD1)
-  thus "0 \<notin> snd ` set (filter P xs)" by auto
-next
-  from assms have "sorted_wrt less_of_comp (map fst xs)" by (rule oalist_invD2)
-  thus "sorted_wrt less_of_comp (map fst (filter P xs))" by (induct xs, simp, simp)
+lemma set_sort_oalist:
+  assumes "oalist_inv (xs, ko1)"
+  shows "set (sort_oalist ko2 xs) = set xs"
+proof -
+  have rl: "set (foldr (update_by_pair ko2) xs ys) = set xs \<union> set ys"
+    if "oalist_inv (ys, ko2)" and "fst ` set xs \<inter> fst ` set ys = {}" for ys
+    using assms that(2)
+  proof (induct xs rule: oalist_inv_induct)
+    case Nil
+    show ?case by simp
+  next
+    case (Cons k v xs)
+    from Cons(6) have "k \<notin> fst ` set ys" and "fst ` set xs \<inter> fst ` set ys = {}" by simp_all
+    from this(2) have eq1: "set (foldr (update_by_pair ko2) xs ys) = set xs \<union> set ys" by (rule Cons(5))
+    have "\<not> lt_of_key_order ko1 k k" by auto
+    with Cons(4) have "k \<notin> fst ` set xs" by blast
+    with \<open>k \<notin> fst ` set ys\<close> have "k \<notin> fst ` (set xs \<union> set ys)" by (simp add: image_Un)
+    hence "(set xs \<union> set ys) \<inter> range (Pair k) = {}" by (smt Int_emptyI fstI image_iff)
+    hence eq2: "(set xs \<union> set ys) - range (Pair k) = set xs \<union> set ys" by (rule Diff_triv)
+    from \<open>oalist_inv (ys, ko2)\<close> have "oalist_inv (foldr (update_by_pair ko2) xs ys, ko2)"
+      by (rule oalist_inv_foldr_update_by_pair)
+    hence "set (update_by_pair ko2 (k, v) (foldr (update_by_pair ko2) xs ys)) =
+            insert (k, v) (set (foldr (update_by_pair ko2) xs ys) - range (Pair k))"
+      using Cons(3) by (rule set_update_by_pair)
+    also have "... = insert (k, v) (set xs \<union> set ys)" by (simp only: eq1 eq2)
+    finally show ?case by simp
+  qed
+  have "set (foldr (update_by_pair ko2) xs []) = set xs \<union> set []"
+    by (rule rl, fact oalist_inv_Nil, simp)
+  thus ?thesis by (simp add: sort_oalist_def)
 qed
 
-lemma map_val_raw_dom_subset: "fst ` set (map_val_raw f xs) \<subseteq> fst ` set xs"
-  by (induct xs rule: map_val_raw.induct, auto simp: Let_def)
+lemma lookup_pair_eqI:
+  assumes "oalist_inv (xs, ox)" and "oalist_inv (ys, oy)" and "set xs = set ys"
+  shows "lookup_pair ox xs = lookup_pair oy ys"
+proof
+  fix k
+  show "lookup_pair ox xs k = lookup_pair oy ys k"
+  proof (cases "lookup_pair oy ys k = 0")
+    case True
+    with assms(2) have "k \<notin> fst ` set ys" by (simp add: lookup_pair_eq_0)
+    with assms(1) show ?thesis by (simp add: True assms(3)[symmetric] lookup_pair_eq_0)
+  next
+    case False
+    define v where "v = lookup_pair oy ys k"
+    from False have "v \<noteq> 0" by (simp add: v_def)
+    with assms(2) v_def[symmetric] have "(k, v) \<in> set ys" by (simp add: lookup_pair_eq_value)
+    with assms(1) \<open>v \<noteq> 0\<close> have "lookup_pair ox xs k = v"
+      by (simp add: assms(3)[symmetric] lookup_pair_eq_value)
+    thus ?thesis by (simp only: v_def)
+  qed
+qed
+
+corollary lookup_pair_sort_oalist:
+  assumes "oalist_inv (xs, ko1)"
+  shows "lookup_pair ko2 (sort_oalist ko2 xs) = lookup_pair ko1 xs"
+  by (rule lookup_pair_eqI, rule oalist_inv_sort_oalist, fact, rule set_sort_oalist, fact)
+
+subsection \<open>Operations on Raw Ordered Associative Lists\<close>
+
+type_synonym ('a, 'b) oalist_raw = "('a \<times> 'b) list \<times> 'a key_order"
+
+fun sort_oalist_aux :: "'a key_order \<Rightarrow> ('a, 'b) oalist_raw \<Rightarrow> ('a \<times> 'b::zero) list"
+  where "sort_oalist_aux ko (xs, ox) = (if ko = ox then xs else sort_oalist ko xs)"
+
+fun lookup_raw :: "('a, 'b) oalist_raw \<Rightarrow> 'a \<Rightarrow> 'b::zero"
+  where "lookup_raw (xs, ko) = lookup_pair ko xs"
+
+definition sorted_domain_raw :: "'a key_order \<Rightarrow> ('a, 'b::zero) oalist_raw \<Rightarrow> 'a list"
+  where "sorted_domain_raw ko xs = map fst (sort_oalist_aux ko xs)"
+
+definition except_min_raw :: "'a key_order \<Rightarrow> ('a, 'b) oalist_raw \<Rightarrow> ('a, 'b::zero) oalist_raw"
+  where "except_min_raw ko xs = (List.tl (sort_oalist_aux ko xs), ko)"
+
+fun min_key_val_raw :: "'a key_order \<Rightarrow> ('a, 'b) oalist_raw \<Rightarrow> ('a \<times> 'b::zero)"
+  where "min_key_val_raw ko (xs, ox) =
+      (if ko = ox then List.hd else min_list_param (\<lambda>x y. le_of_key_order ko (fst x) (fst y))) xs"
+
+fun update_by_raw :: "('a \<times> 'b) \<Rightarrow> ('a, 'b) oalist_raw \<Rightarrow> ('a, 'b::zero) oalist_raw"
+  where "update_by_raw kv (xs, ko) = (update_by_pair ko kv xs, ko)"
+
+fun update_by_fun_raw :: "'a \<Rightarrow> ('b \<Rightarrow> 'b) \<Rightarrow> ('a, 'b) oalist_raw \<Rightarrow> ('a, 'b::zero) oalist_raw"
+  where "update_by_fun_raw k f (xs, ko) = (update_by_fun_pair ko k f xs, ko)"
+
+fun update_by_fun_gr_raw :: "'a \<Rightarrow> ('b \<Rightarrow> 'b) \<Rightarrow> ('a, 'b) oalist_raw \<Rightarrow> ('a, 'b::zero) oalist_raw"
+  where "update_by_fun_gr_raw k f (xs, ko) = (update_by_fun_gr_pair ko k f xs, ko)"
+
+fun filter_raw :: "(('a \<times> 'b) \<Rightarrow> bool) \<Rightarrow> ('a, 'b) oalist_raw \<Rightarrow> ('a, 'b::zero) oalist_raw"
+  where "filter_raw P (xs, ko) = (filter P xs, ko)"
+
+fun map_raw :: "(('a \<times> 'b) \<Rightarrow> ('a \<times> 'c)) \<Rightarrow> ('a, 'b::zero) oalist_raw \<Rightarrow> ('a, 'c::zero) oalist_raw"
+  where "map_raw f (xs, ko) = (map_pair f xs, ko)"
+
+abbreviation map_val_raw :: "('a \<Rightarrow> 'b \<Rightarrow> 'c) \<Rightarrow> ('a, 'b::zero) oalist_raw \<Rightarrow> ('a, 'c::zero) oalist_raw"
+  where "map_val_raw f \<equiv> map_raw (\<lambda>(k, v). (k, f k v))"
+
+fun map2_val_raw :: "('a \<Rightarrow> 'b \<Rightarrow> 'c \<Rightarrow> 'd) \<Rightarrow> (('a, 'b) oalist_raw \<Rightarrow> ('a, 'd) oalist_raw) \<Rightarrow>
+                      (('a, 'c) oalist_raw \<Rightarrow> ('a, 'd) oalist_raw) \<Rightarrow>
+                      ('a, 'b::zero) oalist_raw \<Rightarrow> ('a, 'c::zero) oalist_raw \<Rightarrow>
+                      ('a, 'd::zero) oalist_raw"
+  where "map2_val_raw f g h (xs, ox) ys =
+            (map2_val_pair ox f (\<lambda>ko zs. fst (g (zs, ko))) (\<lambda>ko zs. fst (h (zs, ko)))
+                    xs (sort_oalist_aux ox ys), ox)"
+
+definition lex_ord_raw :: "('a key_order) \<Rightarrow> ('a \<Rightarrow> (('b, 'c) comp_opt)) \<Rightarrow>
+                      (('a, 'b::zero) oalist_raw, ('a, 'c::zero) oalist_raw) comp_opt"
+  where "lex_ord_raw ko f xs ys = lex_ord_pair ko f (sort_oalist_aux ko xs) (sort_oalist_aux ko ys)"
+
+fun prod_ord_raw :: "('a \<Rightarrow> 'b \<Rightarrow> 'c \<Rightarrow> bool) \<Rightarrow> ('a, 'b::zero) oalist_raw \<Rightarrow>
+                      ('a, 'c::zero) oalist_raw \<Rightarrow> bool"
+  where "prod_ord_raw f (xs, ox) ys = prod_ord_pair ox f xs (sort_oalist_aux ox ys)"
+
+fun oalist_eq_raw :: "('a, 'b) oalist_raw \<Rightarrow> ('a, 'b::zero) oalist_raw \<Rightarrow> bool"
+  where "oalist_eq_raw (xs, ox) ys = (xs = (sort_oalist_aux ox ys))"
+
+fun sort_oalist_raw :: "('a, 'b) oalist_raw \<Rightarrow> ('a, 'b::zero) oalist_raw"
+  where "sort_oalist_raw (xs, ko) = (sort_oalist ko xs, ko)"
+
+subsubsection \<open>@{const sort_oalist_aux}\<close>
+
+lemma set_sort_oalist_aux:
+  assumes "oalist_inv xs"
+  shows "set (sort_oalist_aux ko xs) = set (fst xs)"
+proof -
+  obtain xs' ko' where xs: "xs = (xs', ko')" by fastforce
+  from assms show ?thesis by (simp add: xs set_sort_oalist)
+qed
+
+lemma oalist_inv_sort_oalist_aux:
+  assumes "oalist_inv xs"
+  shows "oalist_inv (sort_oalist_aux ko xs, ko)"
+proof -
+  obtain xs' ko' where xs: "xs = (xs', ko')" by fastforce
+  from assms show ?thesis by (simp add: xs oalist_inv_sort_oalist)
+qed
+
+lemma lookup_pair_sort_oalist_aux:
+  assumes "oalist_inv xs"
+  shows "lookup_pair ko (sort_oalist_aux ko xs) = lookup_raw xs"
+proof -
+  obtain xs' ko' where xs: "xs = (xs', ko')" by fastforce
+  from assms show ?thesis by (simp add: xs lookup_pair_sort_oalist)
+qed
+
+subsubsection \<open>@{const lookup_raw}\<close>
+
+lemma lookup_raw_inj:
+  assumes "oalist_inv (xs, ko)" and "oalist_inv (ys, ko)" and "lookup_raw (xs, ko) = lookup_raw (ys, ko)"
+  shows "xs = ys"
+  using assms unfolding lookup_raw.simps by (rule lookup_pair_inj)
+
+subsubsection \<open>@{const sorted_domain_raw}\<close>
+
+lemma set_sorted_domain_raw:
+  assumes "oalist_inv xs"
+  shows "set (sorted_domain_raw ko xs) = fst ` set (fst xs)"
+  using assms by (simp add: sorted_domain_raw_def set_sort_oalist_aux)
+
+corollary in_sorted_domain_raw_iff_lookup_raw:
+  assumes "oalist_inv xs"
+  shows "k \<in> set (sorted_domain_raw ko xs) \<longleftrightarrow> (lookup_raw xs k \<noteq> 0)"
+  unfolding set_sorted_domain_raw[OF assms]
+proof -
+  obtain xs' ko' where xs: "xs = (xs', ko')" by fastforce
+  from assms show "k \<in> fst ` set (fst xs) \<longleftrightarrow> (lookup_raw xs k \<noteq> 0)"
+    by (simp add: xs lookup_pair_eq_0)
+qed
+
+lemma sorted_sorted_domain_raw:
+  assumes "oalist_inv xs"
+  shows "sorted_wrt (lt_of_key_order ko) (sorted_domain_raw ko xs)"
+  unfolding sorted_domain_raw_def by (rule oalist_invD2, rule oalist_inv_sort_oalist_aux, fact)
+
+subsubsection \<open>@{const except_min_raw}\<close>
+
+lemma oalist_inv_except_min_raw:
+  assumes "oalist_inv xs"
+  shows "oalist_inv (except_min_raw ko xs)"
+  unfolding except_min_raw_def by (rule oalist_inv_tl, rule oalist_inv_sort_oalist_aux, fact)
+
+lemma lookup_raw_except_min_raw:
+  assumes "oalist_inv xs"
+  shows "lookup_raw (except_min_raw ko xs) k =
+          (if (\<forall>k'\<in>fst ` set (fst xs). le_of_key_order ko k k') then 0 else lookup_raw xs k)"
+  using assms by (simp add: except_min_raw_def lookup_pair_tl oalist_inv_sort_oalist_aux
+      lookup_pair_sort_oalist_aux  set_sort_oalist_aux split del: if_split cong: if_cong)
+
+subsubsection \<open>@{const min_key_val_raw}\<close>
+
+lemma min_key_val_raw_in:
+  assumes "fst xs \<noteq> []"
+  shows "min_key_val_raw ko xs \<in> set (fst xs)"
+proof -
+  obtain xs' ox where xs: "xs = (xs', ox)" by fastforce
+  from assms have "xs' \<noteq> []" by (simp add: xs)
+  show ?thesis unfolding xs
+  proof (simp, intro conjI impI)
+    from \<open>xs' \<noteq> []\<close> show "hd xs' \<in> set xs'" by simp
+  next
+    from \<open>xs' \<noteq> []\<close> show "min_list_param (\<lambda>x y. le_of_key_order ko (fst x) (fst y)) xs' \<in> set xs'"
+      by (rule min_list_param_in)
+  qed
+qed
+
+lemma snd_min_key_val_raw:
+  assumes "oalist_inv xs" and "fst xs \<noteq> []"
+  shows "snd (min_key_val_raw ko xs) = lookup_raw xs (fst (min_key_val_raw ko xs))"
+proof -
+  obtain xs' ox where xs: "xs = (xs', ox)" by fastforce
+  from assms(1) have "oalist_inv (xs', ox)" by (simp only: xs)
+  from assms(2) have "min_key_val_raw ko xs \<in> set (fst xs)" by (rule min_key_val_raw_in)
+  hence *: "min_key_val_raw ko (xs', ox) \<in> set xs'" by (simp add: xs)
+  show ?thesis unfolding xs lookup_raw.simps
+    by (rule sym, rule lookup_pair_eq_valueI, fact, simp add: * del: min_key_val_raw.simps)
+qed
+
+lemma min_key_val_raw_minimal:
+  assumes "oalist_inv xs" and "z \<in> set (fst xs)"
+  shows "le_of_key_order ko (fst (min_key_val_raw ko xs)) (fst z)"
+proof -
+  obtain xs' ox where xs: "xs = (xs', ox)" by fastforce
+  from assms have "oalist_inv (xs', ox)" and "z \<in> set xs'" by (simp_all add: xs)
+  show ?thesis unfolding xs
+  proof (simp, intro conjI impI)
+    from \<open>z \<in> set xs'\<close> have "xs' \<noteq> []" by auto
+    then obtain k v ys where xs': "xs' = (k, v) # ys" using prod.exhaust list.exhaust by metis
+    from \<open>z \<in> set xs'\<close> have "z = (k, v) \<or> z \<in> set ys" by (simp add: xs')
+    thus "le_of_key_order ox (fst (hd xs')) (fst z)"
+    proof
+      assume "z = (k, v)"
+      show ?thesis by (simp add: xs' \<open>z = (k, v)\<close>)
+    next
+      assume "z \<in> set ys"
+      hence "fst z \<in> fst ` set ys" by fastforce
+      with \<open>oalist_inv (xs', ox)\<close>[simplified xs'] have "lt_of_key_order ox k (fst z)" by (rule oalist_inv_ConsD3)
+      thus ?thesis by (simp add: xs')
+    qed
+  next
+    show "le_of_key_order ko (fst (min_list_param (\<lambda>x y. le_of_key_order ko (fst x) (fst y)) xs')) (fst z)"
+    proof (rule min_list_param_minimal[of "\<lambda>x y. le_of_key_order ko (fst x) (fst y)"])
+      show "transp (\<lambda>x y. le_of_key_order ko (fst x) (fst y))"
+        by (metis (no_types, lifting) key_order_lin.order.trans transpI)
+    qed (auto intro: \<open>z \<in> set xs'\<close>)
+  qed
+qed
+
+subsubsection \<open>@{const filter_raw}\<close>
+
+lemma oalist_inv_filter_raw:
+  assumes "oalist_inv xs"
+  shows "oalist_inv (filter_raw P xs)"
+proof -
+  obtain xs' ko where xs: "xs = (xs', ko)" by fastforce
+  from assms show ?thesis unfolding xs filter_raw.simps by (rule oalist_inv_filter)
+qed
+
+lemma lookup_raw_filter_raw:
+  assumes "oalist_inv xs"
+  shows "lookup_raw (filter_raw P xs) k = (let v = lookup_raw xs k in if P (k, v) then v else 0)"
+proof -
+  obtain xs' ko where xs: "xs = (xs', ko)" by fastforce
+  from assms show ?thesis unfolding xs lookup_raw.simps filter_raw.simps by (rule lookup_pair_filter)
+qed
+
+subsubsection \<open>@{const update_by_raw}\<close>
+
+lemma oalist_inv_update_by_raw:
+  assumes "oalist_inv xs"
+  shows "oalist_inv (update_by_raw kv xs)"
+proof -
+  obtain xs' ko where xs: "xs = (xs', ko)" by fastforce
+  from assms show ?thesis unfolding xs update_by_raw.simps by (rule oalist_inv_update_by_pair)
+qed
+
+lemma lookup_raw_update_by_raw:
+  assumes "oalist_inv xs"
+  shows "lookup_raw (update_by_raw (k1, v) xs) k2 = (if k1 = k2 then v else lookup_raw xs k2)"
+proof -
+  obtain xs' ko where xs: "xs = (xs', ko)" by fastforce
+  from assms show ?thesis unfolding xs lookup_raw.simps update_by_raw.simps by (rule lookup_pair_update_by_pair)
+qed
+
+subsubsection \<open>@{const update_by_fun_raw} and @{const update_by_fun_gr_raw}\<close>
+
+lemma update_by_fun_raw_eq_update_by_raw:
+  assumes "oalist_inv xs"
+  shows "update_by_fun_raw k f xs = update_by_raw (k, f (lookup_raw xs k)) xs"
+proof -
+  obtain xs' ko where xs: "xs = (xs', ko)" by fastforce
+  from assms have "oalist_inv (xs', ko)" by (simp only: xs)
+  show ?thesis unfolding xs update_by_fun_raw.simps lookup_raw.simps update_by_raw.simps
+    by (rule, rule conjI, rule update_by_fun_pair_eq_update_by_pair, fact, fact refl)
+qed
+
+corollary oalist_inv_update_by_fun_raw:
+  assumes "oalist_inv xs"
+  shows "oalist_inv (update_by_fun_raw k f xs)"
+  unfolding update_by_fun_raw_eq_update_by_raw[OF assms] using assms by (rule oalist_inv_update_by_raw)
+
+corollary lookup_raw_update_by_fun_raw:
+  assumes "oalist_inv xs"
+  shows "lookup_raw (update_by_fun_raw k1 f xs) k2 = (if k1 = k2 then f else id) (lookup_raw xs k2)"
+  using assms by (simp add: update_by_fun_raw_eq_update_by_raw lookup_raw_update_by_raw)
+
+lemma update_by_fun_gr_raw_eq_update_by_fun_raw:
+  assumes "oalist_inv xs"
+  shows "update_by_fun_gr_raw k f xs = update_by_fun_raw k f xs"
+proof -
+  obtain xs' ko where xs: "xs = (xs', ko)" by fastforce
+  from assms have "oalist_inv (xs', ko)" by (simp only: xs)
+  show ?thesis unfolding xs update_by_fun_raw.simps lookup_raw.simps update_by_fun_gr_raw.simps
+    by (rule, rule conjI, rule update_by_fun_gr_pair_eq_update_by_fun_pair, fact, fact refl)
+qed
+
+corollary oalist_inv_update_by_fun_gr_raw:
+  assumes "oalist_inv xs"
+  shows "oalist_inv (update_by_fun_gr_raw k f xs)"
+  unfolding update_by_fun_gr_raw_eq_update_by_fun_raw[OF assms] using assms by (rule oalist_inv_update_by_fun_raw)
+
+corollary lookup_raw_update_by_fun_gr_raw:
+  assumes "oalist_inv xs"
+  shows "lookup_raw (update_by_fun_gr_raw k1 f xs) k2 = (if k1 = k2 then f else id) (lookup_raw xs k2)"
+  using assms by (simp add: update_by_fun_gr_raw_eq_update_by_fun_raw lookup_raw_update_by_fun_raw)
+
+subsubsection \<open>@{const map_raw} and @{const map_val_raw}\<close>
+
+lemma oalist_inv_map_raw:
+  assumes "oalist_inv xs"
+    and "\<And>a b. key_compare (snd xs) (fst (f a)) (fst (f b)) = key_compare (snd xs) (fst a) (fst b)"
+  shows "oalist_inv (map_raw f xs)"
+proof -
+  obtain xs' ko where xs: "xs = (xs', ko)" by fastforce
+  from assms(1) have "oalist_inv (xs', ko)" by (simp only: xs)
+  moreover from assms(2) have "\<And>a b. key_compare ko (fst (f a)) (fst (f b)) = key_compare ko (fst a) (fst b)"
+    by (simp add: xs)
+  ultimately show ?thesis unfolding xs map_raw.simps by (rule oalist_inv_map_pair)
+qed
+
+lemma lookup_raw_map_raw:
+  assumes "oalist_inv xs"
+    and "\<And>k'. snd (f (k', 0)) = 0"
+    and "\<And>a b. key_compare (snd xs) (fst (f a)) (fst (f b)) = key_compare (snd xs) (fst a) (fst b)"
+  shows "lookup_raw (map_raw f xs) (fst (f (k, v))) = snd (f (k, lookup_raw xs k))"
+proof -
+  obtain xs' ko where xs: "xs = (xs', ko)" by fastforce
+  from assms(1) have "oalist_inv (xs', ko)" by (simp only: xs)
+  moreover note assms(2)
+  moreover from assms(3) have "\<And>a b. key_compare ko (fst (f a)) (fst (f b)) = key_compare ko (fst a) (fst b)"
+    by (simp add: xs)
+  ultimately show ?thesis unfolding xs lookup_raw.simps map_raw.simps by (rule lookup_pair_map_pair)
+qed
+
+lemma map_raw_id:
+  assumes "oalist_inv xs"
+  shows "map_raw id xs = xs"
+proof -
+  obtain xs' ko where xs: "xs = (xs', ko)" by fastforce
+  from assms have "oalist_inv (xs', ko)" by (simp only: xs)
+  hence "map_pair id xs' = xs'"
+  proof (induct xs' rule: oalist_inv_induct)
+    case Nil
+    show ?case by simp
+  next
+    case (Cons k v xs')
+    show ?case by (simp add: Let_def Cons(3, 5) id_def[symmetric])
+  qed
+  thus ?thesis by (simp add: xs)
+qed
 
 lemma oalist_inv_map_val_raw:
   assumes "oalist_inv xs"
   shows "oalist_inv (map_val_raw f xs)"
-proof (rule oalist_invI)
-  show "0 \<notin> snd ` set (map_val_raw f xs)"
-    by (induct xs rule: map_val_raw.induct, simp, simp add: Let_def)
-next
-  from assms have "sorted_wrt less_of_comp (map fst xs)" by (rule oalist_invD2)
-  thus "sorted_wrt less_of_comp (map fst (map_val_raw f xs))"
-  proof (induct xs rule: map_val_raw.induct)
-    case (1 f)
-    show ?case by simp
-  next
-    case (2 f kx vx xs)
-    from 2(2) have 1: "sorted_wrt less_of_comp (kx # (map fst xs))" by simp
-    hence 3: "\<forall>y \<in> fst ` set xs. less_of_comp kx y" and "sorted_wrt less_of_comp (map fst xs)"
-      by simp_all
-    from refl this(2) have 2: "sorted_wrt less_of_comp (map fst (map_val_raw f xs))" by (rule 2(1))
-    show ?case
-    proof (simp add: Let_def 2, intro impI ballI)
-      fix y
-      assume "y \<in> set (map_val_raw f xs)"
-      hence "fst y \<in> fst ` set (map_val_raw f xs)" by simp
-      also have "... \<subseteq> fst ` set xs" by (fact map_val_raw_dom_subset)
-      finally have "fst y \<in> fst ` set xs" .
-      with 3 show "less_of_comp kx (fst y)" ..
-    qed
-  qed
-qed
-
-subsection \<open>Sorting Associative Lists\<close>
-
-definition sort_alist :: "('a \<times> 'b) list \<Rightarrow> ('a::compare \<times> 'b::zero) list"
-  where "sort_alist xs = foldr update_by' xs []"
-
-lemma oalist_inv_sort_alist: "oalist_inv (sort_alist xs)"
-  unfolding oalist_inv_def
-proof
-  have "0 \<notin> snd ` set (foldr update_by' xs ys)" if "0 \<notin> snd ` set ys" for ys using that
-  proof (induct xs)
-    case Nil
-    thus ?case by simp
-  next
-    case (Cons x xs)
-    from Cons(2) have "0 \<notin> snd ` set (foldr update_by' xs ys)" by (rule Cons(1))
-    hence "0 \<notin> snd ` set (update_by' x (foldr update_by' xs ys))" by (rule update_by'_not_zero)
-    thus ?case by simp
-  qed
-  thus "0 \<notin> snd ` set (sort_alist xs)" by (simp add: sort_alist_def)
-next
-  have "sorted_wrt less_of_comp (map fst (foldr update_by' xs ys))"
-    if "sorted_wrt less_of_comp (map fst ys)" for ys using that
-  proof (induct xs)
-    case Nil
-    thus ?case by simp
-  next
-    case (Cons x xs)
-    from Cons(2) have "sorted_wrt less_of_comp (map fst (foldr update_by' xs ys))" by (rule Cons(1))
-    hence "sorted_wrt less_of_comp (map fst (update_by' x (foldr update_by' xs ys)))"
-      by (rule update_by'_sorted)
-    thus ?case by simp
-  qed
-  thus "sorted_wrt less_of_comp (map fst (sort_alist xs))" by (simp add: sort_alist_def)
-qed
-
-lemma sort_alist_id:
-  assumes "oalist_inv xs"
-  shows "sort_alist xs = xs"
 proof -
-  have "foldr update_by' xs ys = xs @ ys" if "oalist_inv (xs @ ys)" for ys using that
-  proof (induct xs)
-    case Nil
-    show ?case by simp
+  obtain xs' ko where xs: "xs = (xs', ko)" by fastforce
+  from assms show ?thesis unfolding xs map_raw.simps by (rule oalist_inv_map_val_pair)
+qed
+
+lemma lookup_raw_map_val_raw:
+  assumes "oalist_inv xs" and "\<And>k'. f k' 0 = 0"
+  shows "lookup_raw (map_val_raw f xs) k = f k (lookup_raw xs k)"
+proof -
+  obtain xs' ko where xs: "xs = (xs', ko)" by fastforce
+  from assms show ?thesis unfolding xs map_raw.simps lookup_raw.simps by (rule lookup_pair_map_val_pair)
+qed
+
+subsubsection \<open>@{const map2_val_raw}\<close>
+
+definition map2_val_compat' :: "(('a, 'b::zero) oalist_raw \<Rightarrow> ('a, 'c::zero) oalist_raw) \<Rightarrow> bool"
+  where "map2_val_compat' f \<longleftrightarrow>
+      (\<forall>zs. (oalist_inv zs \<longrightarrow> (oalist_inv (f zs) \<and> snd (f zs) = snd zs \<and> fst ` set (fst (f zs)) \<subseteq> fst ` set (fst zs))))"
+
+lemma map2_val_compat'I:
+  assumes "\<And>zs. oalist_inv zs \<Longrightarrow> oalist_inv (f zs)"
+    and "\<And>zs. oalist_inv zs \<Longrightarrow> snd (f zs) = snd zs"
+    and "\<And>zs. oalist_inv zs \<Longrightarrow> fst ` set (fst (f zs)) \<subseteq> fst ` set (fst zs)"
+  shows "map2_val_compat' f"
+  unfolding map2_val_compat'_def using assms by blast
+
+lemma map2_val_compat'D1:
+  assumes "map2_val_compat' f" and "oalist_inv zs"
+  shows "oalist_inv (f zs)"
+  using assms unfolding map2_val_compat'_def by blast
+
+lemma map2_val_compat'D2:
+  assumes "map2_val_compat' f" and "oalist_inv zs"
+  shows "snd (f zs) = snd zs"
+  using assms unfolding map2_val_compat'_def by blast
+
+lemma map2_val_compat'D3:
+  assumes "map2_val_compat' f" and "oalist_inv zs"
+  shows "fst ` set (fst (f zs)) \<subseteq> fst ` set (fst zs)"
+  using assms unfolding map2_val_compat'_def by blast
+
+lemma map2_val_compat'_map_val_raw: "map2_val_compat' (map_val_raw f)"
+proof (rule map2_val_compat'I, erule oalist_inv_map_val_raw)
+  fix zs::"('a, 'b) oalist_raw"
+  obtain zs' ko where "zs = (zs', ko)" by fastforce
+  thus "snd (map_val_raw f zs) = snd zs" by simp
+next
+  fix zs::"('a, 'b) oalist_raw"
+  obtain zs' ko where zs: "zs = (zs', ko)" by fastforce
+  show "fst ` set (fst (map_val_raw f zs)) \<subseteq> fst ` set (fst zs)"
+  proof (simp add: zs)
+    from map_pair_subset have "fst ` set (map_val_pair f zs') \<subseteq> fst ` (\<lambda>(k, v). (k, f k v)) ` set zs'"
+      by (rule image_mono)
+    also have "... = fst ` set zs'" by force
+    finally show "fst ` set (map_val_pair f zs') \<subseteq> fst ` set zs'" .
+  qed
+qed
+
+lemma map2_val_compat'_id: "map2_val_compat' id"
+  by (rule map2_val_compat'I, auto)
+
+lemma map2_val_compat'_imp_map2_val_compat:
+  assumes "map2_val_compat' g"
+  shows "map2_val_compat ko (\<lambda>ko zs. fst (g (zs, ko)))"
+proof (rule map2_val_compatI)
+  fix zs::"('a \<times> 'b) list"
+  assume a: "oalist_inv (zs, ko)"
+  with assms have "oalist_inv (g (zs, ko))" by (rule map2_val_compat'D1)
+  hence "oalist_inv (fst (g (zs, ko)), snd (g (zs, ko)))" by simp
+  thus "oalist_inv (fst (g (zs, ko)), ko)" using assms a by (simp add: map2_val_compat'D2)
+next
+  fix zs::"('a \<times> 'b) list"
+  assume a: "oalist_inv (zs, ko)"
+  with assms have "fst ` set (fst (g (zs, ko))) \<subseteq> fst ` set (fst (zs, ko))" by (rule map2_val_compat'D3)
+  thus "fst ` set (fst (g (zs, ko))) \<subseteq> fst ` set zs" by simp
+qed
+
+lemma oalist_inv_map2_val_raw:
+  assumes "oalist_inv xs" and "oalist_inv ys"
+  assumes "map2_val_compat' g" and "map2_val_compat' h"
+  shows "oalist_inv (map2_val_raw f g h xs ys)"
+proof -
+  obtain xs' ox where xs: "xs = (xs', ox)" by fastforce
+  let ?ys = "sort_oalist_aux ox ys"
+  from assms(1) have "oalist_inv (xs', ox)" by (simp add: xs)
+  moreover from assms(2) have "oalist_inv (sort_oalist_aux ox ys, ox)" by (rule oalist_inv_sort_oalist_aux)
+  moreover from assms(3) have "map2_val_compat ko (\<lambda>ko zs. fst (g (zs, ko)))" for ko
+    by (rule map2_val_compat'_imp_map2_val_compat)
+  moreover from assms(4) have "map2_val_compat ko (\<lambda>ko zs. fst (h (zs, ko)))" for ko
+    by (rule map2_val_compat'_imp_map2_val_compat)
+  ultimately have "oalist_inv (map2_val_pair ox f (\<lambda>ko zs. fst (g (zs, ko))) (\<lambda>ko zs. fst (h (zs, ko))) xs' ?ys, ox)"
+    by (rule oalist_inv_map2_val_pair)
+  thus ?thesis by (simp add: xs)
+qed
+
+lemma lookup_raw_map2_val_raw:
+  assumes "oalist_inv xs" and "oalist_inv ys"
+  assumes "map2_val_compat' g" and "map2_val_compat' h"
+  assumes "\<And>zs. oalist_inv zs \<Longrightarrow> g zs = map_val_raw (\<lambda>k v. f k v 0) zs"
+    and "\<And>zs. oalist_inv zs \<Longrightarrow> h zs = map_val_raw (\<lambda>k. f k 0) zs"
+    and "\<And>k. f k 0 0 = 0"
+  shows "lookup_raw (map2_val_raw f g h xs ys) k0 = f k0 (lookup_raw xs k0) (lookup_raw ys k0)"
+proof -
+  obtain xs' ox where xs: "xs = (xs', ox)" by fastforce
+  let ?ys = "sort_oalist_aux ox ys"
+  from assms(1) have "oalist_inv (xs', ox)" by (simp add: xs)
+  moreover from assms(2) have "oalist_inv (sort_oalist_aux ox ys, ox)" by (rule oalist_inv_sort_oalist_aux)
+  moreover from assms(3) have "map2_val_compat ko (\<lambda>ko zs. fst (g (zs, ko)))" for ko
+    by (rule map2_val_compat'_imp_map2_val_compat)
+  moreover from assms(4) have "map2_val_compat ko (\<lambda>ko zs. fst (h (zs, ko)))" for ko
+    by (rule map2_val_compat'_imp_map2_val_compat)
+  ultimately have "lookup_pair ox (map2_val_pair ox f (\<lambda>ko zs. fst (g (zs, ko))) (\<lambda>ko zs. fst (h (zs, ko))) xs' ?ys) k0 =
+                      f k0 (lookup_pair ox xs' k0) (lookup_pair ox ?ys k0)" using _ _ assms(7)
+  proof (rule lookup_pair_map2_val_pair)
+    fix zs::"('a \<times> 'b) list"
+    assume "oalist_inv (zs, ox)"
+    hence "g (zs, ox) = map_val_raw (\<lambda>k v. f k v 0) (zs, ox)" by (rule assms(5))
+    thus "fst (g (zs, ox)) = map_val_pair (\<lambda>k v. f k v 0) zs" by simp
   next
-    case (Cons x xs)
-    obtain k v where x: "x = (k, v)" by fastforce
-    from Cons(2) have *: "oalist_inv ((k, v) # (xs @ ys))" by (simp add: x)
-    hence 1: "oalist_inv (xs @ ys)" by (simp add: oalist_inv_def)
-    hence 2: "foldr update_by' xs ys = xs @ ys" by (rule Cons(1))
-    show ?case
-    proof (simp add: 2 x, rule update_by'_eq_Cons)
-      from * show "v \<noteq> 0" by (simp add: oalist_inv_def)
+    fix zs::"('a \<times> 'c) list"
+    assume "oalist_inv (zs, ox)"
+    hence "h (zs, ox) = map_val_raw (\<lambda>k. f k 0) (zs, ox)" by (rule assms(6))
+    thus "fst (h (zs, ox)) = map_val_pair (\<lambda>k. f k 0) zs" by simp
+  qed
+  also from assms(2) have "... = f k0 (lookup_pair ox xs' k0) (lookup_raw ys k0)"
+    by (simp only: lookup_pair_sort_oalist_aux)
+  finally have *: "lookup_pair ox (map2_val_pair ox f (\<lambda>ko zs. fst (g (zs, ko))) (\<lambda>ko zs. fst (h (zs, ko))) xs' ?ys) k0 =
+                    f k0 (lookup_pair ox xs' k0) (lookup_raw ys k0)" .
+  thus ?thesis by (simp add: xs)
+qed
+
+lemma map2_val_raw_singleton_eq_update_by_fun_raw:
+  assumes "oalist_inv xs"
+  assumes "\<And>k x. f k x 0 = x" and "\<And>zs. oalist_inv zs \<Longrightarrow> g zs = zs"
+    and "\<And>ko. h ([(k, v)], ko) = map_val_raw (\<lambda>k. f k 0) ([(k, v)], ko)"
+  shows "map2_val_raw f g h xs ([(k, v)], ko) = update_by_fun_raw k (\<lambda>x. f k x v) xs"
+proof -
+  obtain xs' ox where xs: "xs = (xs', ox)" by fastforce
+  let ?ys = "sort_oalist ox [(k, v)]"
+  from assms(1) have inv: "oalist_inv (xs', ox)" by (simp add: xs)
+  show ?thesis
+  proof (simp add: xs, intro conjI impI)
+    assume "ox = ko"
+    from inv have "oalist_inv (xs', ko)" by (simp only: \<open>ox = ko\<close>)
+    thus "map2_val_pair ko f (\<lambda>ko zs. fst (g (zs, ko))) (\<lambda>ko zs. fst (h (zs, ko))) xs' [(k, v)] =
+              update_by_fun_pair ko k (\<lambda>x. f k x v) xs'"
+      using assms(2)
+    proof (rule map2_val_pair_singleton_eq_update_by_fun_pair)
+      fix zs::"('a \<times> 'b) list"
+      assume "oalist_inv (zs, ko)"
+      hence "g (zs, ko) = (zs, ko)" by (rule assms(3))
+      thus "fst (g (zs, ko)) = zs" by simp
     next
-      have "compare_class.compare k (fst (hd (xs @ ys))) = LESS \<or> xs @ ys = []"
-      proof (rule disjCI)
-        assume "xs @ ys \<noteq> []"
-        then obtain k'' v'' zs where eq: "xs @ ys = (k'', v'') # zs"
-          by (meson c.update_by.cases)
-        from * have "less_of_comp k k''" by (simp add: eq oalist_inv_def)
-        thus "compare_class.compare k (fst (hd (xs @ ys))) = LESS" by (simp add: eq less_of_comp_alt)
+      show "fst (h ([(k, v)], ko)) = map_val_pair (\<lambda>k. f k 0) [(k, v)]" by (simp add: assms(4))
+    qed
+  next
+    show "map2_val_pair ox f (\<lambda>ko zs. fst (g (zs, ko))) (\<lambda>ko zs. fst (h (zs, ko))) xs' (sort_oalist ox [(k, v)]) =
+          update_by_fun_pair ox k (\<lambda>x. f k x v) xs'"
+    proof (cases "v = 0")
+      case True
+      have eq1: "sort_oalist ox [(k, 0)] = []" by (simp add: sort_oalist_def)
+      from inv have eq2: "g (xs', ox) = (xs', ox)" by (rule assms(3))
+      show ?thesis
+        by (simp add: True eq1 eq2 assms(2) update_by_fun_pair_eq_update_by_pair[OF inv],
+            rule sym, rule update_by_pair_id, fact inv, fact refl)
+    next
+      case False
+      hence "oalist_inv ([(k, v)], ox)" by (simp add: oalist_inv_singleton)
+      hence eq: "sort_oalist ox [(k, v)] = [(k, v)]" by (rule sort_oalist_id)
+      show ?thesis unfolding eq using inv assms(2)
+      proof (rule map2_val_pair_singleton_eq_update_by_fun_pair)
+        fix zs::"('a \<times> 'b) list"
+        assume "oalist_inv (zs, ox)"
+        hence "g (zs, ox) = (zs, ox)" by (rule assms(3))
+        thus "fst (g (zs, ox)) = zs" by simp
+      next
+        show "fst (h ([(k, v)], ox)) = map_val_pair (\<lambda>k. f k 0) [(k, v)]" by (simp add: assms(4))
       qed
-      thus "xs @ ys = [] \<or> compare_class.compare k (fst (hd (xs @ ys))) = LESS" by auto
     qed
   qed
-  with assms show ?thesis by (simp add: sort_alist_def)
+qed
+
+subsubsection \<open>@{const lex_ord_raw}\<close>
+
+lemma lex_ord_raw_EqI:
+  assumes "oalist_inv xs" and "oalist_inv ys"
+    and "\<And>k. k \<in> fst ` set (fst xs) \<union> fst ` set (fst ys) \<Longrightarrow> f k (lookup_raw xs k) (lookup_raw ys k) = Some Eq"
+  shows "lex_ord_raw ko f xs ys = Some Eq"
+  unfolding lex_ord_raw_def
+  by (rule lex_ord_pair_EqI, simp_all add: assms oalist_inv_sort_oalist_aux lookup_pair_sort_oalist_aux set_sort_oalist_aux)
+
+lemma lex_ord_raw_valI:
+  assumes "oalist_inv xs" and "oalist_inv ys" and "aux \<noteq> Some Eq"
+  assumes "k \<in> fst ` set (fst xs) \<union> fst ` set (fst ys)" and "aux = f k (lookup_raw xs k) (lookup_raw ys k)"
+    and "\<And>k'. k' \<in> fst ` set (fst xs) \<union> fst ` set (fst ys) \<Longrightarrow> lt_of_key_order ko k' k \<Longrightarrow>
+              f k' (lookup_raw xs k') (lookup_raw ys k') = Some Eq"
+  shows "lex_ord_raw ko f xs ys = aux"
+  unfolding lex_ord_raw_def
+  using oalist_inv_sort_oalist_aux[OF assms(1)] oalist_inv_sort_oalist_aux[OF assms(2)] assms(3)
+proof (rule lex_ord_pair_valI)
+  from assms(1, 2, 4) show "k \<in> fst ` set (sort_oalist_aux ko xs) \<union> fst ` set (sort_oalist_aux ko ys)"
+    by (simp add: set_sort_oalist_aux)
+next
+  from assms(1, 2, 5) show "aux = f k (lookup_pair ko (sort_oalist_aux ko xs) k) (lookup_pair ko (sort_oalist_aux ko ys) k)"
+    by (simp add: lookup_pair_sort_oalist_aux)
+next
+  fix k'
+  assume "k' \<in> fst ` set (sort_oalist_aux ko xs) \<union> fst ` set (sort_oalist_aux ko ys)"
+  with assms(1, 2) have "k' \<in> fst ` set (fst xs) \<union> fst ` set (fst ys)" by (simp add: set_sort_oalist_aux)
+  moreover assume "lt_of_key_order ko k' k"
+  ultimately have "f k' (lookup_raw xs k') (lookup_raw ys k') = Some Eq" by (rule assms(6))
+  with assms(1, 2) show "f k' (lookup_pair ko (sort_oalist_aux ko xs) k') (lookup_pair ko (sort_oalist_aux ko ys) k') = Some Eq"
+    by (simp add: lookup_pair_sort_oalist_aux)
+qed
+
+lemma lex_ord_raw_EqD:
+  assumes "oalist_inv xs" and "oalist_inv ys" and "lex_ord_raw ko f xs ys = Some Eq"
+    and "k \<in> fst ` set (fst xs) \<union> fst ` set (fst ys)"
+  shows "f k (lookup_raw xs k) (lookup_raw ys k) = Some Eq"
+proof -
+  have "f k (lookup_pair ko (sort_oalist_aux ko xs) k) (lookup_pair ko (sort_oalist_aux ko ys) k) = Some Eq"
+    by (rule lex_ord_pair_EqD[where f=f],
+        simp_all add: oalist_inv_sort_oalist_aux assms lex_ord_raw_def[symmetric] set_sort_oalist_aux del: Un_iff)
+  with assms(1, 2) show ?thesis by (simp add: lookup_pair_sort_oalist_aux)
+qed
+
+lemma lex_ord_raw_valE:
+  assumes "oalist_inv xs" and "oalist_inv ys" and "lex_ord_raw ko f xs ys = aux"
+    and "aux \<noteq> Some Eq"
+  obtains k where "k \<in> fst ` set (fst xs) \<union> fst ` set (fst ys)"
+    and "aux = f k (lookup_raw xs k) (lookup_raw ys k)"
+    and "\<And>k'. k' \<in> fst ` set (fst xs) \<union> fst ` set (fst ys) \<Longrightarrow> lt_of_key_order ko k' k \<Longrightarrow>
+            f k' (lookup_raw xs k') (lookup_raw ys k') = Some Eq"
+proof -
+  let ?xs = "sort_oalist_aux ko xs"
+  let ?ys = "sort_oalist_aux ko ys"
+  from assms(3) have "lex_ord_pair ko f ?xs ?ys = aux" by (simp only: lex_ord_raw_def)
+  with oalist_inv_sort_oalist_aux[OF assms(1)] oalist_inv_sort_oalist_aux[OF assms(2)]
+  obtain k where a: "k \<in> fst ` set ?xs \<union> fst ` set ?ys"
+    and b: "aux = f k (lookup_pair ko ?xs k) (lookup_pair ko ?ys k)"
+    and c: "\<And>k'. k' \<in> fst ` set ?xs \<union> fst ` set ?ys \<Longrightarrow> lt_of_key_order ko k' k \<Longrightarrow>
+            f k' (lookup_pair ko ?xs k') (lookup_pair ko ?ys k') = Some Eq"
+    using assms(4) by (rule lex_ord_pair_valE, blast)
+  from a have "k \<in> fst ` set (fst xs) \<union> fst ` set (fst ys)"
+    by (simp add: set_sort_oalist_aux assms(1, 2))
+  moreover from b have "aux = f k (lookup_raw xs k) (lookup_raw ys k)"
+    by (simp add: lookup_pair_sort_oalist_aux assms(1, 2))
+  moreover have "f k' (lookup_raw xs k') (lookup_raw ys k') = Some Eq"
+    if k'_in: "k' \<in> fst ` set (fst xs) \<union> fst ` set (fst ys)" and k'_less: "lt_of_key_order ko k' k" for k'
+  proof -
+    have "f k' (lookup_raw xs k') (lookup_raw ys k') = f k' (lookup_pair ko ?xs k') (lookup_pair ko ?ys k')"
+      by (simp add: lookup_pair_sort_oalist_aux assms(1, 2))
+    also have "... = Some Eq"
+    proof (rule c)
+      from k'_in show "k' \<in> fst ` set ?xs \<union> fst ` set ?ys"
+        by (simp add:  set_sort_oalist_aux assms(1, 2))
+    qed (fact k'_less)
+    finally show ?thesis .
+  qed
+  ultimately show ?thesis ..
+qed
+
+subsubsection \<open>@{const prod_ord_raw}\<close>
+
+lemma prod_ord_rawI:
+  assumes "oalist_inv xs" and "oalist_inv ys"
+    and "\<And>k. k \<in> fst ` set (fst xs) \<union> fst ` set (fst ys) \<Longrightarrow> P k (lookup_raw xs k) (lookup_raw ys k)"
+  shows "prod_ord_raw P xs ys"
+proof -
+  obtain xs' ox where xs: "xs = (xs', ox)" by fastforce
+  from assms(1) have "oalist_inv (xs', ox)" by (simp only: xs)
+  hence *: "prod_ord_pair ox P xs' (sort_oalist_aux ox ys)" using oalist_inv_sort_oalist_aux
+  proof (rule prod_ord_pairI)
+    fix k
+    assume "k \<in> fst ` set xs' \<union> fst ` set (sort_oalist_aux ox ys)"
+    hence "k \<in> fst ` set (fst xs) \<union> fst ` set (fst ys)" by (simp add: xs set_sort_oalist_aux assms(2))
+    hence "P k (lookup_raw xs k) (lookup_raw ys k)" by (rule assms(3))
+    thus "P k (lookup_pair ox xs' k) (lookup_pair ox (sort_oalist_aux ox ys) k)"
+      by (simp add: xs lookup_pair_sort_oalist_aux assms(2))
+  qed fact
+  thus ?thesis by (simp add: xs)
+qed
+
+lemma prod_ord_rawD:
+  assumes "oalist_inv xs" and "oalist_inv ys" and "prod_ord_raw P xs ys"
+    and "k \<in> fst ` set (fst xs) \<union> fst ` set (fst ys)"
+  shows "P k (lookup_raw xs k) (lookup_raw ys k)"
+proof -
+  obtain xs' ox where xs: "xs = (xs', ox)" by fastforce
+  from assms(1) have "oalist_inv (xs', ox)" by (simp only: xs)
+  moreover note oalist_inv_sort_oalist_aux[OF assms(2)]
+  moreover from assms(3) have "prod_ord_pair ox P xs' (sort_oalist_aux ox ys)" by (simp add: xs)
+  moreover from assms(4) have "k \<in> fst ` set xs' \<union> fst ` set (sort_oalist_aux ox ys)"
+    by (simp add: xs set_sort_oalist_aux assms(2))
+  ultimately have *: "P k (lookup_pair ox xs' k) (lookup_pair ox (sort_oalist_aux ox ys) k)"
+    by (rule prod_ord_pairD)
+  thus ?thesis by (simp add: xs lookup_pair_sort_oalist_aux assms(2))
+qed
+
+corollary prod_ord_raw_alt:
+  assumes "oalist_inv xs" and "oalist_inv ys"
+  shows "prod_ord_raw P xs ys \<longleftrightarrow>
+          (\<forall>k\<in>fst ` set (fst xs) \<union> fst ` set (fst ys). P k (lookup_raw xs k) (lookup_raw ys k))"
+  using prod_ord_rawI[OF assms] prod_ord_rawD[OF assms] by meson
+
+subsubsection \<open>@{const oalist_eq_raw}\<close>
+
+lemma oalist_eq_rawI:
+  assumes "oalist_inv xs" and "oalist_inv ys"
+    and "\<And>k. k \<in> fst ` set (fst xs) \<union> fst ` set (fst ys) \<Longrightarrow> lookup_raw xs k = lookup_raw ys k"
+  shows "oalist_eq_raw xs ys"
+proof -
+  obtain xs' ox where xs: "xs = (xs', ox)" by fastforce
+  from assms(1) have "oalist_inv (xs', ox)" by (simp only: xs)
+  hence *: "xs' = sort_oalist_aux ox ys" using oalist_inv_sort_oalist_aux[OF assms(2)]
+  proof (rule lookup_pair_inj)
+    show "lookup_pair ox xs' = lookup_pair ox (sort_oalist_aux ox ys)"
+    proof
+      fix k
+      show "lookup_pair ox xs' k = lookup_pair ox (sort_oalist_aux ox ys) k"
+      proof (cases "k \<in> fst ` set xs' \<union> fst ` set (sort_oalist_aux ox ys)")
+        case True
+        hence "k \<in> fst ` set (fst xs) \<union> fst ` set (fst ys)" by (simp add: xs set_sort_oalist_aux assms(2))
+        hence "lookup_raw xs k = lookup_raw ys k" by (rule assms(3))
+        thus ?thesis by (simp add: xs lookup_pair_sort_oalist_aux assms(2))
+      next
+        case False
+        hence "k \<notin> fst ` set xs'" and "k \<notin> fst ` set (sort_oalist_aux ox ys)" by simp_all
+        with \<open>oalist_inv (xs', ox)\<close> oalist_inv_sort_oalist_aux[OF assms(2)]
+        have "lookup_pair ox xs' k = 0" and "lookup_pair ox (sort_oalist_aux ox ys) k = 0"
+          by (simp_all add: lookup_pair_eq_0)
+        thus ?thesis by simp
+      qed
+    qed
+  qed
+  thus ?thesis by (simp add: xs)
+qed
+
+lemma oalist_eq_rawD:
+  assumes "oalist_inv ys" and "oalist_eq_raw xs ys"
+  shows "lookup_raw xs = lookup_raw ys"
+proof -
+  obtain xs' ox where xs: "xs = (xs', ox)" by fastforce
+  from assms(2) have "xs' = sort_oalist_aux ox ys" by (simp add: xs)
+  hence "lookup_pair ox xs' = lookup_pair ox (sort_oalist_aux ox ys)" by simp
+  thus ?thesis by (simp add: xs lookup_pair_sort_oalist_aux assms(1))
+qed
+
+lemma oalist_eq_raw_alt:
+  assumes "oalist_inv xs" and "oalist_inv ys"
+  shows "oalist_eq_raw xs ys \<longleftrightarrow> (lookup_raw xs = lookup_raw ys)"
+  using oalist_eq_rawI[OF assms] oalist_eq_rawD[OF assms(2)] by metis
+
+subsubsection \<open>@{const sort_oalist_raw}\<close>
+
+lemma oalist_inv_sort_oalist_raw: "oalist_inv (sort_oalist_raw xs)"
+proof -
+  obtain xs' ko where xs: "xs = (xs', ko)" by fastforce
+  show ?thesis by (simp add: xs oalist_inv_sort_oalist)
+qed
+
+lemma sort_oalist_raw_id:
+  assumes "oalist_inv xs"
+  shows "sort_oalist_raw xs = xs"
+proof -
+  obtain xs' ko where xs: "xs = (xs', ko)" by fastforce
+  from assms have "oalist_inv (xs', ko)" by (simp only: xs)
+  hence "sort_oalist ko xs' = xs'" by (rule sort_oalist_id)
+  thus ?thesis by (simp add: xs)
 qed
 
 subsection \<open>Abstract characterisation\<close>
 
-typedef (overloaded) ('a, 'b) oalist = "{xs. oalist_inv xs} :: ('a::compare \<times> 'b::zero) list set"
+typedef (overloaded) ('a, 'b) oalist = "{xs::('a, 'b::zero) oalist_raw. oalist_inv xs}"
   morphisms list_of_oalist Abs_oalist
   by (auto intro: oalist_inv_Nil)
-
-setup_lifting type_definition_oalist
 
 lemma oalist_eq_iff: "xs = ys \<longleftrightarrow> list_of_oalist xs = list_of_oalist ys"
   by (simp add: list_of_oalist_inject)
@@ -414,165 +2908,354 @@ lemma oalist_eqI: "list_of_oalist xs = list_of_oalist ys \<Longrightarrow> xs = 
 
 text \<open>Formal, totalized constructor for @{typ "('a, 'b) oalist"}:\<close>
 
-definition OAlist :: "('a \<times> 'b) list \<Rightarrow> ('a::compare, 'b::zero) oalist" where
-  "OAlist xs = Abs_oalist (sort_alist xs)"
+definition OAlist :: "('a \<times> 'b) list \<times> 'a key_order \<Rightarrow> ('a, 'b::zero) oalist" where
+  "OAlist xs = Abs_oalist (sort_oalist_raw xs)"
+
+definition [simp]: "oalist_of_list = OAlist"
 
 lemma oalist_inv_list_of_oalist [simp, intro]: "oalist_inv (list_of_oalist xs)"
   using list_of_oalist [of xs] by simp
 
-lemma list_of_oalist_OAlist [simp]:
-  "list_of_oalist (OAlist xs) = sort_alist xs"
-  by (simp add: OAlist_def Abs_oalist_inverse oalist_inv_sort_alist)
+lemma list_of_oalist_OAlist: "list_of_oalist (OAlist xs) = sort_oalist_raw xs"
+proof -
+  obtain xs' ox where xs: "xs = (xs', ox)" by fastforce
+  show ?thesis by (simp add: xs OAlist_def Abs_oalist_inverse oalist_inv_sort_oalist)
+qed
 
 lemma OAlist_list_of_oalist [simp, code abstype]: "OAlist (list_of_oalist xs) = xs"
-  by (simp add: OAlist_def list_of_oalist_inverse sort_alist_id)
+proof -
+  obtain xs' ox where xs: "list_of_oalist xs = (xs', ox)" by fastforce
+  have "oalist_inv (xs', ox)" by (simp add: xs[symmetric])
+  thus ?thesis by (simp add: xs OAlist_def sort_oalist_id, simp add: list_of_oalist_inverse xs[symmetric])
+qed
 
-text \<open>Fundamental operations:\<close>
+lemma list_of_oalist_OAlist_id:
+  assumes "oalist_inv xs"
+  shows "list_of_oalist (OAlist xs) = xs"
+proof -
+  obtain xs' ox where xs: "xs = (xs', ox)" by fastforce
+  from assms show ?thesis by (simp add: xs Abs_oalist_inverse OAlist_def sort_oalist_id)
+qed
+
+lemma [code abstract]: "list_of_oalist (oalist_of_list xs) = sort_oalist_raw xs"
+  by (simp add: list_of_oalist_OAlist)
+
+subsubsection \<open>Fundamental operations\<close>
 
 context
 begin
 
-qualified definition empty :: "('a::compare, 'b::zero) oalist"
-  where "empty = OAlist []"
+qualified definition lookup :: "('a, 'b::zero) oalist \<Rightarrow> 'a \<Rightarrow> 'b"
+  where "lookup xs = lookup_raw (list_of_oalist xs)"
 
-qualified definition insert :: "('a \<times> 'b) \<Rightarrow> ('a, 'b) oalist \<Rightarrow> ('a::compare, 'b::zero) oalist"
-  where "insert x xs = OAlist (update_by' x (list_of_oalist xs))"
+qualified definition sorted_domain :: "'a key_order \<Rightarrow> ('a, 'b::zero) oalist \<Rightarrow> 'a list"
+  where "sorted_domain ko xs = sorted_domain_raw ko (list_of_oalist xs)"
 
-qualified definition update_by_fun :: "'a \<Rightarrow> ('b \<Rightarrow> 'b) \<Rightarrow> ('a, 'b) oalist \<Rightarrow> ('a::compare, 'b::zero) oalist"
+qualified definition empty :: "'a key_order \<Rightarrow> ('a, 'b::zero) oalist"
+  where "empty ko = OAlist ([], ko)"
+
+qualified definition except_min :: "('a key_order) \<Rightarrow> ('a, 'b) oalist \<Rightarrow> ('a, 'b::zero) oalist"
+  where "except_min ko xs = OAlist (except_min_raw ko (list_of_oalist xs))"
+
+qualified definition min_key_val :: "('a key_order) \<Rightarrow> ('a, 'b) oalist \<Rightarrow> ('a \<times> 'b::zero)"
+  where "min_key_val ko xs = min_key_val_raw ko (list_of_oalist xs)"
+
+qualified definition insert :: "('a \<times> 'b) \<Rightarrow> ('a, 'b) oalist \<Rightarrow> ('a, 'b::zero) oalist"
+  where "insert x xs = OAlist (update_by_raw x (list_of_oalist xs))"
+
+qualified definition update_by_fun :: "'a \<Rightarrow> ('b \<Rightarrow> 'b) \<Rightarrow> ('a, 'b) oalist \<Rightarrow> ('a, 'b::zero) oalist"
   where "update_by_fun k f xs = OAlist (update_by_fun_raw k f (list_of_oalist xs))"
 
-qualified definition update_by_fun_gr :: "'a \<Rightarrow> ('b \<Rightarrow> 'b) \<Rightarrow> ('a, 'b) oalist \<Rightarrow> ('a::compare, 'b::zero) oalist"
+qualified definition update_by_fun_gr :: "'a \<Rightarrow> ('b \<Rightarrow> 'b) \<Rightarrow> ('a, 'b) oalist \<Rightarrow> ('a, 'b::zero) oalist"
   where "update_by_fun_gr k f xs = OAlist (update_by_fun_gr_raw k f (list_of_oalist xs))"
 
-qualified definition map :: "(('a \<times> 'b) \<Rightarrow> ('d \<times> 'c)) \<Rightarrow> ('a::compare, 'b::zero) oalist \<Rightarrow>
-                            ('d::compare, 'c::zero) oalist"
-  where "map f xs = OAlist (List.map f (list_of_oalist xs))"
+qualified definition filter :: "(('a \<times> 'b) \<Rightarrow> bool) \<Rightarrow> ('a, 'b) oalist \<Rightarrow> ('a, 'b::zero) oalist"
+  where "filter P xs = OAlist (filter_raw P (list_of_oalist xs))"
 
-qualified definition lookup :: "('a::compare, 'b::zero) oalist \<Rightarrow> 'a \<Rightarrow> 'b"
-  where "lookup xs = c.lookup_default compare 0 (list_of_oalist xs)"
+qualified definition map_val :: "('a \<Rightarrow> 'b \<Rightarrow> 'c) \<Rightarrow> ('a, 'b::zero) oalist \<Rightarrow> ('a, 'c::zero) oalist"
+  where "map_val f xs = OAlist (map_val_raw f (list_of_oalist xs))"
 
-qualified definition filter :: "(('a \<times> 'b) \<Rightarrow> bool) \<Rightarrow> ('a, 'b) oalist \<Rightarrow> ('a::compare, 'b::zero) oalist"
-  where "filter P xs = OAlist (List.filter P (list_of_oalist xs))"
-
-qualified definition map2_val_neutr :: "('a \<Rightarrow> 'b \<Rightarrow> 'b \<Rightarrow> 'b) \<Rightarrow> ('a, 'b) oalist \<Rightarrow> ('a, 'b) oalist \<Rightarrow>
-                                    ('a::compare, 'b::zero) oalist"
-  where "map2_val_neutr f xs ys = OAlist (map2_val_neutr_raw f (list_of_oalist xs) (list_of_oalist ys))"
+qualified definition map2_val :: "('a \<Rightarrow> 'b \<Rightarrow> 'c \<Rightarrow> 'd) \<Rightarrow> ('a, 'b::zero) oalist \<Rightarrow> ('a, 'c::zero) oalist \<Rightarrow>
+                                        ('a, 'd::zero) oalist"
+  where "map2_val f xs ys =
+            OAlist (map2_val_raw f (map_val_raw (\<lambda>k b. f k b 0)) (map_val_raw (\<lambda>k. f k 0))
+              (list_of_oalist xs) (list_of_oalist ys))"
 
 qualified definition map2_val_rneutr :: "('a \<Rightarrow> 'b \<Rightarrow> 'c \<Rightarrow> 'b) \<Rightarrow> ('a, 'b) oalist \<Rightarrow> ('a, 'c::zero) oalist \<Rightarrow>
-                                    ('a::compare, 'b::zero) oalist"
-  where "map2_val_rneutr f xs ys = OAlist (map2_val_rneutr_raw f (list_of_oalist xs) (list_of_oalist ys))"
+                                         ('a, 'b::zero) oalist"
+  where "map2_val_rneutr f xs ys =
+            OAlist (map2_val_raw f id (map_val_raw (\<lambda>k. f k 0)) (list_of_oalist xs) (list_of_oalist ys))"
 
-qualified definition lex_ord :: "('a \<Rightarrow> ('b comp_opt)) \<Rightarrow> ('a::compare, 'b::zero) oalist comp_opt"
-  where "lex_ord f xs ys = lex_ord_raw f (list_of_oalist xs) (list_of_oalist ys)"
+qualified definition map2_val_neutr :: "('a \<Rightarrow> 'b \<Rightarrow> 'b \<Rightarrow> 'b) \<Rightarrow> ('a, 'b) oalist \<Rightarrow> ('a, 'b) oalist \<Rightarrow>
+                                        ('a, 'b::zero) oalist"
+  where "map2_val_neutr f xs ys = OAlist (map2_val_raw f id id (list_of_oalist xs) (list_of_oalist ys))"
 
-qualified definition prod_ord :: "('a \<Rightarrow> 'b \<Rightarrow> 'b \<Rightarrow> bool) \<Rightarrow> ('a, 'b) oalist \<Rightarrow>
-                                  ('a::compare, 'b::zero) oalist \<Rightarrow> bool"
+qualified definition lex_ord :: "('a key_order) \<Rightarrow> ('a \<Rightarrow> ('b, 'c) comp_opt) \<Rightarrow>
+                                (('a, 'b::zero) oalist, ('a, 'c::zero) oalist) comp_opt"
+  where "lex_ord ko f xs ys = lex_ord_raw ko f (list_of_oalist xs) (list_of_oalist ys)"
+
+qualified definition prod_ord :: "('a \<Rightarrow> 'b \<Rightarrow> 'c \<Rightarrow> bool) \<Rightarrow> ('a, 'b::zero) oalist \<Rightarrow>
+                                  ('a, 'c::zero) oalist \<Rightarrow> bool"
   where "prod_ord f xs ys = prod_ord_raw f (list_of_oalist xs) (list_of_oalist ys)"
 
-definition except_min :: "('a, 'b) oalist \<Rightarrow> ('a::compare, 'b::zero) oalist"
-  where "except_min xs = OAlist (tl (list_of_oalist xs))"
-
-text \<open>Derived operations\<close>
-
-qualified definition map_val :: "('a \<Rightarrow> 'b \<Rightarrow> 'c) \<Rightarrow> ('a, 'b::zero) oalist \<Rightarrow> ('a::compare, 'c::zero) oalist"
-  where "map_val f xs = map (\<lambda>x. (fst x, f (fst x) (snd x))) xs"
+qualified definition oalist_eq :: "('a, 'b) oalist \<Rightarrow> ('a, 'b::zero) oalist \<Rightarrow> bool"
+  where "oalist_eq xs ys = oalist_eq_raw (list_of_oalist xs) (list_of_oalist ys)"
 
 end
 
-subsection \<open>Executable version obeying invariant\<close>
+subsubsection \<open>@{const OAlist.sorted_domain}\<close>
 
-lemma list_of_oalist_empty [simp, code abstract]: "list_of_oalist OAlist.empty = []"
-  by (simp add: OAlist.empty_def sort_alist_def)
+lemma set_sorted_domain: "set (OAlist.sorted_domain ko xs) = fst ` set (fst (list_of_oalist xs))"
+  unfolding OAlist.sorted_domain_def using oalist_inv_list_of_oalist by (rule set_sorted_domain_raw)
+
+lemma in_sorted_domain_iff_lookup: "k \<in> set (OAlist.sorted_domain ko xs) \<longleftrightarrow> (OAlist.lookup xs k \<noteq> 0)"
+  unfolding OAlist.sorted_domain_def OAlist.lookup_def using oalist_inv_list_of_oalist
+  by (rule in_sorted_domain_raw_iff_lookup_raw)
+
+lemma sorted_sorted_domain: "sorted_wrt (lt_of_key_order ko) (OAlist.sorted_domain ko xs)"
+  unfolding OAlist.sorted_domain_def using oalist_inv_list_of_oalist by (rule sorted_sorted_domain_raw)
+
+subsubsection \<open>@{const OAlist.empty}\<close>
+
+lemma list_of_oalist_empty [simp, code abstract]: "list_of_oalist (OAlist.empty ko) = ([], ko)"
+  by (simp add: OAlist.empty_def sort_oalist_def list_of_oalist_OAlist)
+
+lemma lookup_empty: "OAlist.lookup (OAlist.empty ko) k = 0"
+  by (simp add: OAlist.lookup_def)
+
+subsubsection \<open>@{const OAlist.except_min}\<close>
+
+lemma list_of_oalist_except_min [simp, code abstract]:
+  "list_of_oalist (OAlist.except_min ko xs) = except_min_raw ko (list_of_oalist xs)"
+  unfolding OAlist.except_min_def
+  by (rule list_of_oalist_OAlist_id, rule oalist_inv_except_min_raw, fact oalist_inv_list_of_oalist)
+
+lemma lookup_except_min:
+  "OAlist.lookup (OAlist.except_min ko xs) k =
+        (if (\<forall>k'\<in>fst ` set (fst (list_of_oalist xs)). le_of_key_order ko k k') then 0 else OAlist.lookup xs k)"
+  by (simp add: OAlist.lookup_def lookup_raw_except_min_raw split del: if_split cong: if_cong)
+
+subsubsection \<open>@{const OAlist.min_key_val}\<close>
+
+lemma min_key_val_in:
+  assumes "fst (list_of_oalist xs) \<noteq> []"
+  shows "OAlist.min_key_val ko xs \<in> set (fst (list_of_oalist xs))"
+  unfolding OAlist.min_key_val_def using assms by (rule min_key_val_raw_in)
+
+lemma snd_min_key_val:
+  assumes "fst (list_of_oalist xs) \<noteq> []"
+  shows "snd (OAlist.min_key_val ko xs) = OAlist.lookup xs (fst (OAlist.min_key_val ko xs))"
+  unfolding OAlist.lookup_def OAlist.min_key_val_def using oalist_inv_list_of_oalist assms
+  by (rule snd_min_key_val_raw)
+
+lemma min_key_val_minimal:
+  assumes "z \<in> set (fst (list_of_oalist xs))"
+  shows "le_of_key_order ko (fst (OAlist.min_key_val ko xs)) (fst z)"
+  unfolding OAlist.min_key_val_def by (rule min_key_val_raw_minimal, fact oalist_inv_list_of_oalist, fact)
+
+subsubsection \<open>@{const OAlist.insert}\<close>
 
 lemma list_of_oalist_insert [simp, code abstract]:
-  "list_of_oalist (OAlist.insert x xs) = update_by' x (list_of_oalist xs)"
+  "list_of_oalist (OAlist.insert x xs) = update_by_raw x (list_of_oalist xs)"
   unfolding OAlist.insert_def
-  by (metis (no_types, hide_lams) OAlist_list_of_oalist foldr.simps(2) list_of_oalist_OAlist o_def sort_alist_def)
+  by (rule list_of_oalist_OAlist_id, rule oalist_inv_update_by_raw, fact oalist_inv_list_of_oalist)
 
-lemma update_by_fun_gr_eq_update_by_fun: "OAlist.update_by_fun_gr = OAlist.update_by_fun"
-  apply (rule, rule, rule, simp only: OAlist.update_by_fun_gr_def OAlist.update_by_fun_def)
-  by (metis oalist_invD2 oalist_inv_list_of_oalist update_by_fun_gr_raw_eq_update_by_fun_raw)
+lemma lookup_insert: "OAlist.lookup (OAlist.insert (k, v) xs) k' = (if k = k' then v else OAlist.lookup xs k')"
+  by (simp add: OAlist.lookup_def lookup_raw_update_by_raw split del: if_split cong: if_cong)
+
+subsubsection \<open>@{const OAlist.update_by_fun} and @{const OAlist.update_by_fun_gr}\<close>
 
 lemma list_of_oalist_update_by_fun [simp, code abstract]:
   "list_of_oalist (OAlist.update_by_fun k f xs) = update_by_fun_raw k f (list_of_oalist xs)"
-  sorry
+  unfolding OAlist.update_by_fun_def
+  by (rule list_of_oalist_OAlist_id, rule oalist_inv_update_by_fun_raw, fact oalist_inv_list_of_oalist)
+
+lemma lookup_update_by_fun:
+  "OAlist.lookup (OAlist.update_by_fun k f xs) k' = (if k = k' then f else id) (OAlist.lookup xs k')"
+  by (simp add: OAlist.lookup_def lookup_raw_update_by_fun_raw split del: if_split cong: if_cong)
 
 lemma list_of_oalist_update_by_fun_gr [simp, code abstract]:
   "list_of_oalist (OAlist.update_by_fun_gr k f xs) = update_by_fun_gr_raw k f (list_of_oalist xs)"
-  apply (simp only: update_by_fun_gr_eq_update_by_fun list_of_oalist_update_by_fun)
-  by (metis oalist_invD2 oalist_inv_list_of_oalist update_by_fun_gr_raw_eq_update_by_fun_raw)
+  unfolding OAlist.update_by_fun_gr_def
+  by (rule list_of_oalist_OAlist_id, rule oalist_inv_update_by_fun_gr_raw, fact oalist_inv_list_of_oalist)
+
+lemma update_by_fun_gr_eq_update_by_fun: "OAlist.update_by_fun_gr = OAlist.update_by_fun"
+  by (rule, rule, rule,
+      simp add: OAlist.update_by_fun_gr_def OAlist.update_by_fun_def update_by_fun_gr_raw_eq_update_by_fun_raw)
+
+subsubsection \<open>@{const OAlist.filter}\<close>
 
 lemma list_of_oalist_filter [simp, code abstract]:
-  "list_of_oalist (OAlist.filter P xs) = List.filter P (list_of_oalist xs)"
-  by (simp add: OAlist.filter_def, rule sort_alist_id, rule oalist_inv_filter, simp)
+  "list_of_oalist (OAlist.filter P xs) = filter_raw P (list_of_oalist xs)"
+  unfolding OAlist.filter_def
+  by (rule list_of_oalist_OAlist_id, rule oalist_inv_filter_raw, fact oalist_inv_list_of_oalist)
+
+lemma lookup_filter: "OAlist.lookup (OAlist.filter P xs) k = (let v = OAlist.lookup xs k in if P (k, v) then v else 0)"
+  by (simp add: OAlist.lookup_def lookup_raw_filter_raw)
+
+subsubsection \<open>@{const OAlist.map_val}\<close>
 
 lemma list_of_oalist_map_val [simp, code abstract]:
   "list_of_oalist (OAlist.map_val f xs) = map_val_raw f (list_of_oalist xs)"
-  sorry
+  unfolding OAlist.map_val_def
+  by (rule list_of_oalist_OAlist_id, rule oalist_inv_map_val_raw, fact oalist_inv_list_of_oalist)
 
-lemma list_of_oalist_map2_val_neutr [simp, code abstract]:
-  "list_of_oalist (OAlist.map2_val_neutr f xs ys) = map2_val_neutr_raw f (list_of_oalist xs) (list_of_oalist ys)"
-  sorry
+lemma lookup_map_val:
+  assumes "\<And>k'. f k' 0 = 0"
+  shows "OAlist.lookup (OAlist.map_val f xs) k = f k (OAlist.lookup xs k)"
+  by (simp add: OAlist.lookup_def lookup_raw_map_val_raw assms)
+
+subsubsection \<open>@{const OAlist.map2_val}, @{const OAlist.map2_val_rneutr} and @{const OAlist.map2_val_neutr}\<close>
+
+lemma list_of_oalist_map2_val [simp, code abstract]:
+  "list_of_oalist (OAlist.map2_val f xs ys) =
+      map2_val_raw f (map_val_raw (\<lambda>k b. f k b 0)) (map_val_raw (\<lambda>k. f k 0)) (list_of_oalist xs) (list_of_oalist ys)"
+  unfolding OAlist.map2_val_def
+  by (rule list_of_oalist_OAlist_id, rule oalist_inv_map2_val_raw,
+      fact oalist_inv_list_of_oalist, fact oalist_inv_list_of_oalist,
+      fact map2_val_compat'_map_val_raw, fact map2_val_compat'_map_val_raw)
 
 lemma list_of_oalist_map2_val_rneutr [simp, code abstract]:
-  "list_of_oalist (OAlist.map2_val_rneutr f xs ys) = map2_val_rneutr_raw f (list_of_oalist xs) (list_of_oalist ys)"
-  sorry
+  "list_of_oalist (OAlist.map2_val_rneutr f xs ys) =
+      map2_val_raw f id (map_val_raw (\<lambda>k c. f k 0 c)) (list_of_oalist xs) (list_of_oalist ys)"
+  unfolding OAlist.map2_val_rneutr_def
+  by (rule list_of_oalist_OAlist_id, rule oalist_inv_map2_val_raw,
+      fact oalist_inv_list_of_oalist, fact oalist_inv_list_of_oalist,
+      fact map2_val_compat'_id, fact map2_val_compat'_map_val_raw)
 
-lemma list_of_oalist_except_min [code abstract]:
-  "list_of_oalist (except_min xs) = (tl (list_of_oalist xs))"
-  sorry
+lemma list_of_oalist_map2_val_neutr [simp, code abstract]:
+  "list_of_oalist (OAlist.map2_val_neutr f xs ys) = map2_val_raw f id id (list_of_oalist xs) (list_of_oalist ys)"
+  unfolding OAlist.map2_val_neutr_def
+  by (rule list_of_oalist_OAlist_id, rule oalist_inv_map2_val_raw,
+      fact oalist_inv_list_of_oalist, fact oalist_inv_list_of_oalist,
+      fact map2_val_compat'_id, fact map2_val_compat'_id)
 
-(* TODO: Prove relationship between operations and "lookup", and prove that "lookup" is injective. *)
+lemma lookup_map2_val:
+  assumes "\<And>k. f k 0 0 = 0"
+  shows "OAlist.lookup (OAlist.map2_val f xs ys) k = f k (OAlist.lookup xs k) (OAlist.lookup ys k)"
+  by (simp add: OAlist.lookup_def lookup_raw_map2_val_raw map2_val_compat'_map_val_raw assms)
 
-subsection \<open>Further Lemmas\<close>
+lemma lookup_map2_val_rneutr:
+  assumes "\<And>k x. f k x 0 = x"
+  shows "OAlist.lookup (OAlist.map2_val_rneutr f xs ys) k = f k (OAlist.lookup xs k) (OAlist.lookup ys k)"
+proof (simp add: OAlist.lookup_def, rule lookup_raw_map2_val_raw)
+  fix zs::"('a, 'b) oalist_raw"
+  assume "oalist_inv zs"
+  thus "id zs = map_val_raw (\<lambda>k v. f k v 0) zs" by (simp add: assms map_raw_id)
+qed (fact oalist_inv_list_of_oalist, fact oalist_inv_list_of_oalist,
+    fact map2_val_compat'_id, fact map2_val_compat'_map_val_raw, rule refl, simp only: assms)
+
+lemma lookup_map2_val_neutr:
+  assumes "\<And>k x. f k x 0 = x" and "\<And>k x. f k 0 x = x"
+  shows "OAlist.lookup (OAlist.map2_val_neutr f xs ys) k = f k (OAlist.lookup xs k) (OAlist.lookup ys k)"
+proof (simp add: OAlist.lookup_def, rule lookup_raw_map2_val_raw)
+  fix zs::"('a, 'b) oalist_raw"
+  assume "oalist_inv zs"
+  thus "id zs = map_val_raw (\<lambda>k v. f k v 0) zs" by (simp add: assms(1) map_raw_id)
+next
+  fix zs::"('a, 'b) oalist_raw"
+  assume "oalist_inv zs"
+  thus "id zs = map_val_raw (\<lambda>k. f k 0) zs" by (simp add: assms(2) map_raw_id)
+qed (fact oalist_inv_list_of_oalist, fact oalist_inv_list_of_oalist,
+    fact map2_val_compat'_id, fact map2_val_compat'_id, simp only: assms(1))
 
 lemma map2_val_rneutr_singleton_eq_update_by_fun:
-  assumes "\<And>a x. f a x 0 = x" and "list_of_oalist ys = [(k, v)]"
+  assumes "\<And>a x. f a x 0 = x" and "list_of_oalist ys = ([(k, v)], oy)"
   shows "OAlist.map2_val_rneutr f xs ys = OAlist.update_by_fun k (\<lambda>x. f k x v) xs"
-  by (simp add: OAlist.map2_val_rneutr_def OAlist.update_by_fun_def assms map2_val_rneutr_raw_singleton_eq_update_by_fun_raw)
+  by (simp add: OAlist.map2_val_rneutr_def OAlist.update_by_fun_def assms map2_val_raw_singleton_eq_update_by_fun_raw)
 
-lemma map2_val_rneutr_eq_map2_val_neutr:
-  assumes "\<And>a x. f a x 0 = x" and "\<And>a. f a 0 = id"
-  shows "OAlist.map2_val_rneutr f = OAlist.map2_val_neutr f"
-  by (rule, rule, simp add: OAlist.map2_val_rneutr_def OAlist.map2_val_neutr_def assms map2_val_rneutr_raw_eq_map2_val_neutr_raw)
+subsubsection \<open>@{const OAlist.lex_ord}, @{const OAlist.prod_ord} and @{const OAlist.oalist_eq}\<close>
 
-text \<open>Explicit executable conversion\<close>
+lemma lex_ord_EqI:
+  "(\<And>k. k \<in> fst ` set (fst (list_of_oalist xs)) \<union> fst ` set (fst (list_of_oalist ys)) \<Longrightarrow>
+     f k (OAlist.lookup xs k) (OAlist.lookup ys k) = Some Eq) \<Longrightarrow>
+  OAlist.lex_ord ko f xs ys = Some Eq"
+  by (simp add: OAlist.lex_ord_def OAlist.lookup_def, rule lex_ord_raw_EqI,
+      rule oalist_inv_list_of_oalist, rule oalist_inv_list_of_oalist, blast)
 
-definition [simp]: "oalist_of_list = OAlist"
+lemma lex_ord_valI:
+  assumes "aux \<noteq> Some Eq" and "k \<in> fst ` set (fst (list_of_oalist xs)) \<union> fst ` set (fst (list_of_oalist ys))"
+  shows "aux = f k (OAlist.lookup xs k) (OAlist.lookup ys k) \<Longrightarrow>
+         (\<And>k'. k' \<in> fst ` set (fst (list_of_oalist xs)) \<union> fst ` set (fst (list_of_oalist ys)) \<Longrightarrow>
+              lt_of_key_order ko k' k \<Longrightarrow> f k' (OAlist.lookup xs k') (OAlist.lookup ys k') = Some Eq) \<Longrightarrow>
+          OAlist.lex_ord ko f xs ys = aux"
+  by (simp (no_asm_use) add: OAlist.lex_ord_def OAlist.lookup_def, rule lex_ord_raw_valI,
+      rule oalist_inv_list_of_oalist, rule oalist_inv_list_of_oalist, rule assms(1), rule assms(2), blast+)
 
-lemma [code abstract]: "list_of_oalist (oalist_of_list xs) = sort_alist xs"
-  by simp
+lemma lex_ord_EqD:
+  "OAlist.lex_ord ko f xs ys = Some Eq \<Longrightarrow>
+   k \<in> fst ` set (fst (list_of_oalist xs)) \<union> fst ` set (fst (list_of_oalist ys)) \<Longrightarrow>
+   f k (OAlist.lookup xs k) (OAlist.lookup ys k) = Some Eq"
+  by (simp add: OAlist.lex_ord_def OAlist.lookup_def, rule lex_ord_raw_EqD[where f=f],
+      rule oalist_inv_list_of_oalist, rule oalist_inv_list_of_oalist, assumption, simp)
 
-instantiation oalist :: (compare, "{equal,zero}") equal
-begin
+lemma lex_ord_valE:
+  assumes "OAlist.lex_ord ko f xs ys = aux" and "aux \<noteq> Some Eq"
+  obtains k where "k \<in> fst ` set (fst (list_of_oalist xs)) \<union> fst ` set (fst (list_of_oalist ys))"
+    and "aux = f k (OAlist.lookup xs k) (OAlist.lookup ys k)"
+    and "\<And>k'. k' \<in> fst ` set (fst (list_of_oalist xs)) \<union> fst ` set (fst (list_of_oalist ys)) \<Longrightarrow>
+            lt_of_key_order ko k' k \<Longrightarrow> f k' (OAlist.lookup xs k') (OAlist.lookup ys k') = Some Eq"
+proof -
+  note oalist_inv_list_of_oalist oalist_inv_list_of_oalist
+  moreover from assms(1) have "lex_ord_raw ko f (list_of_oalist xs) (list_of_oalist ys) = aux"
+    by (simp only: OAlist.lex_ord_def)
+  ultimately obtain k where 1: "k \<in> fst ` set (fst (list_of_oalist xs)) \<union> fst ` set (fst (list_of_oalist ys))"
+    and "aux = f k (lookup_raw (list_of_oalist xs) k) (lookup_raw (list_of_oalist ys) k)"
+    and "\<And>k'. k' \<in> fst ` set (fst (list_of_oalist xs)) \<union> fst ` set (fst (list_of_oalist ys)) \<Longrightarrow>
+            lt_of_key_order ko k' k \<Longrightarrow>
+            f k' (lookup_raw (list_of_oalist xs) k') (lookup_raw (list_of_oalist ys) k') = Some Eq"
+    using assms(2) by (rule lex_ord_raw_valE, blast)
+  from this(2, 3) have "aux = f k (OAlist.lookup xs k) (OAlist.lookup ys k)"
+    and "\<And>k'. k' \<in> fst ` set (fst (list_of_oalist xs)) \<union> fst ` set (fst (list_of_oalist ys)) \<Longrightarrow>
+            lt_of_key_order ko k' k \<Longrightarrow> f k' (OAlist.lookup xs k') (OAlist.lookup ys k') = Some Eq"
+    by (simp_all only: OAlist.lookup_def)
+  with 1 show ?thesis ..
+qed
 
-definition "equal_oalist xs ys \<longleftrightarrow> equal_class.equal (list_of_oalist xs) (list_of_oalist ys)"
+lemma prod_ord_alt:
+  "OAlist.prod_ord P xs ys \<longleftrightarrow>
+                  (\<forall>k\<in>fst ` set (fst (list_of_oalist xs)) \<union> fst ` set (fst (list_of_oalist ys)).
+                      P k (OAlist.lookup xs k) (OAlist.lookup ys k))"
+  by (simp add: OAlist.prod_ord_def OAlist.lookup_def prod_ord_raw_alt)
 
-instance
-  by (standard, simp add: equal_oalist_def equal oalist_eq_iff)
+lemma oalist_eq_alt: "OAlist.oalist_eq xs ys \<longleftrightarrow> (OAlist.lookup xs = OAlist.lookup ys)"
+  by (simp add: OAlist.oalist_eq_def OAlist.lookup_def oalist_eq_raw_alt)
 
-end
+subsection \<open>Experiment\<close>
 
-lemmas [code] = equal_oalist_def
+definition rv_key_order :: "'a::linorder key_order" where "rv_key_order = - key_order_of_le"
 
-instantiation nat :: compare
-begin
+lemma equal_key_order_code [code]:
+  "HOL.equal key_order_of_le key_order_of_le = True"
+  "HOL.equal key_order_of_le rv_key_order = False"
+  "HOL.equal rv_key_order key_order_of_le = False"
+  "HOL.equal rv_key_order rv_key_order = True"
+  sorry
 
-definition compare_nat :: "nat comparator" where
-  "compare_nat = comparator_of_le"
+code_datatype key_order_of_le rv_key_order
 
-instance sorry
+lemma key_compare_rv_key_order [code]:
+  "key_compare rv_key_order = (\<lambda>x y. if x < y then Gt else if x = y then Eq else Lt)"
+  unfolding rv_key_order_def by (intro ext, auto simp: key_compare_key_order_of_le)
 
-end
+lemmas [code] = key_compare_key_order_of_le
 
-value [code] "oalist_of_list [(0::nat, 4::nat), (1, 3), (0, 2), (1, 1)]"
+value [code] "oalist_of_list ([(0::nat, 4::nat), (1, 3), (0, 2), (1, 1)], key_order_of_le)"
 
-value [code] "except_min (oalist_of_list [(1, 3), (0::nat, 4::nat), (0, 2), (1, 1)])"
+value [code] "OAlist.except_min rv_key_order (oalist_of_list ([(1, 3), (0::nat, 4::nat), (0, 2), (1, 1)], key_order_of_le))"
 
-value [code] "OAlist.lookup (oalist_of_list [(0::nat, 4::nat), (1, 3), (0, 2), (1, 1)]) 1"
+value [code] "OAlist.lookup (oalist_of_list ([(0::nat, 4::nat), (1, 3), (0, 2), (1, 1)], key_order_of_le)) 1"
 
-value [code] "OAlist.prod_ord (\<lambda>_. less_eq)
-                (oalist_of_list [(1, 4), (0::nat, 4::nat), (1, 3), (0, 2), (1, 1)])
-                (oalist_of_list [(0::nat, 4::nat), (1, 3), (0, 2), (1, 1)])"
+value [code] "OAlist.prod_ord (\<lambda>_. greater_eq)
+                (oalist_of_list ([(1, 4), (0::nat, 4::nat), (1, 3), (0, 2), (3, 1)], key_order_of_le))
+                (oalist_of_list ([(0::nat, 4::nat), (1, 3), (2, 2), (1, 1)], rv_key_order))"
+
+value [code] "OAlist.oalist_eq
+                (oalist_of_list ([(1, 4), (0::nat, 2::nat), (2, 3)], key_order_of_le))
+                (oalist_of_list ([(0::nat, 2::nat), (2, 3), (0, 2), (1, 4)], rv_key_order))"
+
+value [code] "OAlist.map2_val_rneutr (\<lambda>_. minus)
+                (oalist_of_list ([(1, 4), (0::nat, 4::nat), (1, 3), (0, 2), (3, 1)], key_order_of_le))
+                (oalist_of_list ([(0::nat, 4::nat), (1, 3), (2, 2), (1, 1)], rv_key_order))"
 
 end (* theory *)
